<?xml version="1.0" encoding="ISO-8859-1"?>
<rdf:RDF
    xmlns:rdf='http://www.w3.org/1999/02/22-rdf-syntax-ns#'
    xmlns:rdfs='http://www.w3.org/2000/01/rdf-schema#'
    xmlns:skos='http://www.w3.org/2004/02/skos/core#'
    xmlns:nt2='http://nasataxonomy.jpl.nasa.gov/cvFields#'
    xmlns:dcterms='http://purl.org/dc/terms/'
    xmlns:dc='http://purl.org/dc/elements/1.1/'>
 <skos:Concept rdf:about='urn:comp:37'>
  <skos:prefLabel>Environmental Control and Life Support Systems</skos:prefLabel>
  <skos:altLabel>ECLSS</skos:altLabel>
  <skos:broader rdf:resource='urn:comp:1244'/>
  <skos:scopeNote>Knowledge, capabilities and practices associated with
    environmental control and/or life support systems used to
    protect life in dangerous or insupportive environments for
    flight or ground operations, including related
    instrumentation, controls, data acquisition, pneumatics and
    mechanisms. May include knowledge and capabilities needed
    for development of advanced and/or regenerative life
    support, such as how to apply plant physiology and
    pathology, microbial ecology, molecular biology, biological
    engineering, chemistry, chemical engineering and landscape
    ecology to development of advanced, regenerative life
    support such as air and water recycling, solid waste
    resource recovery, food sources and thermal environmental
    control.
  </skos:scopeNote>
  <nt2:status>Approved</nt2:status>
  <nt2:type>Descriptor</nt2:type>
  <nt2:inputdate>2006-12-13</nt2:inputdate>
  <dcterms:modified>2006-12-13</dcterms:modified>
  <nt2:code>37</nt2:code>
 </skos:Concept>
 <skos:Concept rdf:about='urn:comp:1280'>
  <skos:prefLabel>Chemical Competency Suite</skos:prefLabel>
  <skos:broader rdf:resource='urn:comp:1208'/>
  <skos:narrower rdf:resource='urn:comp:25'/>
  <skos:narrower rdf:resource='urn:comp:18'/>
  <nt2:status>Approved</nt2:status>
  <nt2:type>Descriptor</nt2:type>
  <nt2:inputdate>2006-12-13</nt2:inputdate>
  <dcterms:modified>2006-12-13</dcterms:modified>
  <nt2:code>1280</nt2:code>
 </skos:Concept>
 <skos:Concept rdf:about='urn:comp:121'>
  <skos:prefLabel>Cost Estimation and Analysis</skos:prefLabel>
  <skos:altLabel>COSTEST</skos:altLabel>
  <skos:broader rdf:resource='urn:comp:1150'/>
  <skos:changeNote>Name changed from "Cost Estimation Analysis" and Scope Note
    updated.
  </skos:changeNote>
  <skos:scopeNote>This competency refers to the knowledge, capabilities, and
    practices associated with the determination, estimation,
    and analysis of costs. It encompasses analytical techniques
    required to develop and assess estimates for
    hardware/software acquisition; design, integration and
    test, production, operations and support costs (e.g.,
    life-cycle costs) of programs, projects, systems, and
    resources. Estimating and cost analysis methodologies used
    include engineering, parametric, grass roots, analogy, cost
    performance analysis, schedule analysis, and statistical
    risk analysis. Knowledge and skills required include Work
    Breakdown Structure (WBS) development, data collection,
    cost estimating relationship development and documentation,
    application of cost models, and evaluation of cost realism
    in proposals.
  </skos:scopeNote>
  <nt2:status>Approved</nt2:status>
  <nt2:type>Descriptor</nt2:type>
  <nt2:inputdate>2003-07-21</nt2:inputdate>
  <dcterms:dateAccepted>2006-04-05</dcterms:dateAccepted>
  <dcterms:modified>2006-12-18</dcterms:modified>
  <nt2:code>121</nt2:code>
 </skos:Concept>
 <skos:Concept rdf:about='urn:comp:1106'>
  <skos:prefLabel>Trend Analysis</skos:prefLabel>
  <skos:altLabel>TREND</skos:altLabel>
  <skos:broader rdf:resource='urn:comp:27'/>
  <skos:scopeNote>Knowledge, capabilities and practices associated with the
    identification of trends and patterns in data. Knowledge
    and demonstrated capability in statistical analysis
    including both classical and Bayesian statistics. Knowledge
    and demonstrated capability in using software packages for
    trend analysis, such as SPLUS, SYSTAT, or SAS. Knowledge
    and capabilities in data mining techniques and statistical
    learning approaches. Involves the ability to identify
    statistically significant time trends, patterns
    associations, outliers, and periodicities. Involves the
    capability to interpret the information provided by trends
    and patterns in terms of their program implications.
  </skos:scopeNote>
  <nt2:status>Approved</nt2:status>
  <nt2:type>Descriptor</nt2:type>
  <nt2:inputdate>2005-12-07</nt2:inputdate>
  <dcterms:dateAccepted>2005-12-07</dcterms:dateAccepted>
  <dcterms:modified>2006-12-18</dcterms:modified>
  <nt2:code>1106</nt2:code>
 </skos:Concept>
 <skos:Concept rdf:about='urn:comp:1042'>
  <skos:prefLabel>Instrumentation Systems</skos:prefLabel>
  <skos:altLabel>ELINSTR</skos:altLabel>
  <skos:broader rdf:resource='urn:comp:13'/>
  <skos:scopeNote>Knowledge, capabilities, and practices related to the
    design, development, characterization, and application of
    measurement and instrumentation systems used on space
    vehicles, flight payloads, experiments, ground test
    equipment, and test facilities. Ability to select and test
    appropriate measurement sensors for the various applications
    and integrate these sensors into larger subsystems.
    Includes knowledge of, and capability to perform, research
    and development of new, advanced and unique measuring
    sensors for both flight and ground instrumentation systems
    in the areas of temperature, pressure, vacuum, vibration,
    position, displacement, acceleration, mass spectroscopy,
    heat flux, flow, optical spectrometry and strain.
  </skos:scopeNote>
  <nt2:status>Approved</nt2:status>
  <nt2:type>Descriptor</nt2:type>
  <nt2:inputdate>2006-12-13</nt2:inputdate>
  <dcterms:modified>2006-12-13</dcterms:modified>
  <nt2:code>1042</nt2:code>
 </skos:Concept>
 <skos:Concept rdf:about='urn:comp:1112'>
  <skos:prefLabel>International Law</skos:prefLabel>
  <skos:altLabel>INTLLAW</skos:altLabel>
  <skos:broader rdf:resource='urn:comp:125'/>
  <skos:scopeNote>Knowledge of public international law, space law,
    international agreement drafting, conclusion, procedure and
    interpretation, international jurisprudence, Space Act
    Agreements, inter-agency procdedures concerning
    international agreements (C-175), negotiation skills and
    general knowledge concerning all other areas of law (e.g.,
    IP, ethics, contracts, environmental).
  </skos:scopeNote>
  <nt2:status>Approved</nt2:status>
  <nt2:type>Descriptor</nt2:type>
  <nt2:inputdate>2006-04-05</nt2:inputdate>
  <dcterms:dateAccepted>2006-04-05</dcterms:dateAccepted>
  <dcterms:modified>2006-12-18</dcterms:modified>
  <nt2:code>1112</nt2:code>
 </skos:Concept>
 <skos:Concept rdf:about='urn:comp:40'>
  <skos:prefLabel>Fundamental Human Factors Research</skos:prefLabel>
  <skos:altLabel>HUMFACTRES</skos:altLabel>
  <skos:broader rdf:resource='urn:comp:1244'/>
  <skos:narrower rdf:resource='urn:comp:1005'/>
  <skos:narrower rdf:resource='urn:comp:1010'/>
  <skos:narrower rdf:resource='urn:comp:1011'/>
  <skos:narrower rdf:resource='urn:comp:1012'/>
  <skos:narrower rdf:resource='urn:comp:1009'/>
  <skos:narrower rdf:resource='urn:comp:WQQ-302'/>
  <skos:narrower rdf:resource='urn:comp:WQQ-303'/>
  <skos:narrower rdf:resource='urn:comp:1018'/>
  <skos:narrower rdf:resource='urn:comp:1014'/>
  <skos:narrower rdf:resource='urn:comp:1015'/>
  <skos:narrower rdf:resource='urn:comp:1013'/>
  <skos:narrower rdf:resource='urn:comp:1007'/>
  <skos:narrower rdf:resource='urn:comp:1008'/>
  <skos:narrower rdf:resource='urn:comp:1016'/>
  <skos:narrower rdf:resource='urn:comp:1017'/>
  <skos:scopeNote>Knowledge of human engineering research methods (e.g.
    literature search, experiment, operational analysis,
    observation, survey, protection of research subjects) and
    activities (e.g., experimental design, planning data
    collection, data analysis, statistics, and documentation.
    Knowledge of the effects of environmental, individual,
    cognitive and organizational factors on the behavior and
    performance of humans, as well as the associated underlying
    physiological, psychological and social/organizational
    drivers that influence human behavior. Includes knowledge
    of a variety of psychophysical areas such as, but not
    limited to, biomechanics, perception, cognition,
    sensory-motor control, communication, decision-making, and
    teamwork and human-automation interaction. Ability to apply
    theories, experimentation, analysis and modeling to
    increase fundamental knowledge about human cognition and
    performance. Ability to develop human factors principles
    and guidelines which could be used toward designing
    technology for human performance in complex aerospace
    operational environments to reduce errors and increase
    productivity.
  </skos:scopeNote>
  <nt2:status>Approved</nt2:status>
  <nt2:type>Descriptor</nt2:type>
  <nt2:inputdate>2006-12-13</nt2:inputdate>
  <dcterms:modified>2006-12-13</dcterms:modified>
  <nt2:code>40</nt2:code>
 </skos:Concept>
 <skos:Concept rdf:about='urn:comp:108'>
  <skos:prefLabel>Air Traffic Systems</skos:prefLabel>
  <skos:altLabel>AIRTRAFFIC</skos:altLabel>
  <skos:broader rdf:resource='urn:comp:1237'/>
  <skos:scopeNote>Knowledge of Air Traffic Management elements, and their
    properties and interactions, such as air space and range
    systems, air traffic regulations, aircraft characteristics,
    airport structures and systems, and geographic and
    topographical patterns. Apply knowledge of these elements
    to the development of new systems and tools to improve the
    efficiency, effectiveness and capacity of the air traffic
    system, using advanced distributed modeling techniques to
    research and test concepts and prototypes.
  </skos:scopeNote>
  <nt2:status>Approved</nt2:status>
  <nt2:type>Descriptor</nt2:type>
  <nt2:inputdate>2006-12-13</nt2:inputdate>
  <dcterms:modified>2006-12-13</dcterms:modified>
  <nt2:code>108</nt2:code>
 </skos:Concept>
 <skos:Concept rdf:about='urn:comp:1016'>
  <skos:prefLabel>Supervisory Control Fundamental Research</skos:prefLabel>
  <skos:altLabel>HFRSUPCNTL</skos:altLabel>
  <skos:broader rdf:resource='urn:comp:40'/>
  <skos:scopeNote>TBD (includes single human operator supervisory control and
    distributed [multi-agent] supervisory control)
  </skos:scopeNote>
  <nt2:status>Approved</nt2:status>
  <nt2:type>Descriptor</nt2:type>
  <nt2:inputdate>2006-12-13</nt2:inputdate>
  <dcterms:modified>2006-12-13</dcterms:modified>
  <nt2:code>1016</nt2:code>
 </skos:Concept>
 <skos:Concept rdf:about='urn:comp:1063'>
  <skos:prefLabel>Contamination Control</skos:prefLabel>
  <skos:altLabel>MSECONTAM</skos:altLabel>
  <skos:broader rdf:resource='urn:comp:66'/>
  <skos:scopeNote>Knowledge capability and practices associated with the
    applications in materials, processes, contamination and
    foreign object debris (FOD) control requirements definition
    and insuring proper implementation through consulting,
    monitoring, testing and training services. Areas of
    responsibility include contamination control and foreign
    object debris (FOD) program development addressing both
    ground processing and on-orbit applications as applicable.
    Ground processing includes all areas from design, materials
    procurement, manufacturing, assembly, test, transportation,
    storage, launch site processing and any post flight
    refurbishment activities. Included are laboratory analysis
    and testing skills useful in ground processing materials
    and instrumentation applications for surface cleaning and
    cleanliness analysis/inspection. On-orbit applications
    include thermal vacuum environmental or space simulation
    testing. Material and process evaluations related to space
    simulation include material and component outgas testing,
    sensitive hardware bake-out certification, and ultraviolet
    enhanced contaminant deposition characterization.
  </skos:scopeNote>
  <nt2:status>Approved</nt2:status>
  <nt2:type>Descriptor</nt2:type>
  <nt2:inputdate>2006-12-13</nt2:inputdate>
  <dcterms:modified>2006-12-13</dcterms:modified>
  <nt2:code>1063</nt2:code>
 </skos:Concept>
 <skos:Concept rdf:about='urn:comp:1052'>
  <skos:prefLabel>Advanced Chemical &amp; Thermal Prop</skos:prefLabel>
  <skos:altLabel>APCHEM</skos:altLabel>
  <skos:broader rdf:resource='urn:comp:72'/>
  <skos:scopeNote>Research, development, design, testing and evaluation of
    propulsion system technologies which seek to increase the
    performance rockets in the space environment through novel
    means such as more energetic chemical propellants,
    ultralightweight propellant storage and management
    subsytems, high temperature system operation, heat addition
    to propellant by insolation concentration, etc.
  </skos:scopeNote>
  <nt2:status>Approved</nt2:status>
  <nt2:type>Descriptor</nt2:type>
  <nt2:inputdate>2006-12-13</nt2:inputdate>
  <dcterms:modified>2006-12-13</dcterms:modified>
  <nt2:code>1052</nt2:code>
 </skos:Concept>
 <skos:Concept rdf:about='urn:comp:154'>
  <skos:prefLabel>Configuration Management</skos:prefLabel>
  <skos:altLabel>CONFIGMMT</skos:altLabel>
  <skos:broader rdf:resource='urn:comp:1381'/>
  <skos:scopeNote>Knowledge of configuration management practices required to
    define, document, control and manage changes to the
    functional and physical attributes of system hardware,
    software, and information as applied to systems life cycle.
    Ability to control baselines, including identification
    (requirements, interfaces, and physical and functional
    attributes of configuration items) and control of changes
    to baseline. Knowledge of CM status accounting methods to
    record and report status of baselines. Capability to
    conduct audits of the overall configuration management
    processes performance, conduct Physical Configuration
    Audits, and support Functional Configuration Audits.
    Knowledge of NASA Program/Project management processes and
    the ability to plan, conduct, and evaluate the evolving
    baselines for NASA Programs/Projects in accordance with the
    NASA configuration management requirements and standards.
  </skos:scopeNote>
  <nt2:status>Approved</nt2:status>
  <nt2:type>Descriptor</nt2:type>
  <nt2:inputdate>2006-12-13</nt2:inputdate>
  <dcterms:modified>2006-12-13</dcterms:modified>
  <nt2:code>154</nt2:code>
 </skos:Concept>
 <skos:Concept rdf:about='urn:comp:20'>
  <skos:prefLabel>Sensors &amp; Data Acquisition</skos:prefLabel>
  <skos:altLabel>SENSORDATA</skos:altLabel>
  <skos:broader rdf:resource='urn:comp:1339'/>
  <skos:changeNote>???
  </skos:changeNote>
  <skos:scopeNote>Knowledge, capabilities and practices associated with
    sensors and data acquisition systems, particularly for use
    in flight vehicles, payloads and/or associated ground
    support equipment processes, such as propulsion system
    sensing or vehicle health management. This includes
    knowledge of sensing characteristics and properties, data
    acquisition and data processing characteristics and
    properties, and system unique requirements for the safe and
    effective implementation of sensors and data acquisition
    usage in aerospace and space systems.
  </skos:scopeNote>
  <nt2:status>Approved</nt2:status>
  <nt2:type>Descriptor</nt2:type>
  <nt2:inputdate>2006-12-13</nt2:inputdate>
  <dcterms:dateAccepted>2005-12-07</dcterms:dateAccepted>
  <dcterms:modified>2006-12-18</dcterms:modified>
  <nt2:code>20</nt2:code>
 </skos:Concept>
 <skos:Concept rdf:about='urn:comp:81'>
  <skos:prefLabel>Network Systems and Technology</skos:prefLabel>
  <skos:altLabel>NETSYS</skos:altLabel>
  <skos:broader rdf:resource='urn:comp:1283'/>
  <skos:scopeNote>Knowledge of how to research and implement high-speed wide
    area networks, including technology development to allow
    very advanced networks to allow data, audio and video
    communication. This includes electrical, optical and
    wireless transmission, telemetry and modeling, simulation
    of communication systems, and emulation of flight systems,
    sensors and data acquisition systems to function in an
    optimal fashion for distributed science and engineering
    applications. Involves technical skills used in the
    development and application of computer networks and
    Internet technology, including switching/routing
    technology, network architecture, and network security.
  </skos:scopeNote>
  <nt2:status>Approved</nt2:status>
  <nt2:type>Descriptor</nt2:type>
  <nt2:inputdate>2006-12-13</nt2:inputdate>
  <dcterms:modified>2006-12-13</dcterms:modified>
  <nt2:code>81</nt2:code>
 </skos:Concept>
 <skos:Concept rdf:about='urn:comp:70'>
  <skos:prefLabel>Hypersonic Airbreathing Propulsion</skos:prefLabel>
  <skos:altLabel>HAIRPRO</skos:altLabel>
  <skos:broader rdf:resource='urn:comp:1314'/>
  <skos:scopeNote>Knowledge of research and testing activities associated
    with hypersonic airbreathing propulsion flowpath and its
    integration with the vehicle concepts. Includes knowledge
    of the physics of high speed fuel-air mixing and
    combustion. Ability to plan, conduct, and interpret results
    of experimental and computational investigations to derive
    engine performance. Inherent within this competency is also
    the ability to design and develop engine components (inlet,
    combustor, and nozzle) and their interaction.
  </skos:scopeNote>
  <nt2:status>Approved</nt2:status>
  <nt2:type>Descriptor</nt2:type>
  <nt2:inputdate>2006-12-13</nt2:inputdate>
  <dcterms:modified>2006-12-13</dcterms:modified>
  <nt2:code>70</nt2:code>
 </skos:Concept>
 <skos:Concept rdf:about='urn:comp:90'>
  <skos:prefLabel>Aerospace Systems Concept Development &amp; Technology Assessment</skos:prefLabel>
  <skos:altLabel>ASCDTA</skos:altLabel>
  <skos:broader rdf:resource='urn:comp:1231'/>
  <skos:changeNote>???
  </skos:changeNote>
  <skos:scopeNote>Knowledge, capabilities and practices associated with the
    development of aerospace vehicle and spacecraft concepts
    from a systems perspective to satisfy prescribed mission
    architectures and identify enabling technologies for
    performance, cost, risk and safety. Knowledge of conceptual
    design, sizing &amp; synthesis of aerospace vehicles or
    spacecraft. Knowledge of elicitation from subject matter
    experts of the potential technology improvements from R&amp;D
    projects in all the relevant aerospace disciplines.
  </skos:scopeNote>
  <nt2:status>Approved</nt2:status>
  <nt2:type>Descriptor</nt2:type>
  <nt2:inputdate>2006-12-13</nt2:inputdate>
  <dcterms:dateAccepted>2005-12-07</dcterms:dateAccepted>
  <dcterms:modified>2006-12-18</dcterms:modified>
  <nt2:code>90</nt2:code>
 </skos:Concept>
 <skos:Concept rdf:about='urn:comp:76'>
  <skos:prefLabel>Power -Energy Storage</skos:prefLabel>
  <skos:altLabel>PWRENG</skos:altLabel>
  <skos:broader rdf:resource='urn:comp:1314'/>
  <skos:scopeNote>Knowledge, capabilities, and practices associated with the
    design, development, test, and evaluation of battery,
    flywheel, fuel cell, membrane technology and other
    electrical power storage components and systems.
  </skos:scopeNote>
  <nt2:status>Approved</nt2:status>
  <nt2:type>Descriptor</nt2:type>
  <nt2:inputdate>2006-12-13</nt2:inputdate>
  <dcterms:modified>2006-12-13</dcterms:modified>
  <nt2:code>76</nt2:code>
 </skos:Concept>
 <skos:Concept rdf:about='urn:comp:1394'>
  <skos:prefLabel>Management Competency Suite</skos:prefLabel>
  <skos:broader rdf:resource='urn:comp:1393'/>
  <skos:narrower rdf:resource='urn:comp:172'/>
  <skos:narrower rdf:resource='urn:comp:170'/>
  <skos:narrower rdf:resource='urn:comp:173'/>
  <skos:narrower rdf:resource='urn:comp:171'/>
  <nt2:status>Approved</nt2:status>
  <nt2:type>Descriptor</nt2:type>
  <nt2:inputdate>2006-12-13</nt2:inputdate>
  <dcterms:modified>2006-12-13</dcterms:modified>
  <nt2:code>1394</nt2:code>
 </skos:Concept>
 <skos:Concept rdf:about='urn:comp:89'>
  <skos:prefLabel>Advanced Mission Analysis</skos:prefLabel>
  <skos:altLabel>ADVMIS</skos:altLabel>
  <skos:broader rdf:resource='urn:comp:1231'/>
  <skos:changeNote>Modified for 6a by ???
  </skos:changeNote>
  <skos:scopeNote>Knowledge, capabilities, and practices associated with the
    conception, development, and planning of advanced mission
    architectures and systems synthesizing science, commercial,
    military and exploration requirements and considering
    feasibility, performance, cost, risk, schedule,
    reliability/safety and environmental effects.
  </skos:scopeNote>
  <nt2:status>Approved</nt2:status>
  <nt2:type>Descriptor</nt2:type>
  <nt2:inputdate>2006-12-13</nt2:inputdate>
  <dcterms:dateAccepted>2006-04-05</dcterms:dateAccepted>
  <dcterms:modified>2006-12-18</dcterms:modified>
  <nt2:code>89</nt2:code>
 </skos:Concept>
 <skos:Concept rdf:about='urn:comp:38'>
  <skos:prefLabel>Extravehicular Activity Systems</skos:prefLabel>
  <skos:altLabel>EAS</skos:altLabel>
  <skos:broader rdf:resource='urn:comp:1244'/>
  <skos:scopeNote>Knowledge of engineering, design, development, analysis and
    test of EVA systems. Requires knowledge and skills
    regarding the unique environment and constraints in sending
    a crewmember into space outside of a vehicle, and expertise
    in designing and developing spacesuits, tools, mechanisms,
    and operations that support such an activity. Includes
    knowledge of operational impacts and sustaining engineering
    on the system.
  </skos:scopeNote>
  <nt2:status>Approved</nt2:status>
  <nt2:type>Descriptor</nt2:type>
  <nt2:inputdate>2006-12-13</nt2:inputdate>
  <dcterms:modified>2006-12-13</dcterms:modified>
  <nt2:code>38</nt2:code>
 </skos:Concept>
 <skos:Concept rdf:about='urn:comp:144'>
  <skos:prefLabel>Export Control</skos:prefLabel>
  <skos:altLabel>EXPORT</skos:altLabel>
  <skos:broader rdf:resource='urn:comp:1125'/>
  <skos:scopeNote>Knowledge, capabilities, and practices associated with
    complying with federal laws controlling the export of items
    and technical data. This includes the formulation and
    implementation of export control policy, plans, and
    procedures that ensure compliance with federal law. The
    primary focus of export control it to ensure compliance
    through programs, education of the workforce, and
    addressing unique situations in the aerospace environment.
  </skos:scopeNote>
  <nt2:status>Approved</nt2:status>
  <nt2:type>Descriptor</nt2:type>
  <nt2:inputdate>2006-12-13</nt2:inputdate>
  <dcterms:modified>2006-12-13</dcterms:modified>
  <nt2:code>144</nt2:code>
 </skos:Concept>
 <skos:Concept rdf:about='urn:comp:10'>
  <skos:prefLabel>Test Engineering</skos:prefLabel>
  <skos:altLabel>TESTENG</skos:altLabel>
  <skos:broader rdf:resource='urn:comp:1209'/>
  <skos:narrower rdf:resource='urn:comp:1040'/>
  <skos:narrower rdf:resource='urn:comp:1038'/>
  <skos:narrower rdf:resource='urn:comp:1041'/>
  <skos:narrower rdf:resource='urn:comp:1037'/>
  <skos:narrower rdf:resource='urn:comp:1039'/>
  <skos:scopeNote>Knowledge of physics, engineering and manufacturing to test
    systems or subsystems under development for their
    functioning, efficacy and conformance to design
    requirements, or to test prototypes for feasibility. May
    involve ability to plan, conduct, and evaluate
    developmental, qualification, and acceptance testing in
    accordance with NASA, Military or Commercial Specifications
    of air, space and ground systems, components, piece parts,
    as well as integrated systems. Includes knowledge of
    environmental test techniques used to simulate loading
    conditions such as launch, reentry, orbit, and landing,
    including vibration, shock, acoustics, contamination,
    acceleration, electromagnetics, radiation, pressure,
    thermal, chemical, microgravity and solar vacuum,
    aerodynamics and temperature and humidity. Includes
    knowledge required for safe and reliable system
    development/integration.
  </skos:scopeNote>
  <nt2:status>Approved</nt2:status>
  <nt2:type>Descriptor</nt2:type>
  <nt2:inputdate>2006-12-13</nt2:inputdate>
  <dcterms:modified>2006-12-13</dcterms:modified>
  <nt2:code>10</nt2:code>
 </skos:Concept>
 <skos:Concept rdf:about='urn:comp:1098'>
  <skos:prefLabel>Facilities Operations and Maintenance</skos:prefLabel>
  <skos:altLabel>FACOPSMAIN</skos:altLabel>
  <skos:broader rdf:resource='urn:comp:112'/>
  <skos:scopeNote>Knowledge of operation and maintenance of office,
    operations and/or research facilities, and associated
    systems and
    equipment. Includes but is not limited to: knowledge
    required to develop and manage a comprehensive program of
    facilities management services, such as test planning and
    development, development of operational plans and
    procedures, data acquisition and analysis, test scheduling,
    resource planning, development of facility capability
    enhancements, reliability centered maintenance, energy
    conservation, system health monitoring, minor facility
    modification and repair, etc., to operate, sustain and
    optimize facilities and equipment. Includes the ability to
    effectively integrate these services to be consistent with
    the strategies and program goals of the organization.
  </skos:scopeNote>
  <nt2:status>Approved</nt2:status>
  <nt2:type>Descriptor</nt2:type>
  <nt2:inputdate>2006-12-13</nt2:inputdate>
  <dcterms:modified>2006-12-13</dcterms:modified>
  <nt2:code>1098</nt2:code>
 </skos:Concept>
 <skos:Concept rdf:about='urn:comp:151'>
  <skos:prefLabel>Emergency Management</skos:prefLabel>
  <skos:altLabel>EMERGMMT</skos:altLabel>
  <skos:broader rdf:resource='urn:comp:1159'/>
  <skos:scopeNote>Knowledge, capabilities, and practices of Comprehensive
    Emergency Management are associated with an integrated
    approach to the management of emergency programs and
    activities for all four emergency phases (mitigation,
    preparedness, response, and recovery), for all types of
    emergencies and disasters (natural, man-made, and attack),
    and for all NASA sites and centers, to include special
    National Level requests. Applies expert knowledge of the
    National Incident Management System, the National Response
    Plan, and Homeland Security Presidential Directives and
    other federal policies to enable effective emergency
    programs at the national, state, or local level as
    appropriate. Ability to
    NASA Competency Management SystemPage 21
    lead, coordinate, manage and direct the development and
    implementation of NASA’s and Federal emergency management
    policies, plans, and procedures for emergency response
    conditions, contingencies, continuity of operations,
    occupant emergency plans, and NASA’s interagency support
    functions in a full spectrum of emergencies. This
    competency includes the commitment to produce sound policy
    through requirements development that may affect lives,
    property, and operations in the event of unknown scenarios.
    Demonstrates the ability to: develop standards and
    specifications for new data analysis and data collection
    processes related to emergency preparedness; serve as an
    Aency, national level and industry-wide resource and has an
    established network to facilitate the acquisition of other
    resources and information; develop and/or modify safety
    procedures and requirements for related work and
    organization; maintain expert knowledge of applicable NASA,
    federal, aerospace and/or industry emergency preparedness
    trends, standards and policies; provide design concepts,
    risk management, trouble-shooting and trade-off analysis;
    technical expertise to represent Agency-wide, federal,
    industry and academic working groups, boards and panes;
    manage and provide comprehensive interpretation and
    equivalencies for all phases of emergency management;
    exhibit comprehensive knowledge of FEMA, OSHA and NASA
    standards pertaining to emergency management; represents
    agency in determining levels of coordination with
    intergovernmental departments, state and local agencies;
    evaluate agency exercise design criteria for emergency
    response; conduct risk assessments.
  </skos:scopeNote>
  <nt2:status>Approved</nt2:status>
  <nt2:type>Descriptor</nt2:type>
  <nt2:inputdate>2006-12-13</nt2:inputdate>
  <dcterms:modified>2006-12-13</dcterms:modified>
  <nt2:code>151</nt2:code>
 </skos:Concept>
 <skos:Concept rdf:about='urn:comp:19'>
  <skos:prefLabel>Flight and Ground Data Systems</skos:prefLabel>
  <skos:altLabel>FLTGNDSYS</skos:altLabel>
  <skos:broader rdf:resource='urn:comp:1294'/>
  <skos:scopeNote>Knowledge of controlling and monitoring systems for
    aerospace vehicles, payload flight systems and related
    ground equipment. Knowledge of processing techniques and
    requirements for housekeeping, health and status,
    operational and science data for spacecraft and science
    instruments. Includes knowledge of data acquisition,
    storage, distribution systems, as well as data analysis and
    troubleshooting techniques; special purpose analog/digital
    data handling and unique interface applications software.
    Assumes broad understanding of IT, electronics and
    communications disciplines and an ability to integrate the
    pieces together to optimize the design, integration and
    test of flight and ground hardware and software
  </skos:scopeNote>
  <nt2:status>Approved</nt2:status>
  <nt2:type>Descriptor</nt2:type>
  <nt2:inputdate>2006-12-13</nt2:inputdate>
  <dcterms:modified>2006-12-13</dcterms:modified>
  <nt2:code>19</nt2:code>
 </skos:Concept>
 <skos:Concept rdf:about='urn:comp:1005'>
  <skos:prefLabel>Biomechanics and Ergonomics Fundamental Research</skos:prefLabel>
  <skos:altLabel>HFRBIOMECH</skos:altLabel>
  <skos:broader rdf:resource='urn:comp:40'/>
  <skos:scopeNote>TBD
  </skos:scopeNote>
  <nt2:status>Approved</nt2:status>
  <nt2:type>Descriptor</nt2:type>
  <nt2:inputdate>2006-12-13</nt2:inputdate>
  <dcterms:modified>2006-12-13</dcterms:modified>
  <nt2:code>1005</nt2:code>
 </skos:Concept>
 <skos:Concept rdf:about='urn:comp:1012'>
  <skos:prefLabel>Decision Making and Risk Management Fundamental Research</skos:prefLabel>
  <skos:altLabel>HFRDECISMK</skos:altLabel>
  <skos:broader rdf:resource='urn:comp:40'/>
  <skos:scopeNote>TBD
  </skos:scopeNote>
  <nt2:status>Approved</nt2:status>
  <nt2:type>Descriptor</nt2:type>
  <nt2:inputdate>2006-12-13</nt2:inputdate>
  <dcterms:modified>2006-12-13</dcterms:modified>
  <nt2:code>1012</nt2:code>
 </skos:Concept>
 <skos:Concept rdf:about='urn:comp:54'>
  <skos:prefLabel>Astrobiology</skos:prefLabel>
  <skos:altLabel>ASTROBIO</skos:altLabel>
  <skos:broader rdf:resource='urn:comp:1407'/>
  <skos:scopeNote>Apply knowledge of biology, chemistry, physics, and other
    sciences in interdisciplinary experimental, observational,
    theoretical, and modeling studies of the origin, early
    development, and transmission of life in or on astronomical
    bodies and media, including the Earth and its atmosphere,
    and to determine how and where life arose and evolved on
    Earth and elsewhere, with due regard to environmental
    conditions and limits.
  </skos:scopeNote>
  <nt2:status>Approved</nt2:status>
  <nt2:type>Descriptor</nt2:type>
  <nt2:inputdate>2006-12-13</nt2:inputdate>
  <dcterms:modified>2006-12-13</dcterms:modified>
  <nt2:code>54</nt2:code>
 </skos:Concept>
 <skos:Concept rdf:about='urn:comp:1121'>
  <skos:prefLabel>Performance Management</skos:prefLabel>
  <skos:altLabel>HCMPERFMGT</skos:altLabel>
  <skos:broader rdf:resource='urn:comp:128'/>
  <skos:scopeNote>Knowledge of performance management concepts, principles,
    and practices related to planning, monitoring,
    rating,and rewarding employee performance.
  </skos:scopeNote>
  <nt2:status>Approved</nt2:status>
  <nt2:type>Descriptor</nt2:type>
  <nt2:inputdate>2006-04-05</nt2:inputdate>
  <dcterms:dateAccepted>2006-04-05</dcterms:dateAccepted>
  <dcterms:modified>2006-12-18</dcterms:modified>
  <nt2:code>1121</nt2:code>
 </skos:Concept>
 <skos:Concept rdf:about='urn:comp:85'>
  <skos:prefLabel>Intelligent/Adaptive Systems</skos:prefLabel>
  <skos:altLabel>IASYS</skos:altLabel>
  <skos:broader rdf:resource='urn:comp:1283'/>
  <skos:scopeNote>Knowledge of research and development techniques involving
    autonomous reasoning, human-centered computing and
    intelligent systems for data understanding towards mission
    requirements. Possesses knowledge of the practices
    associated with creating advanced intelligent,
    self-monitoring and adaptive computer science systems for
    use in development of aerospace vehicles (including
    unmanned systems), enhancement of aerospace flight safety
    and efficiency, and understanding of scientific data.
    Includes knowledge of modeling and simulation, techniques
    of artificial intelligence, virtual reality, automated
    software engineering, and collaborative and assistant
    systems, as well as understanding of vehicle health
    management.
  </skos:scopeNote>
  <nt2:status>Approved</nt2:status>
  <nt2:type>Descriptor</nt2:type>
  <nt2:inputdate>2006-12-13</nt2:inputdate>
  <dcterms:modified>2006-12-13</dcterms:modified>
  <nt2:code>85</nt2:code>
 </skos:Concept>
 <skos:Concept rdf:about='urn:comp:159'>
  <skos:prefLabel>Wireless Communications and Telemetry</skos:prefLabel>
  <skos:altLabel>WIRELESS</skos:altLabel>
  <skos:broader rdf:resource='urn:comp:1294'/>
  <skos:scopeNote>Knowledge, capabilities and practices associated with the
    design, analysis, development and/or test of microwave, RF
    electronic/Electromagnetic systems, particularly for use in
    flight vehicles, payloads or associated ground support
    equipment processes. Includes devices utilizing advanced
    technology for instrument (including data system) and
    communications (including telemetry) applications. Includes
    knowledge and capability in one or more of the following
    areas; RADAR, antenna systems for general electromagnetic
    components, communications systems for space, suborbital,
    aircraft, and ground applications, instrument systems (both
    active and passive), transmitting and receiving systems,
    transmission lines, electromagnetic propagation, data
    interleaving systems, navigational aids, atmospheric
    effects, multipath, scattering, Electromagnetic
    Interference, Compatibility and Effects (EMI/EMC/EME),
    modulation techniques, spectrum analysis, and non-ionizing
    radiation safety.`
  </skos:scopeNote>
  <nt2:status>Approved</nt2:status>
  <nt2:type>Descriptor</nt2:type>
  <nt2:inputdate>2006-12-13</nt2:inputdate>
  <dcterms:modified>2006-12-13</dcterms:modified>
  <nt2:code>159</nt2:code>
 </skos:Concept>
 <skos:Concept rdf:about='urn:comp:1008'>
  <skos:prefLabel>Psychophysiology Fundamental Research</skos:prefLabel>
  <skos:altLabel>HFRPSYPHY</skos:altLabel>
  <skos:broader rdf:resource='urn:comp:40'/>
  <skos:scopeNote>TBD (includes memory, attention, task processing, etc.)
  </skos:scopeNote>
  <nt2:status>Approved</nt2:status>
  <nt2:type>Descriptor</nt2:type>
  <nt2:inputdate>2006-12-13</nt2:inputdate>
  <dcterms:modified>2006-12-13</dcterms:modified>
  <nt2:code>1008</nt2:code>
 </skos:Concept>
 <skos:Concept rdf:about='urn:comp:1120'>
  <skos:prefLabel>Labor Relations</skos:prefLabel>
  <skos:altLabel>HCMLABOR</skos:altLabel>
  <skos:broader rdf:resource='urn:comp:128'/>
  <skos:scopeNote>Knowledge of laws, rules, regulations, case law,
    principles, and practices related to negotiating and
    administering
    labor agreements.
  </skos:scopeNote>
  <nt2:status>Approved</nt2:status>
  <nt2:type>Descriptor</nt2:type>
  <nt2:inputdate>2006-04-05</nt2:inputdate>
  <dcterms:dateAccepted>2006-04-05</dcterms:dateAccepted>
  <dcterms:modified>2006-12-18</dcterms:modified>
  <nt2:code>1120</nt2:code>
 </skos:Concept>
 <skos:Concept rdf:about='urn:comp:1294'>
  <skos:prefLabel>Electrical &amp; Electronic Competency Suite</skos:prefLabel>
  <skos:broader rdf:resource='urn:comp:1208'/>
  <skos:narrower rdf:resource='urn:comp:21'/>
  <skos:narrower rdf:resource='urn:comp:60'/>
  <skos:narrower rdf:resource='urn:comp:22'/>
  <skos:narrower rdf:resource='urn:comp:13'/>
  <skos:narrower rdf:resource='urn:comp:12'/>
  <skos:narrower rdf:resource='urn:comp:15'/>
  <skos:narrower rdf:resource='urn:comp:19'/>
  <skos:narrower rdf:resource='urn:comp:160'/>
  <skos:narrower rdf:resource='urn:comp:16'/>
  <skos:narrower rdf:resource='urn:comp:159'/>
  <nt2:status>Approved</nt2:status>
  <nt2:type>Descriptor</nt2:type>
  <nt2:inputdate>2006-12-13</nt2:inputdate>
  <dcterms:modified>2006-12-13</dcterms:modified>
  <nt2:code>1294</nt2:code>
 </skos:Concept>
 <skos:Concept rdf:about='urn:comp:1085'>
  <skos:prefLabel>Contracts Law</skos:prefLabel>
  <skos:altLabel>CONTRCTLAW</skos:altLabel>
  <skos:broader rdf:resource='urn:comp:125'/>
  <skos:changeNote>???
  </skos:changeNote>
  <skos:scopeNote>Speciaized knowledge of matters related to procurement,
    including but not limited to contracts, grants, cooperative
    agreements, Space Act agreements, source selections,
    claims, protests, and litigation and appeals related to
    procurement matters .
  </skos:scopeNote>
  <nt2:status>Approved</nt2:status>
  <nt2:type>Descriptor</nt2:type>
  <nt2:inputdate>2006-12-13</nt2:inputdate>
  <dcterms:dateAccepted>2006-04-05</dcterms:dateAccepted>
  <dcterms:modified>2006-12-18</dcterms:modified>
  <nt2:code>1085</nt2:code>
 </skos:Concept>
 <skos:Concept rdf:about='urn:comp:1041'>
  <skos:prefLabel>Propulsion Test Engineering</skos:prefLabel>
  <skos:altLabel>TSTPROPUL</skos:altLabel>
  <skos:broader rdf:resource='urn:comp:10'/>
  <skos:scopeNote>Knowledge, capabilities and practice associated with
    propulsion systems, subsystem, and/or component testing and
    cryogenic fluids as it relates to the functioning, efficacy
    and conformance to design requirements, or to test
    prototypes for feasibility or flight performance. Includes
    developing the procedures, methods, and techniques
    necessary to perform the test, to prepare, checkout, and
    assess the readiness of the test facility, and to ensure
    the safety of the systems or hardware. Includes full-scale
    or sub-scale testing of engine systems, subsystems, or
    components such as combustion chambers, nozzles,
    turbomachinery, ducts, valves, and pressurization systems.
    Includes knowledge of test techniques used to verify
    workmanship and validate operations in a relevant
    environment in accordance with NASA, Military or Commercial
    Specifications of air, space and ground systems,
    components, piece parts, as well as integrated propulsion
    systems or sub-systems.
  </skos:scopeNote>
  <nt2:status>Approved</nt2:status>
  <nt2:type>Descriptor</nt2:type>
  <nt2:inputdate>2006-12-13</nt2:inputdate>
  <dcterms:modified>2006-12-13</dcterms:modified>
  <nt2:code>1041</nt2:code>
 </skos:Concept>
 <skos:Concept rdf:about='urn:comp:1095'>
  <skos:prefLabel>Contract Management and Performance Assessment</skos:prefLabel>
  <skos:altLabel>CONPERFORM</skos:altLabel>
  <skos:broader rdf:resource='urn:comp:124'/>
  <skos:scopeNote>Knowledge and capabilities associated with managing
    contracts and evaluating a contractor's performance,
    including identifying and evaluating commercial and
    noncommercial financing arrangements, determining the
    appropriate actions necessary to ensure customer
    satisfaction, identifying and selecting the appropriate
    course of action for resolving a contractor dispute, and
    identifying and implementing contract close-out procedures.
  </skos:scopeNote>
  <nt2:status>Approved</nt2:status>
  <nt2:type>Descriptor</nt2:type>
  <nt2:inputdate>2006-12-13</nt2:inputdate>
  <dcterms:modified>2006-12-13</dcterms:modified>
  <nt2:code>1095</nt2:code>
 </skos:Concept>
 <skos:Concept rdf:about='urn:comp:1061'>
  <skos:prefLabel>Non-metallics</skos:prefLabel>
  <skos:altLabel>MSENONMET</skos:altLabel>
  <skos:broader rdf:resource='urn:comp:66'/>
  <skos:scopeNote>Knowledge capability and practices associated with research
    into the production, characteristics, structure,
    properties, and performance of non-metallic materials,
    including organic and inorganic polymeric materials, fiber
    and resin systems, as well as the design, development,
    processing and testing of those non-metals within aerospace
    structures such as flight systems, ground support and
    facility systems. Includes assessment of the durability and
    response of non-metallic materials to environmental
    conditions, composition, manufacturing processes and
    applied forces. Includes broad knowledge of the
    non-metallic materials engineering discipline, including
    characteristics of non-metal types such as ceramics,
    glasses, polymers, composites, thermal insulation, polymer
    and ceramic matrix
    composites as well as methods of processing into final
    products. Also includes broad capabilities in analysis,
    evaluation and testing of non-metallics including the
    analysis of the nature, behavior, and physical
    characteristics of non-metals and their constituents,
    including the mechanisms and effects by which materials
    react to stresses, environments, and processes.
  </skos:scopeNote>
  <nt2:status>Approved</nt2:status>
  <nt2:type>Descriptor</nt2:type>
  <nt2:inputdate>2006-12-13</nt2:inputdate>
  <dcterms:modified>2006-12-13</dcterms:modified>
  <nt2:code>1061</nt2:code>
 </skos:Concept>
 <skos:Concept rdf:about='urn:comp:166'>
  <skos:prefLabel>Imaging Analysis</skos:prefLabel>
  <skos:altLabel>IMAGING</skos:altLabel>
  <skos:broader rdf:resource='urn:comp:1283'/>
  <skos:scopeNote>This competency referes to the knowledge and capabilities
    associated with the analysis of all imaging media to
    include film, motion picture and video in both visible and
    non-visible spectra. Includes using digital imagery
    manipulation techniques such as frame averaging, motion
    stabilization, point tracking, etc. to obtain specific data
    from the images such as object size, orientation,
    trajectory, and velocity. Requires detailed understanding
    of the cameras and photographic and digital processes used
    to obtain the imagery. The analysis supports vehicle
    preparation, launch, on orbit, in-flight, landing,
    terestrial, extratrestrial and planetary study as well as
    other areas of imaging. This competency supports
    exploration, research and operations from basic scientific
    knowledge through flight safety.
  </skos:scopeNote>
  <nt2:status>Approved</nt2:status>
  <nt2:type>Descriptor</nt2:type>
  <nt2:inputdate>2006-12-13</nt2:inputdate>
  <dcterms:modified>2006-12-13</dcterms:modified>
  <nt2:code>166</nt2:code>
 </skos:Concept>
 <skos:Concept rdf:about='urn:comp:26'>
  <skos:prefLabel>Cryogenics Engineering</skos:prefLabel>
  <skos:altLabel>CRYOENG</skos:altLabel>
  <skos:broader rdf:resource='urn:comp:1359'/>
  <skos:scopeNote>Knowledge, capabilities and practices associated with
    aerospace cryogenic systems, particularly for use in
    propulsion, life support, refrigeration and laboratory
    processes. This includes handling characteristics, material
    properties, system safety, and system unique requirements
    for the safe and effective usage of cryogenic fluids for
    research, development, design, analysis, test, operation
    and/or evaluation of cryogenic fluids storage and transfer
    systems for both fuels and oxidizers.
  </skos:scopeNote>
  <nt2:status>Approved</nt2:status>
  <nt2:type>Descriptor</nt2:type>
  <nt2:inputdate>2006-12-13</nt2:inputdate>
  <dcterms:modified>2006-12-13</dcterms:modified>
  <nt2:code>26</nt2:code>
 </skos:Concept>
 <skos:Concept rdf:about='urn:comp:9'>
  <skos:prefLabel>Integration Engineering</skos:prefLabel>
  <skos:altLabel>INTEGENG</skos:altLabel>
  <skos:broader rdf:resource='urn:comp:1209'/>
  <skos:narrower rdf:resource='urn:comp:1035'/>
  <skos:narrower rdf:resource='urn:comp:1033'/>
  <skos:narrower rdf:resource='urn:comp:1036'/>
  <skos:narrower rdf:resource='urn:comp:1032'/>
  <skos:narrower rdf:resource='urn:comp:1034'/>
  <skos:scopeNote>Knowledge and capability to integrate all elements into a
    functioning system or subsystem such as complex flight to
    flight and flight to ground and facilities systems.
    Includes knowledge and capabilities required for safe and
    reliable integration of different elements of a system,
    schedules, configurations and resources as well as the
    development of launch, mission, manifest, contigency and
    long-range plans and responses to externally-driven
    requirements.
  </skos:scopeNote>
  <nt2:status>Approved</nt2:status>
  <nt2:type>Descriptor</nt2:type>
  <nt2:inputdate>2006-12-13</nt2:inputdate>
  <dcterms:modified>2006-12-13</dcterms:modified>
  <nt2:code>9</nt2:code>
 </skos:Concept>
 <skos:Concept rdf:about='urn:comp:136'>
  <skos:prefLabel>Governmental Affairs</skos:prefLabel>
  <skos:altLabel>GOVAF</skos:altLabel>
  <skos:broader rdf:resource='urn:comp:1125'/>
  <skos:scopeNote>Knowledge of NASA-related legislation, the legislative
    process and public affairs as it pertains to NASA. Includes
    the ability to monitor legislation that is of interest to
    NASA, monitor NASA-related hearings and markups scheduled
    before the House and Senate committees and subcommittees
    that have oversight over NASA, to especially include
    Authorization and Appropriations subcommittees. Ability to
    help manage NASA press releases of Congressional interest
    and identify key members and issues of importance to them.
    Broad knowledge of NASA programs and specific knowledge of
    local center programs.
  </skos:scopeNote>
  <nt2:status>Approved</nt2:status>
  <nt2:type>Descriptor</nt2:type>
  <nt2:inputdate>2006-12-13</nt2:inputdate>
  <dcterms:modified>2006-12-13</dcterms:modified>
  <nt2:code>136</nt2:code>
 </skos:Concept>
 <skos:Concept rdf:about='urn:comp:120'>
  <skos:prefLabel>Internal Control / Audit</skos:prefLabel>
  <skos:altLabel>INTAUD</skos:altLabel>
  <skos:broader rdf:resource='urn:comp:1150'/>
  <skos:scopeNote>Knowledge of how to evaluate control systems for financial,
    administrative, program, and operational activities to
    provide reasonable assurances that obligations, costs and
    disbursements comply with applicable regulations and laws,
    that property is funded, and assets are safeguarded; and
    that revenues and expenditures applicable to operations are
    properly recorded and accounted for. Involves ability to
    conduct surveys, studies and other investigations for
    management operations or related processes to assess and
    report adequacy, validity and compliance/non-compliance to
    requirements. Ability to communicate derived audit
    assessment and recommend, establish, modify and/or
    implement internal controls to mitigate findings.
  </skos:scopeNote>
  <nt2:status>Approved</nt2:status>
  <nt2:type>Descriptor</nt2:type>
  <nt2:inputdate>2006-12-13</nt2:inputdate>
  <dcterms:modified>2006-12-13</dcterms:modified>
  <nt2:code>120</nt2:code>
 </skos:Concept>
 <skos:Concept rdf:about='urn:comp:1037'>
  <skos:prefLabel>Structural Test Engineering</skos:prefLabel>
  <skos:altLabel>TSTSTRUCT</skos:altLabel>
  <skos:broader rdf:resource='urn:comp:10'/>
  <skos:scopeNote>Knowledge of physics, engineering, and manufacturing to
    test structural systems, subsystems, and components that
    verify the functioning, efficacy, and conformance to deign
    requirements of these structures. This activity involves
    the planning, conduct, and evaluation of results for
    structural system development, qualification, or acceptance
    tests in accordance with NASA, military or commercial
    specifications. It includes the knowledge of structural
    test techniques to simulate loading conditions for
    structural systems experiencing launch, on-orbit, re-entry
    or landing environments and the associated response
    measurement methods to verify or correlate the structural
    system’s analytical models. Test discipline skills
    associated with this competency include: vibration;
    acoustics; shock; static structural loads; and modal
    analysis.
  </skos:scopeNote>
  <nt2:status>Approved</nt2:status>
  <nt2:type>Descriptor</nt2:type>
  <nt2:inputdate>2006-12-13</nt2:inputdate>
  <dcterms:modified>2006-12-13</dcterms:modified>
  <nt2:code>1037</nt2:code>
 </skos:Concept>
 <skos:Concept rdf:about='urn:comp:1125'>
  <skos:prefLabel>Business Operations Competency Suite</skos:prefLabel>
  <skos:broader rdf:resource='urn:comp:1124'/>
  <skos:narrower rdf:resource='urn:comp:131'/>
  <skos:narrower rdf:resource='urn:comp:113'/>
  <skos:narrower rdf:resource='urn:comp:117'/>
  <skos:narrower rdf:resource='urn:comp:137'/>
  <skos:narrower rdf:resource='urn:comp:144'/>
  <skos:narrower rdf:resource='urn:comp:136'/>
  <skos:narrower rdf:resource='urn:comp:127'/>
  <skos:narrower rdf:resource='urn:comp:157'/>
  <skos:narrower rdf:resource='urn:comp:125'/>
  <skos:narrower rdf:resource='urn:comp:176'/>
  <skos:narrower rdf:resource='urn:comp:116'/>
  <skos:narrower rdf:resource='urn:comp:169'/>
  <skos:narrower rdf:resource='urn:comp:135'/>
  <nt2:status>Approved</nt2:status>
  <nt2:type>Descriptor</nt2:type>
  <nt2:inputdate>2006-12-13</nt2:inputdate>
  <dcterms:modified>2006-12-13</dcterms:modified>
  <nt2:code>1125</nt2:code>
 </skos:Concept>
 <skos:Concept rdf:about='urn:comp:1066'>
  <skos:prefLabel>Occupational Medicine</skos:prefLabel>
  <skos:altLabel>OCCMED</skos:altLabel>
  <skos:broader rdf:resource='urn:comp:130'/>
  <skos:scopeNote>Professional skills and knowledge to apply occupational
    health related requirements to protect and maintain
    workers’ physical and mental health. Knowledge to apply and
    initiate preventive health and wellness measures to reduce
    work-related illnesses and injuries. Knowledge and
    experience to manage implement and evaluate occupational
    medicine program areas. This includes clinical case
    management, health surveillance, and emergency medical
    response.
  </skos:scopeNote>
  <nt2:status>Approved</nt2:status>
  <nt2:type>Descriptor</nt2:type>
  <nt2:inputdate>2006-12-13</nt2:inputdate>
  <dcterms:modified>2006-12-13</dcterms:modified>
  <nt2:code>1066</nt2:code>
 </skos:Concept>
 <skos:Concept rdf:about='urn:comp:1122'>
  <skos:prefLabel>Recruitment/Placement</skos:prefLabel>
  <skos:altLabel>HCMRECRUIT</skos:altLabel>
  <skos:broader rdf:resource='urn:comp:128'/>
  <skos:scopeNote>Knowledge of HR concepts, principles,and practices related
    to identifying, attracting, and selecting individuals and
    placing them into positions to address changing
    organizational needs.
  </skos:scopeNote>
  <nt2:status>Approved</nt2:status>
  <nt2:type>Descriptor</nt2:type>
  <nt2:inputdate>2006-04-05</nt2:inputdate>
  <dcterms:dateAccepted>2006-04-05</dcterms:dateAccepted>
  <dcterms:modified>2006-12-18</dcterms:modified>
  <nt2:code>1122</nt2:code>
 </skos:Concept>
 <skos:Concept rdf:about='urn:comp:1415'>
  <skos:prefLabel>Earth Sciences Competency Suite</skos:prefLabel>
  <skos:broader rdf:resource='urn:comp:1406'/>
  <skos:narrower rdf:resource='urn:comp:46'/>
  <skos:narrower rdf:resource='urn:comp:164'/>
  <skos:narrower rdf:resource='urn:comp:49'/>
  <skos:narrower rdf:resource='urn:comp:50'/>
  <skos:narrower rdf:resource='urn:comp:45'/>
  <skos:narrower rdf:resource='urn:comp:88'/>
  <skos:narrower rdf:resource='urn:comp:47'/>
  <skos:narrower rdf:resource='urn:comp:48'/>
  <nt2:status>Approved</nt2:status>
  <nt2:type>Descriptor</nt2:type>
  <nt2:inputdate>2006-12-13</nt2:inputdate>
  <dcterms:modified>2006-12-13</dcterms:modified>
  <nt2:code>1415</nt2:code>
 </skos:Concept>
 <skos:Concept rdf:about='urn:comp:1074'>
  <skos:prefLabel>Information Security</skos:prefLabel>
  <skos:altLabel>SECINFO</skos:altLabel>
  <skos:broader rdf:resource='urn:comp:126'/>
  <skos:scopeNote>Knowledge, capabilities and practices associated with the
    protection of national classified information and sensitive
    but unclassified (SBU) information including;
    classification, declassification, and protection of
    classified national defense information originated or
    controlled by Federal agencies in accordance with Executive
    Order 12958, April 17, 1995, "Classified National Security
    Information,"
  </skos:scopeNote>
  <nt2:status>Approved</nt2:status>
  <nt2:type>Descriptor</nt2:type>
  <nt2:inputdate>2006-12-13</nt2:inputdate>
  <dcterms:modified>2006-12-13</dcterms:modified>
  <nt2:code>1074</nt2:code>
 </skos:Concept>
 <skos:Concept rdf:about='urn:comp:1030'>
  <skos:prefLabel>Propulsion Design and Development Engineering</skos:prefLabel>
  <skos:altLabel>DDEPROP</skos:altLabel>
  <skos:broader rdf:resource='urn:comp:8'/>
  <skos:scopeNote>Knowledge, capabilities and practices associated with the
    detailed mechanical design of propulsion components,
    subsystems and systems. Includes expertise required for
    safe and reliable component and system design, development,
    and integration. Competency assumes a breadth of knowledge
    of many specialty areas such as
    geometric dimensioning and tolerancing, cutting edge
    computer aided design and modeling tools, state of the art
    manufacturing and fabrication processes, specialty hardware
    and fasteners, bolted joint design, fits and interfaces,
    technical specifications, instructions and procedures,
    engine systems design, functional design, and design for
    optimization of component performance in relation to
    mission environments through testing. Also, depth in
    familiarization with system engineering tools, procedures,
    and documentation such as configuration management, the
    design review process, interface control documents, and
    interface requirements documents.
  </skos:scopeNote>
  <nt2:status>Approved</nt2:status>
  <nt2:type>Descriptor</nt2:type>
  <nt2:inputdate>2006-12-13</nt2:inputdate>
  <dcterms:modified>2006-12-13</dcterms:modified>
  <nt2:code>1030</nt2:code>
 </skos:Concept>
 <skos:Concept rdf:about='urn:comp:86'>
  <skos:prefLabel>Mathematical Modeling &amp; Analysis</skos:prefLabel>
  <skos:altLabel>MMA</skos:altLabel>
  <skos:broader rdf:resource='urn:comp:1363'/>
  <skos:scopeNote>Knowledge, capabilities and practices associated with
    mathematical modeling, the design of algorithms and applied
    computational methods, simulation and analysis of physical
    systems to represent structural, fluid, thermal, dynamic,
    chemical, or other real phenomena in a quantifiable manner.
    This includes using manual calculations and computer
    simulation software. Models can refer to launch vehicle,
    spacecraft, ground support equipment, handling equipment,
    and facility/flight interface hardware related physical
    systems design of algorithms and applied computational
    methods. This includes capability in the area of quantum
    computing. Understanding of the physical principle
    represented in the model is essential to this competency.
  </skos:scopeNote>
  <nt2:status>Approved</nt2:status>
  <nt2:type>Descriptor</nt2:type>
  <nt2:inputdate>2006-12-13</nt2:inputdate>
  <dcterms:modified>2006-12-13</dcterms:modified>
  <nt2:code>86</nt2:code>
 </skos:Concept>
 <skos:Concept rdf:about='urn:comp:107'>
  <skos:prefLabel>Icing Physics</skos:prefLabel>
  <skos:altLabel>ICEPHYSICS</skos:altLabel>
  <skos:broader rdf:resource='urn:comp:1424'/>
  <skos:scopeNote>Knowledge, capabilities and practices associated with
    researching and understanding icing physics analysis and
    testing, atmospheric science, and ice sensing and
    protection methods.
  </skos:scopeNote>
  <nt2:status>Approved</nt2:status>
  <nt2:type>Descriptor</nt2:type>
  <nt2:inputdate>2006-12-13</nt2:inputdate>
  <dcterms:modified>2006-12-13</dcterms:modified>
  <nt2:code>107</nt2:code>
 </skos:Concept>
 <skos:Concept rdf:about='urn:comp:25'>
  <skos:prefLabel>Chemistry/ Chemical Engineering</skos:prefLabel>
  <skos:altLabel>CHEMENG</skos:altLabel>
  <skos:broader rdf:resource='urn:comp:1280'/>
  <skos:scopeNote>Knowledge, capabilities and practices associated with
    Chemistry and Chemical Engineering as applied to aerospace
    systems for ground and flight application, particularly for
    use in sensors, material sciences, propulsion,
    environmental,
    NASA Competency Management SystemPage 37
    ecological, biological or laboratory processes. This
    includes an understanding of organic, inorganic, analytical
    and physical chemistry and their application to a wide
    variety of research, development, failure analysis, and
    operational systems or topics and/or principles and
    practices of chemical engineering.
  </skos:scopeNote>
  <nt2:status>Approved</nt2:status>
  <nt2:type>Descriptor</nt2:type>
  <nt2:inputdate>2006-12-13</nt2:inputdate>
  <dcterms:modified>2006-12-13</dcterms:modified>
  <nt2:code>25</nt2:code>
 </skos:Concept>
 <skos:Concept rdf:about='urn:comp:101'>
  <skos:prefLabel>Aerodynamics</skos:prefLabel>
  <skos:altLabel>AERODYN</skos:altLabel>
  <skos:broader rdf:resource='urn:comp:1237'/>
  <skos:changeNote>???
  </skos:changeNote>
  <skos:scopeNote>Knowledge of the science of aerodynamics, with the ability
    to plan, conduct, interpret and correlate results of
    experimental investigations, analytical methods and
    numerical simulations with varying degree of fidelity such
    as computational fluid dynamics (CFD) analyses for the
    design of aerospace vehicles and components, which include
    commercial and military aircraft, space transportation
    systems and launch vehicles, and the prediction of their
    aerodynamic performance from subsonic to hypersonic Mach
    numbers, including incompressible flows, and over wide
    range of Reynolds numbers and flight conditions. Includes
    knowledge, capabilities and practices associated with fluid
    dynamics and flow physics modeling in specialized areas
    such as external and internal flows, analytical and CFD
    prediction methods, wind tunnel model and flight testing
    techniques, unsteady and high angle-of-attack flow
    phenomena, propulsion system-airframe integration, rotary
    wing aerodynamics, cavity flows, etc., for a realistic
    assessment and improvement of the vehicle aerodynamic
    performance.
  </skos:scopeNote>
  <nt2:status>Approved</nt2:status>
  <nt2:type>Descriptor</nt2:type>
  <nt2:inputdate>2006-12-13</nt2:inputdate>
  <dcterms:dateAccepted>2005-12-07</dcterms:dateAccepted>
  <dcterms:modified>2006-12-18</dcterms:modified>
  <nt2:code>101</nt2:code>
 </skos:Concept>
 <skos:Concept rdf:about='urn:comp:1381'>
  <skos:prefLabel>Quality/Safety/Performance Competency Suite</skos:prefLabel>
  <skos:broader rdf:resource='urn:comp:1371'/>
  <skos:narrower rdf:resource='urn:comp:154'/>
  <skos:narrower rdf:resource='urn:comp:149'/>
  <skos:narrower rdf:resource='urn:comp:29'/>
  <skos:narrower rdf:resource='urn:comp:28'/>
  <skos:narrower rdf:resource='urn:comp:123'/>
  <skos:narrower rdf:resource='urn:comp:27'/>
  <skos:narrower rdf:resource='urn:comp:139'/>
  <nt2:status>Approved</nt2:status>
  <nt2:type>Descriptor</nt2:type>
  <nt2:inputdate>2006-12-13</nt2:inputdate>
  <dcterms:modified>2006-12-13</dcterms:modified>
  <nt2:code>1381</nt2:code>
 </skos:Concept>
 <skos:Concept rdf:about='urn:comp:122'>
  <skos:prefLabel>Program/Project Management</skos:prefLabel>
  <skos:altLabel>PROJPROGMT</skos:altLabel>
  <skos:broader rdf:resource='urn:comp:1399'/>
  <skos:scopeNote>Knowledge, capabilities and practices associated with
    formulating, planning, implementing, managing, tracking and
    evaluating work and its associated requirements and risks,
    ranging from one-time projects to program-level work.
    Critical abilities are to define customer and stakeholder
    needs and constraints, reduce ambiguity in objectives,
    develop and manage an efficient project organizational
    structure, and apply system architecture principles to
    develop and manage technical requirements in order to
    achieve the appropriate balance between resources,
    schedule, and technical requirements. Includes knowledge
    associated with system architecture, finance, budgeting,
    risk assessment, schedule, configuration management,
    contract technical management, and project controls.
  </skos:scopeNote>
  <nt2:status>Approved</nt2:status>
  <nt2:type>Descriptor</nt2:type>
  <nt2:inputdate>2006-12-13</nt2:inputdate>
  <dcterms:modified>2006-12-13</dcterms:modified>
  <nt2:code>122</nt2:code>
 </skos:Concept>
 <skos:Concept rdf:about='urn:comp:30'>
  <skos:prefLabel>Mission Assurance</skos:prefLabel>
  <skos:altLabel>MA</skos:altLabel>
  <skos:broader rdf:resource='urn:comp:1372'/>
  <skos:scopeNote>Knowledge of methodologies and practices such as risk
    identification, analysis, planning, tracking and control
    (e.g., Certificate of Flight Readiness process, product
    management process) used to achieve mission, product or
    process
    success. Activities include independent verification of
    product design requirements, testing validation, critical
    inspections, facility evaluations, flight safety analysis,
    development of recommendations, and tracking corrective
    actions.
  </skos:scopeNote>
  <nt2:status>Approved</nt2:status>
  <nt2:type>Descriptor</nt2:type>
  <nt2:inputdate>2006-12-13</nt2:inputdate>
  <dcterms:modified>2006-12-13</dcterms:modified>
  <nt2:code>30</nt2:code>
 </skos:Concept>
 <skos:Concept rdf:about='urn:comp:1123'>
  <skos:prefLabel>Workforce Planning</skos:prefLabel>
  <skos:altLabel>HCMWORKPLN</skos:altLabel>
  <skos:broader rdf:resource='urn:comp:128'/>
  <skos:scopeNote>Knowledge of HR concepts, principles, and practices related
    to determining workload projections and current and
    future competency gaps to align human capital with
    organizational goals.
  </skos:scopeNote>
  <nt2:status>Approved</nt2:status>
  <nt2:type>Descriptor</nt2:type>
  <nt2:inputdate>2006-04-04</nt2:inputdate>
  <dcterms:dateAccepted>2006-04-05</dcterms:dateAccepted>
  <dcterms:modified>2006-12-18</dcterms:modified>
  <nt2:code>1123</nt2:code>
 </skos:Concept>
 <skos:Concept rdf:about='urn:comp:1004'>
  <skos:prefLabel>International Relations</skos:prefLabel>
  <skos:altLabel>LEADGLOBAL</skos:altLabel>
  <skos:broader rdf:resource='urn:comp:140'/>
  <skos:scopeNote>Knowledge, capabilities and practices associated with
    forming and maintaining cross-cultural relationships and
    international partnerships and alliances. Understanding of
    the rules and policies that regulate or dictate
    international partnerships and how to work within those
    guidelines in order to accomplish objectives and sustain
    ongoing relationships.
  </skos:scopeNote>
  <nt2:status>Approved</nt2:status>
  <nt2:type>Descriptor</nt2:type>
  <nt2:inputdate>2006-12-13</nt2:inputdate>
  <dcterms:modified>2006-12-13</dcterms:modified>
  <nt2:code>1004</nt2:code>
 </skos:Concept>
 <skos:Concept rdf:about='urn:comp:8'>
  <skos:prefLabel>Design and Development Engineering</skos:prefLabel>
  <skos:altLabel>DESDEVENG</skos:altLabel>
  <skos:broader rdf:resource='urn:comp:1209'/>
  <skos:narrower rdf:resource='urn:comp:1029'/>
  <skos:narrower rdf:resource='urn:comp:1030'/>
  <skos:narrower rdf:resource='urn:comp:1028'/>
  <skos:narrower rdf:resource='urn:comp:1031'/>
  <skos:scopeNote>Knowledge, capabilities and practices associated with all
    aspects of the technical design and development process
    including the development of flight hardware, payloads,
    technology projects fabrication processes and techniques,
    concurrent engineering, production assessment, and process
    verification as applied to aerospace vehicles and systems
    used in atmospheric and space environments. Includes
    ability to create models and prototypes, particularly in a
    laboratory setting, based on research oriented plans and
    schematics and capability to design the system for safe and
    reliable development, integration and manufacturability.
  </skos:scopeNote>
  <nt2:status>Approved</nt2:status>
  <nt2:type>Descriptor</nt2:type>
  <nt2:inputdate>2006-12-13</nt2:inputdate>
  <dcterms:modified>2006-12-13</dcterms:modified>
  <nt2:code>8</nt2:code>
 </skos:Concept>
 <skos:Concept rdf:about='urn:comp:1062'>
  <skos:prefLabel>Failure Analysis</skos:prefLabel>
  <skos:altLabel>MSEFAILURE</skos:altLabel>
  <skos:broader rdf:resource='urn:comp:66'/>
  <skos:scopeNote>Knowledge capability and practices associated with research
    into the characteristics and performance of materials and
    the design, development and testing of those materials
    within aerospace structures such as flight systems, ground
    support and facility systems, and investigation and
    evaluation of failed materials and surfaces to determine
    the root causes of failure. Includes the capability to
    analyze, plan, and execute failure analysis for a component
    fabricated of a structural material, identify failure modes
    and recommend improvements to resolve original problem
    (e.g., redesign component, which may include fabricating it
    from a more resistant material). Examines failures by
    evaluating metallurgical cross sections, plus application
    of the full range of etching techniques in addition to the
    traditional techniques based on reflected light microscopy,
    and also use a broad range of non-destructive testing
    techniques and a full range of mechanical testing equipment
    to quantify the failure modes and rates. Includes knowledge
    and practices in operation of electro-optical and
    diagnostic equipment (such as scanning electron microscopy,
    TEM, ESCA, OLM, SIMS, energy-dispersive x-ray, computerized
    radiography and Auger microprobe spectroscopy, etc.) to
    augment observations made metallographically to detect or
    confirm chemical contributions to failure mechanism
    composition, examine fractures or crack-like defects, and
    to analyze hardness, grain size, surface chemistry of the
    first few atomic layers, as well as bulk microstructural
    features. Includes the development of math models for
    assessment of material durability and response to
    environmental conditions and contaminants. Includes broad
    knowledge of materials disciplines, including material
    types such as ceramics, metallics, composites and polymers
    as well as tribology or surface science.
  </skos:scopeNote>
  <nt2:status>Approved</nt2:status>
  <nt2:type>Descriptor</nt2:type>
  <nt2:inputdate>2006-12-13</nt2:inputdate>
  <dcterms:modified>2006-12-13</dcterms:modified>
  <nt2:code>1062</nt2:code>
 </skos:Concept>
 <skos:Concept rdf:about='urn:comp:104'>
  <skos:prefLabel>Thermal Systems</skos:prefLabel>
  <skos:altLabel>THERMALSYS</skos:altLabel>
  <skos:broader rdf:resource='urn:comp:1359'/>
  <skos:scopeNote>Knowledge, capabilities and practices associated with heat
    transfer, fluid flow, and thermodynamics in the design,
    development, testing, integration and evaluation of passive
    and active thermal control systems for spacecraft,
    propulsion systems, instruments, experiments, sensors,
    aircraft, ground systems, thermal protection systems and
    facility systems. Includes knowledge and practices in the
    development of advanced thermal hardware and thermal
    technology for future spacecraft, propulsion systems,
    instrument, and sensor applications including heat pipes,
    two-phase heat transfer systems, cryogenic systems,
    advanced coatings, and heat pumps. Includes knowledge of
    the development of math models for low and high speed
    convection, conduction, radiation, ablation and aeroheating.
  </skos:scopeNote>
  <nt2:status>Approved</nt2:status>
  <nt2:type>Descriptor</nt2:type>
  <nt2:inputdate>2006-12-13</nt2:inputdate>
  <dcterms:modified>2006-12-13</dcterms:modified>
  <nt2:code>104</nt2:code>
 </skos:Concept>
 <skos:Concept rdf:about='urn:comp:78'>
  <skos:prefLabel>Power Generation -Thermal Systems</skos:prefLabel>
  <skos:altLabel>PWRTHM</skos:altLabel>
  <skos:broader rdf:resource='urn:comp:1314'/>
  <skos:scopeNote>Design development, test, and evaluation of dynamic power
    systems including thermal and solar dynamic systems.
  </skos:scopeNote>
  <nt2:status>Approved</nt2:status>
  <nt2:type>Descriptor</nt2:type>
  <nt2:inputdate>2006-12-13</nt2:inputdate>
  <dcterms:modified>2006-12-13</dcterms:modified>
  <nt2:code>78</nt2:code>
 </skos:Concept>
 <skos:Concept rdf:about='urn:comp:105'>
  <skos:prefLabel>Thermal Structures</skos:prefLabel>
  <skos:altLabel>THERMALSTR</skos:altLabel>
  <skos:broader rdf:resource='urn:comp:1347'/>
  <skos:scopeNote>Research knowledge, capabilities, and practices for
    designing, developing, analyzing, and validating
    thermal-structural concepts for aerospace systems subjected
    to extreme operational environments and for developing
    design technology for thermal-structures applications and
    for multiscale optimization of metallic materials,
    structures, and fabrication processes.
  </skos:scopeNote>
  <nt2:status>Approved</nt2:status>
  <nt2:type>Descriptor</nt2:type>
  <nt2:inputdate>2006-12-13</nt2:inputdate>
  <dcterms:modified>2006-12-13</dcterms:modified>
  <nt2:code>105</nt2:code>
 </skos:Concept>
 <skos:Concept rdf:about='urn:comp:95'>
  <skos:prefLabel>Remote Sensing Technologies</skos:prefLabel>
  <skos:altLabel>REMOTESENS</skos:altLabel>
  <skos:broader rdf:resource='urn:comp:1339'/>
  <skos:scopeNote>Knowledge, capabilities, and practices related to the
    reasearch, design, development, characterization, and
    application of active and passive remote sensing and
    detector systems. This includes advanced flight-qualified
    laser systems, optical components, microwave systems,
    radiometric sensors, and other remote sensing instruments
    as well as associated component subsystems, detectors,
    calibration systems, and data acquisition systems. Includes
    knowledge of, and capability to perform, research and
    development of advanced detectors and detector systems
    covering a wide spectral range to include UV, visible, IR,
    and microwave. May include the design, development, test,
    characterization, and
  </skos:scopeNote>
  <nt2:status>Approved</nt2:status>
  <nt2:type>Descriptor</nt2:type>
  <nt2:inputdate>2006-12-13</nt2:inputdate>
  <dcterms:modified>2006-12-13</dcterms:modified>
  <nt2:code>95</nt2:code>
 </skos:Concept>
 <skos:Concept rdf:about='urn:comp:114'>
  <skos:prefLabel>Process Engineering</skos:prefLabel>
  <skos:altLabel>PROCESSENG</skos:altLabel>
  <skos:broader rdf:resource='urn:comp:1209'/>
  <skos:changeNote>???
  </skos:changeNote>
  <skos:scopeNote>Knowledge, capabilities and practices associated with the
    development and implementation of safe, efficient, and
    effective processes to achieve performance excellence in
    Center operations, development, and enabling functions.
    This includes the identification, development, mapping,
    modeling, measuring, and analysis of processes that enable
    work activities, including their suppliers, inputs,
    outputs, customers, outcomes, and related decisions. Areas
    of specialization
    include queuing theory, function analysis, work method/task
    analysis, human factors, stochastic methods, advanced
    statistical analysis methods, process improvement
    techniques, optimization algorithms, process simulation
    modeling (discrete and/or continuous), linear programming,
    and scheduling and capacity analysis systems.
  </skos:scopeNote>
  <nt2:status>Approved</nt2:status>
  <nt2:type>Descriptor</nt2:type>
  <nt2:inputdate>2006-12-13</nt2:inputdate>
  <dcterms:dateAccepted>2005-12-07</dcterms:dateAccepted>
  <dcterms:modified>2006-12-18</dcterms:modified>
  <nt2:code>114</nt2:code>
 </skos:Concept>
 <skos:Concept rdf:about='urn:comp:1077'>
  <skos:prefLabel>Industrial Security</skos:prefLabel>
  <skos:altLabel>SECINDUST</skos:altLabel>
  <skos:broader rdf:resource='urn:comp:126'/>
  <skos:scopeNote>This competency refers to the knowledge and ability to
    perform personnel, physical, and information security
    functions related to contractors and contract facilities,
    in accordance with the National Industrial Security Program
    (NISP), established by Executive Order 12829; the National
    Industrial Security Program Operating Manual (NISPOM),
    NIPSOM Supplement and Executive Order 12958, "Classified
    National Security Information. Includes ensuring that
    private industry and colleges/universities, while
    performing on government contracts or conducting research
    and development, properly protect classified assets in
    their possession. Capabilities include conducting site
    security reviews and establishing criteria for contractors
    and subcontractors covering such matters as foreign
    ownership or influence; classification and clearance levels
    required for contract performance; product classification;
    and access to communication security, intelligence or
    international organization information.
  </skos:scopeNote>
  <nt2:status>Approved</nt2:status>
  <nt2:type>Descriptor</nt2:type>
  <nt2:inputdate>2006-12-13</nt2:inputdate>
  <dcterms:modified>2006-12-13</dcterms:modified>
  <nt2:code>1077</nt2:code>
 </skos:Concept>
 <skos:Concept rdf:about='urn:comp:131'>
  <skos:prefLabel>Business IT Systems</skos:prefLabel>
  <skos:altLabel>BITSYS</skos:altLabel>
  <skos:broader rdf:resource='urn:comp:1125'/>
  <skos:narrower rdf:resource='urn:comp:1078'/>
  <skos:narrower rdf:resource='urn:comp:1081'/>
  <skos:narrower rdf:resource='urn:comp:1079'/>
  <skos:scopeNote>Knowledge, capabilities and practices associated with
    computer architectures and computer-based information
    systems related to business operations and mission support.
    This competency is based on knowledge comprised from one or
    more of the following interrelated technologies: computer
    and other hardware, programming languages, commercial
    operating systems, web or database systems, network
    hardware and software, IT security and other technologies
    that pertain to the acquisition, computation, storage,
    distribution, reporting, and management of information.
  </skos:scopeNote>
  <nt2:status>Approved</nt2:status>
  <nt2:type>Descriptor</nt2:type>
  <nt2:inputdate>2006-12-13</nt2:inputdate>
  <dcterms:modified>2006-12-13</dcterms:modified>
  <nt2:code>131</nt2:code>
 </skos:Concept>
 <skos:Concept rdf:about='urn:comp:1014'>
  <skos:prefLabel>Human-Machine Interaction Fundamental Research</skos:prefLabel>
  <skos:altLabel>HFRHUMMACH</skos:altLabel>
  <skos:broader rdf:resource='urn:comp:40'/>
  <skos:scopeNote>TBD (includes human-computer interaction and
    human-automation interaction) (includes human-computer
    interaction and human-automation interaction)
  </skos:scopeNote>
  <nt2:status>Approved</nt2:status>
  <nt2:type>Descriptor</nt2:type>
  <nt2:inputdate>2006-12-13</nt2:inputdate>
  <dcterms:modified>2006-12-13</dcterms:modified>
  <nt2:code>1014</nt2:code>
 </skos:Concept>
 <skos:Concept rdf:about='urn:comp:1057'>
  <skos:prefLabel>Spacecraft and Auxiliary Propulsion System Design and Analysis</skos:prefLabel>
  <skos:altLabel>RPAUXPRP</skos:altLabel>
  <skos:broader rdf:resource='urn:comp:73'/>
  <skos:scopeNote>Knowledge, capabilities and practices associated with the
    development of reaction control thrusters, orbital
    manuevering engines, pressurization systems, propellant
    acquisition devices and feedsystems for storable and
    cryogenic propellants in pressure-fed spacecraft auxiliary
    propulsion systems.
  </skos:scopeNote>
  <nt2:status>Approved</nt2:status>
  <nt2:type>Descriptor</nt2:type>
  <nt2:inputdate>2006-12-13</nt2:inputdate>
  <dcterms:modified>2006-12-13</dcterms:modified>
  <nt2:code>1057</nt2:code>
 </skos:Concept>
 <skos:Concept rdf:about='urn:comp:1347'>
  <skos:prefLabel>Structures, Materials &amp; Mechanics Competency Suite</skos:prefLabel>
  <skos:broader rdf:resource='urn:comp:1208'/>
  <skos:narrower rdf:resource='urn:comp:64'/>
  <skos:narrower rdf:resource='urn:comp:66'/>
  <skos:narrower rdf:resource='urn:comp:17'/>
  <skos:narrower rdf:resource='urn:comp:62'/>
  <skos:narrower rdf:resource='urn:comp:67'/>
  <skos:narrower rdf:resource='urn:comp:61'/>
  <skos:narrower rdf:resource='urn:comp:63'/>
  <skos:narrower rdf:resource='urn:comp:105'/>
  <nt2:status>Approved</nt2:status>
  <nt2:type>Descriptor</nt2:type>
  <nt2:inputdate>2006-12-13</nt2:inputdate>
  <dcterms:modified>2006-12-18</dcterms:modified>
  <nt2:code>1347</nt2:code>
 </skos:Concept>
 <skos:Concept rdf:about='urn:comp:98'>
  <skos:prefLabel>Flight Dynamics</skos:prefLabel>
  <skos:altLabel>FLTDYN</skos:altLabel>
  <skos:broader rdf:resource='urn:comp:1237'/>
  <skos:scopeNote>Knowledge, capabilities, and practices associated with
    research and technology in analytical, computational, and
    experimental methods to characterize the flight dynamics
    behaviors of aerospace vehicles.
  </skos:scopeNote>
  <nt2:status>Approved</nt2:status>
  <nt2:type>Descriptor</nt2:type>
  <nt2:inputdate>2006-12-13</nt2:inputdate>
  <dcterms:modified>2006-12-13</dcterms:modified>
  <nt2:code>98</nt2:code>
 </skos:Concept>
 <skos:Concept rdf:about='urn:comp:130'>
  <skos:prefLabel>Occupational and Environmental Health</skos:prefLabel>
  <skos:altLabel>OCCHEALTH</skos:altLabel>
  <skos:broader rdf:resource='urn:comp:1159'/>
  <skos:narrower rdf:resource='urn:comp:1069'/>
  <skos:narrower rdf:resource='urn:comp:1068'/>
  <skos:narrower rdf:resource='urn:comp:1067'/>
  <skos:narrower rdf:resource='urn:comp:1066'/>
  <skos:scopeNote>Knowledge, capabilities, and practice associated with NASA,
    Federal, and State OSHA health and safety regulations,
    policies and procedures used to develop and implement
    mishap and environmental health prevention practices and
    measures in all NASA work places. These knowledge areas
    include safety of personnel and equipment during launch
    vehicle processing, normal and industrial and laboratory
    operations, special high hazard tests and operations,
    aviation and space operations, use and handling of
    materials and chemicals, and design, construction, and use
    of facilities. Capabilities include ability to develop and
    analyze policy, manage, and assess the effectiveness of
    health programs and practices, which are designed to
    prevent injury to personnel and loss of NASA property in
    the industrial work environment, and promote the health and
    well being of employees.
  </skos:scopeNote>
  <nt2:status>Approved</nt2:status>
  <nt2:type>Descriptor</nt2:type>
  <nt2:inputdate>2006-12-13</nt2:inputdate>
  <dcterms:modified>2006-12-13</dcterms:modified>
  <nt2:code>130</nt2:code>
 </skos:Concept>
 <skos:Concept rdf:about='urn:comp:1283'>
  <skos:prefLabel>Computer Science &amp; Information Technology Competency Suite</skos:prefLabel>
  <skos:broader rdf:resource='urn:comp:1208'/>
  <skos:narrower rdf:resource='urn:comp:80'/>
  <skos:narrower rdf:resource='urn:comp:161'/>
  <skos:narrower rdf:resource='urn:comp:166'/>
  <skos:narrower rdf:resource='urn:comp:85'/>
  <skos:narrower rdf:resource='urn:comp:81'/>
  <skos:narrower rdf:resource='urn:comp:84'/>
  <skos:narrower rdf:resource='urn:comp:79'/>
  <skos:narrower rdf:resource='urn:comp:82'/>
  <nt2:status>Approved</nt2:status>
  <nt2:type>Descriptor</nt2:type>
  <nt2:inputdate>2006-12-13</nt2:inputdate>
  <dcterms:modified>2006-12-13</dcterms:modified>
  <nt2:code>1283</nt2:code>
 </skos:Concept>
 <skos:Concept rdf:about='urn:comp:1017'>
  <skos:prefLabel>Training and Adaptation Fundamental Research</skos:prefLabel>
  <skos:altLabel>HFRTRNG</skos:altLabel>
  <skos:broader rdf:resource='urn:comp:40'/>
  <skos:scopeNote>TBD (includes basic research on perceptual and behavioral
    adaptation, learning, memory, etc.)
  </skos:scopeNote>
  <nt2:status>Approved</nt2:status>
  <nt2:type>Descriptor</nt2:type>
  <nt2:inputdate>2006-12-13</nt2:inputdate>
  <dcterms:modified>2006-12-13</dcterms:modified>
  <nt2:code>1017</nt2:code>
 </skos:Concept>
 <skos:Concept rdf:about='urn:comp:175'>
  <skos:prefLabel>Simulation Systems</skos:prefLabel>
  <skos:altLabel>SIMULATE</skos:altLabel>
  <skos:broader rdf:resource='urn:comp:1231'/>
  <skos:scopeNote>Knowledge, capabilities, and practices associated with
    real-time simulation which is a realistic representation of
    the physical system being studied (as opposed to pure
    mathematical analysis or standard computer analysis) and
    permits both quantitative and qualitative (human analysis)
    evaluation. A simulation system is usually characterized by
    a space or aviation flight deck/cockpit, interface
    hardware, computers, and flight crew, all of which are
    linked together in a closed loop system. In addition,
    flight crew can be trained for various operational concepts
    without using expensive vehicles.
    Require knowledge and experience in real-time concepts,
    computer system engineering and operations; simulator
    hardware engineering, operation, and maintenance; real-time
    simulation modeling analysis; and real-time software
    design, development, verification, and validation.
    Require knowledge and capabilities in simulator hardware
    engineering that includes design and implementation of a
    flight deck equiped with instrument panels, side
    stick/wheel column as vehicle controlling devices, visual
    scene for out-the-window view, heads-down display systems,
    and environmental sound effects.
    Require knowledge and capabilities in developing and
    operating a simulation driven by high speed, high
    performance computers for complex math model computation;
    specialized graphics computers, visual scence computers,
    and video distribution; high performance computer network;
    and special purpose software for real-time math modeling,
    graphics generation, system interfaces, communications, and
    networking.
  </skos:scopeNote>
  <nt2:status>Approved</nt2:status>
  <nt2:type>Descriptor</nt2:type>
  <nt2:inputdate>2006-12-13</nt2:inputdate>
  <dcterms:dateAccepted>2006-04-05</dcterms:dateAccepted>
  <dcterms:modified>2006-12-18</dcterms:modified>
  <nt2:code>175</nt2:code>
 </skos:Concept>
 <skos:Concept rdf:about='urn:comp:1029'>
  <skos:prefLabel>Electrical Design and Development Engineering</skos:prefLabel>
  <skos:altLabel>DDEELEC</skos:altLabel>
  <skos:broader rdf:resource='urn:comp:8'/>
  <skos:scopeNote>Knowledge, capability and practices associated with all
    aspects of the technical electrical design and development
    process of electrical systems and components for air, space
    and ground systems and instruments. Includes knowledge of
    electrical integration such as electrical / electronic
    design requirements definition, subsystem and circuit
    analysis, test procedure development, and safety analysis.
    Includes broad knowledge EEE parts, electronic packaging
    design and tools, reliability and environmental effects,
    power generation, distribution, storage and conditioning
    systems.
  </skos:scopeNote>
  <nt2:status>Approved</nt2:status>
  <nt2:type>Descriptor</nt2:type>
  <nt2:inputdate>2006-12-13</nt2:inputdate>
  <dcterms:modified>2006-12-13</dcterms:modified>
  <nt2:code>1029</nt2:code>
 </skos:Concept>
 <skos:Concept rdf:about='urn:comp:1099'>
  <skos:prefLabel>Large Scale Data Systems</skos:prefLabel>
  <skos:altLabel>DATLARGE</skos:altLabel>
  <skos:broader rdf:resource='urn:comp:161'/>
  <skos:scopeNote>Knowledge of design, development and implementation of
    large-scale scientific data storage, access, retrieval and
    mining systems or techniques. Includes ability to transfer
    research algorithms into processing code that produces
    scientific data products for the science community.
    Includes knowledge of image methods and procedures for
    automated feature extraction from large data sets.
  </skos:scopeNote>
  <nt2:status>Approved</nt2:status>
  <nt2:type>Descriptor</nt2:type>
  <nt2:inputdate>2006-12-13</nt2:inputdate>
  <dcterms:modified>2006-12-13</dcterms:modified>
  <nt2:code>1099</nt2:code>
 </skos:Concept>
 <skos:Concept rdf:about='urn:comp:84'>
  <skos:prefLabel>Neural Networks &amp; Systems</skos:prefLabel>
  <skos:altLabel>NEUNETSYS</skos:altLabel>
  <skos:broader rdf:resource='urn:comp:1283'/>
  <skos:scopeNote>Knowledge, capabilities, and practices of synthesizing
    practical implementations of artificial neural networks for
    application to NASA missions, programs, and projects. This
    includes such applications as machine learning algorithms
    and pattern recognition systems for intelligent flight
    control systems, complex spacecraft docking capabilities,
    and instrument control mechanisms.
  </skos:scopeNote>
  <nt2:status>Approved</nt2:status>
  <nt2:type>Descriptor</nt2:type>
  <nt2:inputdate>2006-12-13</nt2:inputdate>
  <dcterms:modified>2006-12-13</dcterms:modified>
  <nt2:code>84</nt2:code>
 </skos:Concept>
 <skos:Concept rdf:about='urn:comp:1208'>
  <skos:prefLabel>Engineering &amp; Technology Knowledge Domain</skos:prefLabel>
  <skos:broader rdf:resource='urn:comp:1438'/>
  <skos:narrower rdf:resource='urn:comp:1237'/>
  <skos:narrower rdf:resource='urn:comp:1280'/>
  <skos:narrower rdf:resource='urn:comp:1283'/>
  <skos:narrower rdf:resource='urn:comp:1294'/>
  <skos:narrower rdf:resource='urn:comp:1209'/>
  <skos:narrower rdf:resource='urn:comp:1244'/>
  <skos:narrower rdf:resource='urn:comp:1363'/>
  <skos:narrower rdf:resource='urn:comp:1314'/>
  <skos:narrower rdf:resource='urn:comp:1339'/>
  <skos:narrower rdf:resource='urn:comp:1347'/>
  <skos:narrower rdf:resource='urn:comp:1231'/>
  <skos:narrower rdf:resource='urn:comp:1359'/>
  <nt2:status>Approved</nt2:status>
  <nt2:type>Descriptor</nt2:type>
  <nt2:inputdate>2006-12-13</nt2:inputdate>
  <dcterms:modified>2007-01-11</dcterms:modified>
  <nt2:code>1208</nt2:code>
 </skos:Concept>
 <skos:Concept rdf:about='urn:comp:1047'>
  <skos:prefLabel>Vehicle Control Design and Analysis</skos:prefLabel>
  <skos:altLabel>GNCVEHCNTL</skos:altLabel>
  <skos:broader rdf:resource='urn:comp:22'/>
  <skos:scopeNote>Knowledge of and ability to research and develop
    analytical, computational, and experimental methods for
    control algorithm and control mechnism design and
    development for launch vehicles, space vehicles, and space
    systems and subsystems. Apply research to develop
    requirements for control mechanisms, sensors and
    instrumentation systems; establish functional, performance,
    design, analysis, test, integration and verification
    requirements for vehicle control systems, subsystems,
    control mechanisms and components; and use analytical
    modeling and simulation tools that determine control system
    solutions. Knowledge of research and engineering of
    integrated aerospace vehicle systems for vehicle control
    and health management of flight vehicles in the atmosphere
    and space. Includes knowledge of sensors, avionics,
    actuation and control mechanisms, flight dynamics,
    mathematical modeling, experimental methods and a broad
    array of engineering disciplines.
  </skos:scopeNote>
  <nt2:status>Approved</nt2:status>
  <nt2:type>Descriptor</nt2:type>
  <nt2:inputdate>2006-12-13</nt2:inputdate>
  <dcterms:modified>2006-12-13</dcterms:modified>
  <nt2:code>1047</nt2:code>
 </skos:Concept>
 <skos:Concept rdf:about='urn:comp:1107'>
  <skos:prefLabel>Precursor Analysis</skos:prefLabel>
  <skos:altLabel>PRECURSOR</skos:altLabel>
  <skos:broader rdf:resource='urn:comp:27'/>
  <skos:scopeNote>Knowledge, capabilities, and practices associated with the
    identification of forerunners to failure. Knowledge of risk
    analysis techniques and risk models to be able to infer the
    risk implications of conditions, events or sequences of
    events that are precursors to accidents. Knowledge of
    quantification techniques to assess the probability
    implications of a precursor event or a precursor sequence
    events. Involves the screening of data and records to
    identify potential candidate precursors and assessing the
    risk implications of the screened events to estimate the
    severity of the event in terms of the nearness of the event
    to a failure or accident. Involves the assessment of
    preventative or mitigative actions to determine their
    impact on the precursor probability or consequences.
  </skos:scopeNote>
  <nt2:status>Approved</nt2:status>
  <nt2:type>Descriptor</nt2:type>
  <nt2:inputdate>2006-12-13</nt2:inputdate>
  <dcterms:modified>2006-12-13</dcterms:modified>
  <nt2:code>1107</nt2:code>
 </skos:Concept>
 <skos:Concept rdf:about='urn:comp:53'>
  <skos:prefLabel>Planetary Science</skos:prefLabel>
  <skos:altLabel>PLANETSCI</skos:altLabel>
  <skos:broader rdf:resource='urn:comp:1407'/>
  <skos:scopeNote>Knowledge of space science applied to conducting
    experimental, observational, and theoretical studies and
    modeling of planets, planetary satellites, asteroids,
    comets, meteoroids, and other objects, media, and particles
    in the solar system, in order to determine their
    composition and properties in such areas as atmospheres,
    magnetospheres, lithospheres, cryospheres, and interiors.
  </skos:scopeNote>
  <nt2:status>Approved</nt2:status>
  <nt2:type>Descriptor</nt2:type>
  <nt2:inputdate>2006-12-13</nt2:inputdate>
  <dcterms:modified>2006-12-13</dcterms:modified>
  <nt2:code>53</nt2:code>
 </skos:Concept>
 <skos:Concept rdf:about='urn:comp:1124'>
  <skos:prefLabel>Business Knowledge Domain</skos:prefLabel>
  <skos:broader rdf:resource='urn:comp:1438'/>
  <skos:narrower rdf:resource='urn:comp:1125'/>
  <skos:narrower rdf:resource='urn:comp:1150'/>
  <skos:narrower rdf:resource='urn:comp:1159'/>
  <skos:narrower rdf:resource='urn:comp:1189'/>
  <nt2:status>Approved</nt2:status>
  <nt2:type>Descriptor</nt2:type>
  <nt2:inputdate>2006-12-13</nt2:inputdate>
  <dcterms:modified>2007-01-11</dcterms:modified>
  <nt2:code>1124</nt2:code>
 </skos:Concept>
 <skos:Concept rdf:about='urn:comp:1021'>
  <skos:prefLabel>Space Human Factors Engineering, Technology, and Standards</skos:prefLabel>
  <skos:altLabel>HFESPACE</skos:altLabel>
  <skos:broader rdf:resource='urn:comp:41'/>
  <skos:scopeNote>TBD (focus on humans in micro-gravity, radiation
    environments)
  </skos:scopeNote>
  <nt2:status>Approved</nt2:status>
  <nt2:type>Descriptor</nt2:type>
  <nt2:inputdate>2006-12-13</nt2:inputdate>
  <dcterms:modified>2006-12-13</dcterms:modified>
  <nt2:code>1021</nt2:code>
 </skos:Concept>
 <skos:Concept rdf:about='urn:comp:24'>
  <skos:prefLabel>Manufacturing Engineering</skos:prefLabel>
  <skos:altLabel>MANUFACT</skos:altLabel>
  <skos:broader rdf:resource='urn:comp:1209'/>
  <skos:scopeNote>Knowledge, capabilities and practices to perform concurrent
    engineering and producibility. Includes knowledge and
    ability to review design documentation, determine resource
    requirements for manufacturing activities, research and
    develop manufacturing processes, plan and manage hardware
    fabrication and assembly, develop and maintain
    manufacturing project schedules, and resolve manufacturing
    related problems.
  </skos:scopeNote>
  <nt2:status>Approved</nt2:status>
  <nt2:type>Descriptor</nt2:type>
  <nt2:inputdate>2006-12-13</nt2:inputdate>
  <dcterms:modified>2006-12-13</dcterms:modified>
  <nt2:code>24</nt2:code>
 </skos:Concept>
 <skos:Concept rdf:about='urn:comp:1159'>
  <skos:prefLabel>Institutional Operations &amp; Support Competency Suite</skos:prefLabel>
  <skos:broader rdf:resource='urn:comp:1124'/>
  <skos:narrower rdf:resource='urn:comp:151'/>
  <skos:narrower rdf:resource='urn:comp:112'/>
  <skos:narrower rdf:resource='urn:comp:143'/>
  <skos:narrower rdf:resource='urn:comp:152'/>
  <skos:narrower rdf:resource='urn:comp:133'/>
  <skos:narrower rdf:resource='urn:comp:134'/>
  <skos:narrower rdf:resource='urn:comp:167'/>
  <skos:narrower rdf:resource='urn:comp:130'/>
  <skos:narrower rdf:resource='urn:comp:168'/>
  <skos:narrower rdf:resource='urn:comp:126'/>
  <skos:narrower rdf:resource='urn:comp:150'/>
  <nt2:status>Approved</nt2:status>
  <nt2:type>Descriptor</nt2:type>
  <nt2:inputdate>2006-12-13</nt2:inputdate>
  <dcterms:modified>2006-12-13</dcterms:modified>
  <nt2:code>1159</nt2:code>
 </skos:Concept>
 <skos:Concept rdf:about='urn:comp:1081'>
  <skos:prefLabel>Information Systems Security</skos:prefLabel>
  <skos:altLabel>BITSECURE</skos:altLabel>
  <skos:broader rdf:resource='urn:comp:131'/>
  <skos:scopeNote>Knowledge of methods, tools, and procedures, including
    development of information security plans, to prevent
    information systems vulnerabilities, and provide or restore
    security of information systems and network services. May
    also include the knowledge of the principles, methods, and
    tools for evaluating information systems security features
    against a set of specified security requirements.
  </skos:scopeNote>
  <nt2:status>Approved</nt2:status>
  <nt2:type>Descriptor</nt2:type>
  <nt2:inputdate>2006-12-13</nt2:inputdate>
  <dcterms:modified>2006-12-13</dcterms:modified>
  <nt2:code>1081</nt2:code>
 </skos:Concept>
 <skos:Concept rdf:about='urn:comp:1097'>
  <skos:prefLabel>Real Property Management</skos:prefLabel>
  <skos:altLabel>FACPROPRTY</skos:altLabel>
  <skos:broader rdf:resource='urn:comp:112'/>
  <skos:scopeNote>Knowledge of requirements and processes to manage real
    property including buildings, other infrastructure, land,
    and leases and other interests in property and real estate
    for industrial and aerospace operations. Knowledge of real
    estate principles, practices and law as they apply to the
    management, leasing or acquisition of real estate.
    Knowledge of records management for financial accounting
    and value maintenance, including development of files and
    records to serve as legal documentation of ownership and
    material value. Knowledge of facility utilization
    include space planning and tracking for institutional
    charges as well as for space management and utilization
    reporting at the agency as well as at the federal level.
  </skos:scopeNote>
  <nt2:status>Approved</nt2:status>
  <nt2:type>Descriptor</nt2:type>
  <nt2:inputdate>2006-12-13</nt2:inputdate>
  <dcterms:modified>2006-12-13</dcterms:modified>
  <nt2:code>1097</nt2:code>
 </skos:Concept>
 <skos:Concept rdf:about='urn:comp:93'>
  <skos:prefLabel>Optical Systems</skos:prefLabel>
  <skos:altLabel>OPTSYS</skos:altLabel>
  <skos:broader rdf:resource='urn:comp:1339'/>
  <skos:scopeNote>Applies principles and practices related to the research,
    design, development, test, and evaluation and/or operation
    of optical components and systems, including optical
    sensors and optical data/image processing. Inherent within
    this competency is knowledge, capabilities, and practices
    associated with mechanically and digitally based optical
    instruments and associated measurement systems required to
    support siting, construction, assembly or operation of
    facilities, flight vehicles, payloads, infrastructure,
    and/or associated ground support equipment and processes.
    This includes the knowledge of light and optical theory and
    its application, surveying techniques; measurement
    equipment operation, care and calibration; measurement data
    acquisition and data processing techniques; and system
    unique requirements for the safe and effective
    implementation of data acquisition in a wide variety of
    systems.
  </skos:scopeNote>
  <nt2:status>Approved</nt2:status>
  <nt2:type>Descriptor</nt2:type>
  <nt2:inputdate>2006-12-13</nt2:inputdate>
  <dcterms:modified>2006-12-13</dcterms:modified>
  <nt2:code>93</nt2:code>
 </skos:Concept>
 <skos:Concept rdf:about='urn:comp:113'>
  <skos:prefLabel>Business Management</skos:prefLabel>
  <skos:altLabel>BUSMMT</skos:altLabel>
  <skos:broader rdf:resource='urn:comp:1125'/>
  <skos:scopeNote>Knowledge of principles and practices related to managing
    the internal and external operations of a business unit,
    such as a Center, to accomplish mission objectives and
    goals efficiently. Includes ability to integrate
    performance goals with budget and financial resources as
    well as the ability to achieve customer satisfaction,
    develop strong relationships with other NASA and external
    entities, and adhere to agencywide programs, policies, and
    procedures. Understanding ofAgency and federal government
    financial, budget and performance operations and processes,
    and how to apply these processes to optimize operational
    and investment decisions.
  </skos:scopeNote>
  <nt2:status>Approved</nt2:status>
  <nt2:type>Descriptor</nt2:type>
  <nt2:inputdate>2006-12-13</nt2:inputdate>
  <dcterms:modified>2006-12-13</dcterms:modified>
  <nt2:code>113</nt2:code>
 </skos:Concept>
 <skos:Concept rdf:about='urn:comp:1393'>
  <skos:prefLabel>Leadership &amp; Management Knowledge Domain</skos:prefLabel>
  <skos:broader rdf:resource='urn:comp:1438'/>
  <skos:narrower rdf:resource='urn:comp:1394'/>
  <skos:narrower rdf:resource='urn:comp:1399'/>
  <nt2:status>Approved</nt2:status>
  <nt2:type>Descriptor</nt2:type>
  <nt2:inputdate>2006-12-13</nt2:inputdate>
  <dcterms:modified>2007-01-11</dcterms:modified>
  <nt2:code>1393</nt2:code>
 </skos:Concept>
 <skos:Concept rdf:about='urn:comp:1059'>
  <skos:prefLabel>Dynamic Data Analysis</skos:prefLabel>
  <skos:altLabel>RPDYNDATA</skos:altLabel>
  <skos:broader rdf:resource='urn:comp:73'/>
  <skos:scopeNote>Diagnostic evaluation of rocket engine vibration data
    acquired from high frequency sensors such as
    accelerometers, strain gauges, proximity probes, and
    fluctuating pressures. Data from these sensors is acquired
    at high speeds (10,000 to 100,000 samples/second) allowing
    for high frequency spectral analysis to be performed on
    engine/engine components. Time, frequency, and phase domain
    analyses results are maintained in databases that are
    utilized to determine engine/engine component health,
    statistical family comparability, and flight acceptability.
    NASA Competency Management SystemPage 46
  </skos:scopeNote>
  <nt2:status>Approved</nt2:status>
  <nt2:type>Descriptor</nt2:type>
  <nt2:inputdate>2006-12-13</nt2:inputdate>
  <dcterms:modified>2006-12-13</dcterms:modified>
  <nt2:code>1059</nt2:code>
 </skos:Concept>
 <skos:Concept rdf:about='urn:comp:16'>
  <skos:prefLabel>Micro-Electromechanical Systems</skos:prefLabel>
  <skos:altLabel>MICROELMEC</skos:altLabel>
  <skos:broader rdf:resource='urn:comp:1294'/>
  <skos:scopeNote>Knowledge, capabilities and practices associated with the
    research, design, development, test, evaluation,
    application and manufacture of MEMS technologies, including
    microfabrication, microsystem design and integration,
    modeling, and packaging.
  </skos:scopeNote>
  <nt2:status>Approved</nt2:status>
  <nt2:type>Descriptor</nt2:type>
  <nt2:inputdate>2006-12-13</nt2:inputdate>
  <dcterms:modified>2006-12-13</dcterms:modified>
  <nt2:code>16</nt2:code>
 </skos:Concept>
 <skos:Concept rdf:about='urn:comp:1091'>
  <skos:prefLabel>Facility Mechanical Engineering</skos:prefLabel>
  <skos:altLabel>FACMECHENG</skos:altLabel>
  <skos:broader rdf:resource='urn:comp:112'/>
  <skos:scopeNote>Knowledge of planning, designing, developing, testing, or
    evaluating mechanical, electromechanical, pneumatic,
    hydraulic, fluid or structural equipment and systems for
    aerospace facility programs. May include specialization in
    Heating Ventalation and Air Conditioning (HVAC), piping and
    elevators. etc. Also requires knowledge of construction
    contracting and contractor oversight and contracts
    management.
  </skos:scopeNote>
  <nt2:status>Approved</nt2:status>
  <nt2:type>Descriptor</nt2:type>
  <nt2:inputdate>2006-12-13</nt2:inputdate>
  <dcterms:modified>2006-12-13</dcterms:modified>
  <nt2:code>1091</nt2:code>
 </skos:Concept>
 <skos:Concept rdf:about='urn:comp:42'>
  <skos:prefLabel>Fundamental Physics</skos:prefLabel>
  <skos:altLabel>FUNPHYSICS</skos:altLabel>
  <skos:broader rdf:resource='urn:comp:1424'/>
  <skos:scopeNote>Knowledge, capabilities and practices associated with
    research and application of electromagnetism, continuum and
    classical mechanics, quantum mechanics, and thermodynamics.
    May also include studies in materials, cryogenics,
    acoustics, and electromagnetic fields ranging from DC to
    X-ray. It also includes the development of sensors
    necessary to carry out these studies. Involves ability to
    conduct microgravitational research designed to answer
    basic questions about the nature and structure of the
    universe and its chemical, biological and geophysical
    systems.
  </skos:scopeNote>
  <nt2:status>Approved</nt2:status>
  <nt2:type>Descriptor</nt2:type>
  <nt2:inputdate>2006-12-13</nt2:inputdate>
  <dcterms:modified>2006-12-13</dcterms:modified>
  <nt2:code>42</nt2:code>
 </skos:Concept>
 <skos:Concept rdf:about='urn:comp:1093'>
  <skos:prefLabel>Acquisition Planning</skos:prefLabel>
  <skos:altLabel>ACQPLAN</skos:altLabel>
  <skos:broader rdf:resource='urn:comp:124'/>
  <skos:scopeNote>Knowledge of contract regulations and government contract
    vehicles, and ability to form contracts through source
    selection planning, identifying solicitation terms and
    conditions, and identifying and selecting techniques for
    determining price reasonableness. Also includes ability to
    recognize factors to be considered when evaluating and
    providing government financing, conducting price analyses,
    negotiating, identifying actions to resolve protests, and
    contract awarding.
  </skos:scopeNote>
  <nt2:status>Approved</nt2:status>
  <nt2:type>Descriptor</nt2:type>
  <nt2:inputdate>2006-12-13</nt2:inputdate>
  <dcterms:modified>2006-12-13</dcterms:modified>
  <nt2:code>1093</nt2:code>
 </skos:Concept>
 <skos:Concept rdf:about='urn:comp:35'>
  <skos:prefLabel>Biomedical Engineering</skos:prefLabel>
  <skos:altLabel>BIOMEDENG</skos:altLabel>
  <skos:broader rdf:resource='urn:comp:1244'/>
  <skos:scopeNote>Knowledge of engineering, design, development, analysis and
    test of biomedical systems such as equipment and tools for
    maintaining crew psychological and physical health for
    long-duration missions in space. Involves knowledge of
    broad array of engineering disciplines, and biomedical
    research, human factors and space medicine findings and
    practices. Includes knowledge of operational impacts and
    sustaining engineering on the systems.
  </skos:scopeNote>
  <nt2:status>Approved</nt2:status>
  <nt2:type>Descriptor</nt2:type>
  <nt2:inputdate>2006-12-13</nt2:inputdate>
  <dcterms:modified>2006-12-13</dcterms:modified>
  <nt2:code>35</nt2:code>
 </skos:Concept>
 <skos:Concept rdf:about='urn:comp:1048'>
  <skos:prefLabel>Guidance Design and Analysis</skos:prefLabel>
  <skos:altLabel>GNCGUIDE</skos:altLabel>
  <skos:broader rdf:resource='urn:comp:22'/>
  <skos:scopeNote>Design of guidance algorithms that command vehicle attitude
    angles and throttle settings (if applicable) for taking a
    vehicle from the current state to the desired final state
    in an optimal fashion within constraints. Includes all
    flight phases. Implementation of guidance algorithms in
    simulation. Support of vehicle design analysis through
    guided simulations including aborts and dispersions.
    Support of verification through demonstration that guidance
    integrates with the other subsystems to meet overall
    requirements. Detailed definition of guidance algorithms
    and support of software development and testing.
  </skos:scopeNote>
  <nt2:status>Approved</nt2:status>
  <nt2:type>Descriptor</nt2:type>
  <nt2:inputdate>2006-12-13</nt2:inputdate>
  <dcterms:modified>2006-12-13</dcterms:modified>
  <nt2:code>1048</nt2:code>
 </skos:Concept>
 <skos:Concept rdf:about='urn:comp:171'>
  <skos:prefLabel>Technical Work &amp; Team Management</skos:prefLabel>
  <skos:altLabel>TECWORKMMT</skos:altLabel>
  <skos:broader rdf:resource='urn:comp:1394'/>
  <skos:scopeNote>Knowledge, capabilities and practices associated with
    individuals that must understand and manage both the
    aspects of technical work, as well as management of
    employees and/or teams. This pseudo competency requires the
    supervisor or lead to have the following competencies:
    Technical Management
    Employee &amp; Team Leadership
    Work Performance Leadership
  </skos:scopeNote>
  <nt2:status>Approved</nt2:status>
  <nt2:type>Descriptor</nt2:type>
  <nt2:inputdate>2006-12-13</nt2:inputdate>
  <dcterms:modified>2006-12-13</dcterms:modified>
  <nt2:code>171</nt2:code>
 </skos:Concept>
 <skos:Concept rdf:about='urn:comp:1076'>
  <skos:prefLabel>Personnel Security</skos:prefLabel>
  <skos:altLabel>SECPERSON</skos:altLabel>
  <skos:broader rdf:resource='urn:comp:126'/>
  <skos:scopeNote>Knowledge and ability to request background investigations
    appropriate to position sensitivity and to review and
    evaluate completed background investigations for the
    purpose of assessing loyalty, reliability, suitability, and
    trustworthiness of applicants, employees, and others to
    work for the U.S. Government, on U.S. Government contracts,
    and/or will have access to classified national security
    information and material.
  </skos:scopeNote>
  <nt2:status>Approved</nt2:status>
  <nt2:type>Descriptor</nt2:type>
  <nt2:inputdate>2006-12-13</nt2:inputdate>
  <dcterms:modified>2006-12-13</dcterms:modified>
  <nt2:code>1076</nt2:code>
 </skos:Concept>
 <skos:Concept rdf:about='urn:comp:5'>
  <skos:prefLabel>Payload Integration</skos:prefLabel>
  <skos:altLabel>PAYLOADINT</skos:altLabel>
  <skos:broader rdf:resource='urn:comp:1372'/>
  <skos:scopeNote>Applies knowledge and practices of management, science and
    engineering to lifecycle of all payload research
    experiments. Ability to optimize use of existing systems
    for accomplishment of science objectives, and to determine
    engineering requirements such as payload support hardware
    definition, design, fabrication, integration and testing,
    and operating procedures. Includes ability to integrate
    payloads into vehicles and determine requirements and
    predict operating impacts between payloads and vehicles.
    Ability to test and process payloads, and integrate them
    successfully on-board the vehicle.
  </skos:scopeNote>
  <nt2:status>Approved</nt2:status>
  <nt2:type>Descriptor</nt2:type>
  <nt2:inputdate>2006-12-13</nt2:inputdate>
  <dcterms:modified>2006-12-13</dcterms:modified>
  <nt2:code>5</nt2:code>
 </skos:Concept>
 <skos:Concept rdf:about='urn:comp:1399'>
  <skos:prefLabel>Professional Development Competency Suite</skos:prefLabel>
  <skos:broader rdf:resource='urn:comp:1393'/>
  <skos:narrower rdf:resource='urn:comp:140'/>
  <skos:narrower rdf:resource='urn:comp:122'/>
  <nt2:status>Approved</nt2:status>
  <nt2:type>Descriptor</nt2:type>
  <nt2:inputdate>2006-12-13</nt2:inputdate>
  <dcterms:modified>2006-12-13</dcterms:modified>
  <nt2:code>1399</nt2:code>
 </skos:Concept>
 <skos:Concept rdf:about='urn:comp:50'>
  <skos:prefLabel>Earth System Modeling</skos:prefLabel>
  <skos:altLabel>EARSYMODEL</skos:altLabel>
  <skos:broader rdf:resource='urn:comp:1415'/>
  <skos:scopeNote>Apply understanding of Earth systems to consolidation of
    scientific findings into integrated representations of
    atmosphere, ocean, ice land and biosphere systems, with the
    ability to predict future system trends and evolution of
    chemical and biological components.
  </skos:scopeNote>
  <nt2:status>Approved</nt2:status>
  <nt2:type>Descriptor</nt2:type>
  <nt2:inputdate>2006-12-13</nt2:inputdate>
  <dcterms:modified>2006-12-13</dcterms:modified>
  <nt2:code>50</nt2:code>
 </skos:Concept>
 <skos:Concept rdf:about='urn:comp:1049'>
  <skos:prefLabel>Navigation System Design and Analysis</skos:prefLabel>
  <skos:altLabel>GNCNAVSYS</skos:altLabel>
  <skos:broader rdf:resource='urn:comp:22'/>
  <skos:scopeNote>Knowledge of and ability to employ navigation hardware
    including Inertial Measurement Unit’s (IMU: gyro and
    accelerometers), Global Position Satellite receivers, star
    trackers, sun sensors, etc. Knowledge of and skill in using
    Kalman filtering and other software techniques to merge
    data from different sources to obtain an accurate and
    optimum navigation solution. Skill in using the output
    navigation solution for orbit determination.
  </skos:scopeNote>
  <nt2:status>Approved</nt2:status>
  <nt2:type>Descriptor</nt2:type>
  <nt2:inputdate>2006-12-13</nt2:inputdate>
  <dcterms:modified>2006-12-13</dcterms:modified>
  <nt2:code>1049</nt2:code>
 </skos:Concept>
 <skos:Concept rdf:about='urn:comp:34'>
  <skos:prefLabel>Biomedical Research</skos:prefLabel>
  <skos:altLabel>BIOMEDRES</skos:altLabel>
  <skos:broader rdf:resource='urn:comp:1430'/>
  <skos:scopeNote>Involves the capability to research, investigate and
    characterize the effects of space flight and exposure to
    microgravity, radiation, and other stresses on
    physiological functions (e.g., musculoskeletal,
    cardiovascular, etc.). In-depth understanding of the human
    body, its physical and chemical make-up and the associated
    technology and methods to examine the effects of various
    environments and stresses. Ability to understand the
    underlying physiological, behavioral and psychological
    mechanisms and performance aspects responsible for
    biomedical and behavioral changes in humans and animals
    during spaceflight and apply this information to conduct
    operational and clinical research to develop, and validate
    countermeasures that will ensure the health, safety and
    performance of flight crews involved during launches,
    landings, and while in space.
  </skos:scopeNote>
  <nt2:status>Approved</nt2:status>
  <nt2:type>Descriptor</nt2:type>
  <nt2:inputdate>2006-12-13</nt2:inputdate>
  <dcterms:modified>2006-12-13</dcterms:modified>
  <nt2:code>34</nt2:code>
 </skos:Concept>
 <skos:Concept rdf:about='urn:comp:128'>
  <skos:prefLabel>Human Capital Management</skos:prefLabel>
  <skos:altLabel>HUMCAPMMT</skos:altLabel>
  <skos:broader rdf:resource='urn:comp:1189'/>
  <skos:narrower rdf:resource='urn:comp:1115'/>
  <skos:narrower rdf:resource='urn:comp:1116'/>
  <skos:narrower rdf:resource='urn:comp:1117'/>
  <skos:narrower rdf:resource='urn:comp:1118'/>
  <skos:narrower rdf:resource='urn:comp:1119'/>
  <skos:narrower rdf:resource='urn:comp:1120'/>
  <skos:narrower rdf:resource='urn:comp:1121'/>
  <skos:narrower rdf:resource='urn:comp:1122'/>
  <skos:narrower rdf:resource='urn:comp:1123'/>
  <skos:scopeNote>Apply knowledge and practices of the full range of
    personnel/human resource functions, such as classification,
    workforce planning &amp; analysis, employee and labor
    relations, retirement, benefits, disciplinary actions,
    recruitment, selection, training, employee development,
    promotion regulations and procedures, compensation, and
    personnel information systems. Provide guidance and
    leadership in the motivation, performance measurement and
    overall management of the workforce including the design,
    delivery, implementation and evaluation of programs and
    processes. Includes understanding of organizational
    mission, strategy and business objectives as well as
    various rules, regulations and culture on people and their
    work.
  </skos:scopeNote>
  <nt2:status>Approved</nt2:status>
  <nt2:type>Descriptor</nt2:type>
  <nt2:inputdate>2006-12-13</nt2:inputdate>
  <dcterms:modified>2006-12-13</dcterms:modified>
  <nt2:code>128</nt2:code>
 </skos:Concept>
 <skos:Concept rdf:about='urn:comp:1053'>
  <skos:prefLabel>Turbomachinery Design and Analysis</skos:prefLabel>
  <skos:altLabel>RPTURBO</skos:altLabel>
  <skos:broader rdf:resource='urn:comp:73'/>
  <skos:scopeNote>Knowledge, capabilities and practices associated with
    defining, developing, integrating and verifying liquid
    engine
    turbomachinery for advanced propulsion systems. This
    includes the ability to derive turbomachinery design
    requirements, perform design analyses necessary to size
    turbomachinery, define hydrodynamic and aerodynamic
    performance, establish geometry of flow path components,
    and perform trade studies required to evaluate the
    mechanical layout of the machine. Technical abilities
    include coordinating engine and turbomachinery interfaces;
    internal flow dynamics, heat transfer, rotordynamics,
    structural design, and material selection for all
    turbomachinery components especially high speed seals and
    bearings. Also includes component test planning, test
    integration, and data analysis.
  </skos:scopeNote>
  <nt2:status>Approved</nt2:status>
  <nt2:type>Descriptor</nt2:type>
  <nt2:inputdate>2006-12-13</nt2:inputdate>
  <dcterms:modified>2006-12-13</dcterms:modified>
  <nt2:code>1053</nt2:code>
 </skos:Concept>
 <skos:Concept rdf:about='urn:comp:1116'>
  <skos:prefLabel>Compensation</skos:prefLabel>
  <skos:altLabel>HCMCOMP</skos:altLabel>
  <skos:broader rdf:resource='urn:comp:128'/>
  <skos:scopeNote>Knowledge of compensation concepts, principles, and
    practices, including pay and leave administration and
    compensation flexibilities..
  </skos:scopeNote>
  <nt2:status>Approved</nt2:status>
  <nt2:type>Descriptor</nt2:type>
  <nt2:inputdate>2006-04-05</nt2:inputdate>
  <dcterms:dateAccepted>2006-04-05</dcterms:dateAccepted>
  <dcterms:modified>2006-12-18</dcterms:modified>
  <nt2:code>1116</nt2:code>
 </skos:Concept>
 <skos:Concept rdf:about='urn:comp:1150'>
  <skos:prefLabel>Financial Operations Competency Suite</skos:prefLabel>
  <skos:broader rdf:resource='urn:comp:1124'/>
  <skos:narrower rdf:resource='urn:comp:124'/>
  <skos:narrower rdf:resource='urn:comp:119'/>
  <skos:narrower rdf:resource='urn:comp:121'/>
  <skos:narrower rdf:resource='urn:comp:118'/>
  <skos:narrower rdf:resource='urn:comp:120'/>
  <nt2:status>Approved</nt2:status>
  <nt2:type>Descriptor</nt2:type>
  <nt2:inputdate>2006-12-13</nt2:inputdate>
  <dcterms:modified>2006-12-13</dcterms:modified>
  <nt2:code>1150</nt2:code>
 </skos:Concept>
 <skos:Concept rdf:about='urn:comp:1071'>
  <skos:prefLabel>Behavioral Health</skos:prefLabel>
  <skos:altLabel>MDBEHAVIOR</skos:altLabel>
  <skos:broader rdf:resource='urn:comp:36'/>
  <skos:scopeNote>Knowledge and expertise of psychology/psychiatry in
    aviation and operational settings to maintain health and
    performance of crewmembers and appropriate associated
    personnel during all mission phases. Knowledge and skills
    of clinical and operational psychiatry, clinical, aviation
    or organizational psychology, psychosocial psychology,
    behavioral health maintenance, human systems interfaces and
    astronaut selection and training.
  </skos:scopeNote>
  <nt2:status>Approved</nt2:status>
  <nt2:type>Descriptor</nt2:type>
  <nt2:inputdate>2006-12-13</nt2:inputdate>
  <dcterms:modified>2006-12-13</dcterms:modified>
  <nt2:code>1071</nt2:code>
 </skos:Concept>
 <skos:Concept rdf:about='urn:comp:75'>
  <skos:prefLabel>Power Systems</skos:prefLabel>
  <skos:altLabel>PWRSYS</skos:altLabel>
  <skos:broader rdf:resource='urn:comp:1314'/>
  <skos:scopeNote>Applies knowledge and capabilities involved in the design,
    development, test, and evaluation of hardware for power
    generation, storage, conditioning and distribution for all
    vehicles, spacecraft, and experiments. Inherent within this
    is a broad knowledge of power sources and technologies and
    the ability to develop power architectures and integrate
    all elements into networked systems tailored to their
    specific environments. Also includes development, test and
    evaluation of the impact of environments and material on
    power systems.
  </skos:scopeNote>
  <nt2:status>Approved</nt2:status>
  <nt2:type>Descriptor</nt2:type>
  <nt2:inputdate>2006-12-13</nt2:inputdate>
  <dcterms:modified>2006-12-13</dcterms:modified>
  <nt2:code>75</nt2:code>
 </skos:Concept>
 <skos:Concept rdf:about='urn:comp:1094'>
  <skos:prefLabel>Contract Formation</skos:prefLabel>
  <skos:altLabel>CONFORMAT</skos:altLabel>
  <skos:broader rdf:resource='urn:comp:124'/>
  <skos:scopeNote>Knowledge of contract regulations and government contract
    vehicles, and ability to form contracts through source
    selection planning, identifying solicitation terms and
    conditions, and identifying and selecting techniques for
    determining price reasonableness. Also includes ability to
    recognize factors to be considered when evaluating and
    providing government financing, conducting price analyses,
    negotiating, identifying actions to resolve protests, and
    contract awarding.
  </skos:scopeNote>
  <nt2:status>Approved</nt2:status>
  <nt2:type>Descriptor</nt2:type>
  <nt2:inputdate>2006-12-13</nt2:inputdate>
  <dcterms:modified>2006-12-13</dcterms:modified>
  <nt2:code>1094</nt2:code>
 </skos:Concept>
 <skos:Concept rdf:about='urn:comp:174'>
  <skos:prefLabel>Student Trainee</skos:prefLabel>
  <skos:altLabel>STUDENT</skos:altLabel>
  <skos:broader rdf:resource='urn:comp:1189'/>
  <skos:narrower rdf:resource='urn:comp:1102'/>
  <skos:narrower rdf:resource='urn:comp:1103'/>
  <skos:narrower rdf:resource='urn:comp:1101'/>
  <skos:scopeNote>This is a training and development competency for employees
    who are classified as Student Trainees. It is a generic
    competency that is intended to be used to help simplify the
    workforce planning process so tat students will be
    correctly identified and planned for during the workforce
    competency needs assesmement. Reference the Business Rules
    section in this document for further clarification.
  </skos:scopeNote>
  <nt2:status>Approved</nt2:status>
  <nt2:type>Descriptor</nt2:type>
  <nt2:inputdate>2005-12-07</nt2:inputdate>
  <dcterms:dateAccepted>2005-12-07</dcterms:dateAccepted>
  <dcterms:modified>2006-12-18</dcterms:modified>
  <nt2:code>174</nt2:code>
 </skos:Concept>
 <skos:Concept rdf:about='urn:comp:135'>
  <skos:prefLabel>Public Communications &amp; Outreach</skos:prefLabel>
  <skos:altLabel>PUBLICOMM</skos:altLabel>
  <skos:broader rdf:resource='urn:comp:1125'/>
  <skos:scopeNote>Knowledge, capabilities and practices associated with the
    assessment, development and execution of public
    communication and outreach efforts. Knowledge of effective
    public relations and presentation techniques for
    representing and expressing the views, work operations and
    policies of NASA including liaising with and presenting
    information to a variety of external audiences. Effectively
    advocates for the Agency through communication of the
    organization's expertise and contributions, and assessing
    the effectiveness of past or ongoing efforts. Apply
    principles and practices of domestic and international
    customs, regulations and details to ceremonies or other
    interaction with distinguished visitors or in public
    forums. Manage Agency knowledge so it can be accessed where
    and when needed for communication purposes inside and
    outside the Agency. This includes public writing and
    speaking, information collection and dissemination, news
    broadcasting and writing, media relations, exhibit design,
    story development, visitor and guest programs, protocols,
    and concessionaire management.
  </skos:scopeNote>
  <nt2:status>Approved</nt2:status>
  <nt2:type>Descriptor</nt2:type>
  <nt2:inputdate>2006-12-13</nt2:inputdate>
  <dcterms:modified>2006-12-13</dcterms:modified>
  <nt2:code>135</nt2:code>
 </skos:Concept>
 <skos:Concept rdf:about='urn:comp:1314'>
  <skos:prefLabel>Power &amp; Propulsion Competency Suite</skos:prefLabel>
  <skos:broader rdf:resource='urn:comp:1208'/>
  <skos:narrower rdf:resource='urn:comp:72'/>
  <skos:narrower rdf:resource='urn:comp:69'/>
  <skos:narrower rdf:resource='urn:comp:74'/>
  <skos:narrower rdf:resource='urn:comp:71'/>
  <skos:narrower rdf:resource='urn:comp:70'/>
  <skos:narrower rdf:resource='urn:comp:138'/>
  <skos:narrower rdf:resource='urn:comp:76'/>
  <skos:narrower rdf:resource='urn:comp:77'/>
  <skos:narrower rdf:resource='urn:comp:78'/>
  <skos:narrower rdf:resource='urn:comp:75'/>
  <skos:narrower rdf:resource='urn:comp:68'/>
  <skos:narrower rdf:resource='urn:comp:73'/>
  <nt2:status>Approved</nt2:status>
  <nt2:type>Descriptor</nt2:type>
  <nt2:inputdate>2006-12-13</nt2:inputdate>
  <dcterms:modified>2006-12-13</dcterms:modified>
  <nt2:code>1314</nt2:code>
 </skos:Concept>
 <skos:Concept rdf:about='urn:comp:1075'>
  <skos:prefLabel>National Security Systems</skos:prefLabel>
  <skos:altLabel>SECNATION</skos:altLabel>
  <skos:broader rdf:resource='urn:comp:126'/>
  <skos:scopeNote>Knowledge, capabilities and practices associated with
    researching and implementing national security systems used
    for transmitting national security information, including
    classified and sensitive unclassified information
    technology systems and programs involving secure voice,
    data, video, and facsimile to include ground-to-ground,
    space-to-space, and ground-to-space communications assets.
  </skos:scopeNote>
  <nt2:status>Approved</nt2:status>
  <nt2:type>Descriptor</nt2:type>
  <nt2:inputdate>2006-12-13</nt2:inputdate>
  <dcterms:modified>2006-12-13</dcterms:modified>
  <nt2:code>1075</nt2:code>
 </skos:Concept>
 <skos:Concept rdf:about='urn:comp:1046'>
  <skos:prefLabel>Spacecraft &amp; Stabilization Control Design and Analysis</skos:prefLabel>
  <skos:altLabel>GNCSPACE</skos:altLabel>
  <skos:broader rdf:resource='urn:comp:22'/>
  <skos:scopeNote>Knowledge of and ability to conduct research and develop
    analytical, computational, and experimental methods for
    control algorithm and control mechnism design and
    development for space vehicles, space systems and
    subsystems. Appliction of research and or trade studies to
    develop requirements for control mechanisms, sensors and
    instrumentation systems; establish functional, performance,
    design, analysis, test, integration and verification
    requirements for in-space control systems and precision
    pointing and stabilization systems, subsystems, control
    mechanisms and components. Competency includes the use
    analytical modeling and simulation tools that determine
    control system solutions, along with the knowledge of
    research and engineering of integrated space vehicle systems
    for spacecraft control and health management of flight
    vehicles in diverse space environments. Includes knowledge
    of sensors, avionics, actuation and control mechanisms,
    large space structure dynamics, mathematical modeling,
    interplanetary environmental models, experimental methods
    and a broad array of engineering disciplines.
  </skos:scopeNote>
  <nt2:status>Approved</nt2:status>
  <nt2:type>Descriptor</nt2:type>
  <nt2:inputdate>2006-12-13</nt2:inputdate>
  <dcterms:modified>2006-12-13</dcterms:modified>
  <nt2:code>1046</nt2:code>
 </skos:Concept>
 <skos:Concept rdf:about='urn:comp:1083'>
  <skos:prefLabel>Intellectual Property Law</skos:prefLabel>
  <skos:altLabel>INTPROPLAW</skos:altLabel>
  <skos:broader rdf:resource='urn:comp:125'/>
  <skos:changeNote>???
  </skos:changeNote>
  <skos:scopeNote>Speciaized knowledge of matter related to intellectual
    property, including but not limited to patents, copyrights,
    data rights, trademarks, and commercialization of
    technology. Be in good standing to practice before the
    United States Patent and Trademark Office.
  </skos:scopeNote>
  <nt2:status>Approved</nt2:status>
  <nt2:type>Descriptor</nt2:type>
  <nt2:inputdate>2006-12-13</nt2:inputdate>
  <dcterms:dateAccepted>2006-04-05</dcterms:dateAccepted>
  <dcterms:modified>2006-12-18</dcterms:modified>
  <nt2:code>1083</nt2:code>
 </skos:Concept>
 <skos:Concept rdf:about='urn:comp:1363'>
  <skos:prefLabel>Multi-disciplinary R&amp;D Competency Suite</skos:prefLabel>
  <skos:broader rdf:resource='urn:comp:1208'/>
  <skos:narrower rdf:resource='urn:comp:91'/>
  <skos:narrower rdf:resource='urn:comp:109'/>
  <skos:narrower rdf:resource='urn:comp:111'/>
  <skos:narrower rdf:resource='urn:comp:86'/>
  <skos:narrower rdf:resource='urn:comp:57'/>
  <skos:narrower rdf:resource='urn:comp:155'/>
  <skos:narrower rdf:resource='urn:comp:WQQ-470'/>
  <skos:narrower rdf:resource='urn:comp:WQQ-471'/>
  <nt2:status>Approved</nt2:status>
  <nt2:type>Descriptor</nt2:type>
  <nt2:inputdate>2006-12-13</nt2:inputdate>
  <dcterms:modified>2006-12-13</dcterms:modified>
  <nt2:code>1363</nt2:code>
 </skos:Concept>
 <skos:Concept rdf:about='urn:comp:1010'>
  <skos:prefLabel>Cognitive Science Fundamental Research</skos:prefLabel>
  <skos:altLabel>HFRCOG</skos:altLabel>
  <skos:broader rdf:resource='urn:comp:40'/>
  <skos:scopeNote>TBD (includes memory, attention, task processing, etc.)
  </skos:scopeNote>
  <nt2:status>Approved</nt2:status>
  <nt2:type>Descriptor</nt2:type>
  <nt2:inputdate>2006-12-13</nt2:inputdate>
  <dcterms:modified>2006-12-13</dcterms:modified>
  <nt2:code>1010</nt2:code>
 </skos:Concept>
 <skos:Concept rdf:about='urn:comp:176'>
  <skos:prefLabel>Legal Assistance</skos:prefLabel>
  <skos:altLabel>LEGALSUP</skos:altLabel>
  <skos:broader rdf:resource='urn:comp:1125'/>
  <skos:narrower rdf:resource='urn:comp:1082'/>
  <skos:narrower rdf:resource='urn:comp:1114'/>
  <skos:scopeNote>Other knowledge of legal research and writing, litigation
    case management, and providing professional administrative
    and technical legal support, not otherwise categorized.
  </skos:scopeNote>
  <nt2:status>Approved</nt2:status>
  <nt2:type>Descriptor</nt2:type>
  <nt2:inputdate>2006-12-13</nt2:inputdate>
  <dcterms:dateAccepted>2006-04-05</dcterms:dateAccepted>
  <dcterms:modified>2006-12-18</dcterms:modified>
  <nt2:code>176</nt2:code>
 </skos:Concept>
 <skos:Concept rdf:about='urn:comp:32'>
  <skos:prefLabel>Developmental Biology</skos:prefLabel>
  <skos:altLabel>DEVELOPBIO</skos:altLabel>
  <skos:broader rdf:resource='urn:comp:1430'/>
  <skos:scopeNote>Knowledge of and ability to conduct research on the
    processes of development, differentiation, and growth in
    animals and plants at the molecular, cellular, and genetic
    levels.
  </skos:scopeNote>
  <nt2:status>Approved</nt2:status>
  <nt2:type>Descriptor</nt2:type>
  <nt2:inputdate>2006-12-13</nt2:inputdate>
  <dcterms:modified>2006-12-13</dcterms:modified>
  <nt2:code>32</nt2:code>
 </skos:Concept>
 <skos:Concept rdf:about='urn:comp:1035'>
  <skos:prefLabel>Electrical Integration Engineering</skos:prefLabel>
  <skos:altLabel>INTELECT</skos:altLabel>
  <skos:broader rdf:resource='urn:comp:9'/>
  <skos:scopeNote>Knowledge and capability to integrate electrical components
    for air, space and ground systems and instruments into a
    functioning system or subsystems such as complex flight to
    flight, flight to ground, and facilities systems. Includes
    knowledge and capabilities required for safe and reliable
    integration of electrical systems, schedules,
    configurations, and electrical resources including power
    generation, control, and storage; controls and
    instrumentation; communications and data management; and
    electrical packaging, as well as the development of
    electrical and electronic systems impacts to launch,
    mission, manifest, contingency and long-range plans, and
    responses to externally-driven requirements.
  </skos:scopeNote>
  <nt2:status>Approved</nt2:status>
  <nt2:type>Descriptor</nt2:type>
  <nt2:inputdate>2006-12-13</nt2:inputdate>
  <dcterms:modified>2006-12-13</dcterms:modified>
  <nt2:code>1035</nt2:code>
 </skos:Concept>
 <skos:Concept rdf:about='urn:comp:163'>
  <skos:prefLabel>Planetary Atmospheres</skos:prefLabel>
  <skos:altLabel>PLANETATM</skos:altLabel>
  <skos:broader rdf:resource='urn:comp:1407'/>
  <skos:scopeNote>Knowledge of the fundamental processes of radiation,
    chemistry and dynamics in the study of the structure and
    conposition of the lower and upper atmosphiere of the
    panets and the origin and evolution of planetary
    atmospheres. Conceive and implement a variety of
    observational methods to characterize the state of the
    atmospheres of the planets-past and present, detect
    variability and explain the responsible forcing mechanisms,
    and predict the future evolution and state of planetary
    atmospheres instrument and tnd sensor development. Includes
    subspeciality knowledge in areas such as Radiation and
    Climate, Atmospheric Chemistry and Dynamics,
    Atmosphere-Surface Interactions, CelestialMechanics,
    Solar-Planetary Relationships, Planetary Magnetic Fields
    and Magnetospheres.
  </skos:scopeNote>
  <nt2:status>Approved</nt2:status>
  <nt2:type>Descriptor</nt2:type>
  <nt2:inputdate>2006-12-13</nt2:inputdate>
  <dcterms:modified>2006-12-13</dcterms:modified>
  <nt2:code>163</nt2:code>
 </skos:Concept>
 <skos:Concept rdf:about='urn:comp:67'>
  <skos:prefLabel>Non-destructive Evaluation Sciences</skos:prefLabel>
  <skos:altLabel>NONDESSCI</skos:altLabel>
  <skos:broader rdf:resource='urn:comp:1347'/>
  <skos:scopeNote>Research knowledge, capabilities, and practices for
    developing and applying advanced sensors, health monitoring
    technologies, computational techniques, and NonDestructive
    Evaluation (NDE) methodologies, e.g., x-ray, ultrasonic,
    eddy current inspection, to characterize advanced materials
    and structures, for developing intelligent, autonomous
    micro and nano-methods for characterization, health
    monitoring, control, and self-repair of aerospace systems,
    and for developing techniques and concepts for
    nondestructive flaw detection, manufacturing process
    control sensing, and instrument system miniaturization.
  </skos:scopeNote>
  <nt2:status>Approved</nt2:status>
  <nt2:type>Descriptor</nt2:type>
  <nt2:inputdate>2006-12-13</nt2:inputdate>
  <dcterms:modified>2006-12-13</dcterms:modified>
  <nt2:code>67</nt2:code>
 </skos:Concept>
 <skos:Concept rdf:about='urn:comp:1003'>
  <skos:prefLabel>Work Performance Leadership</skos:prefLabel>
  <skos:altLabel>LEADWORK</skos:altLabel>
  <skos:broader rdf:resource='urn:comp:140'/>
  <skos:scopeNote>Knowledge, capabilities and practices associated with
    determining an organization’s business direction and
    vision, and setting goals that align with broader Agency
    objectives and related functional or program plans.
    Knowledge of how to apply policies and regulations that
    impact NASA including NASA Strategic Plan, President’s
    Management Agenda, Space Act, and GPRA. Ability to assess
    impact of work performance on NASA’s relationship with
    external customers and stakeholders. Ability to develop
    systems that facilitate the effective assignment of work
    and measurement of results. Knowledge of methods for
    integrating work from across functional and organizational
    boundaries.
  </skos:scopeNote>
  <nt2:status>Approved</nt2:status>
  <nt2:type>Descriptor</nt2:type>
  <nt2:inputdate>2006-12-13</nt2:inputdate>
  <dcterms:modified>2006-12-13</dcterms:modified>
  <nt2:code>1003</nt2:code>
 </skos:Concept>
 <skos:Concept rdf:about='urn:comp:1189'>
  <skos:prefLabel>Workforce Operations &amp; Support Competency Suite</skos:prefLabel>
  <skos:broader rdf:resource='urn:comp:1124'/>
  <skos:narrower rdf:resource='urn:comp:158'/>
  <skos:narrower rdf:resource='urn:comp:129'/>
  <skos:narrower rdf:resource='urn:comp:128'/>
  <skos:narrower rdf:resource='urn:comp:165'/>
  <skos:narrower rdf:resource='urn:comp:115'/>
  <skos:narrower rdf:resource='urn:comp:174'/>
  <nt2:status>Approved</nt2:status>
  <nt2:type>Descriptor</nt2:type>
  <nt2:inputdate>2006-12-13</nt2:inputdate>
  <dcterms:modified>2006-12-13</dcterms:modified>
  <nt2:code>1189</nt2:code>
 </skos:Concept>
 <skos:Concept rdf:about='urn:comp:170'>
  <skos:prefLabel>Executive Management</skos:prefLabel>
  <skos:altLabel>EXECMMT</skos:altLabel>
  <skos:broader rdf:resource='urn:comp:1394'/>
  <skos:scopeNote>Knowledge, capabilities and practices associated with
    leading change, people, and work of an organization.
    Includes awareness and understanding of relevant strategies
    and techniques to effectively create a vision for change
    and engage others in implementing the change process.
    Ability to apply human capital and leadership strategies to
    empower teams and develop leadership capabilities in lower
    level managers. Ability to determine an organization’s
    business direction and vision, and set goals that align
    with broader Agency objectives and related functional or
    program plans. Knowledge of methods for integrating work
    from across functional and organizational boundaries,
    considering complex cross-functional, cross-center,
    division, business and geographic implications when
    approaching problems or issues. Knowledge of how to apply
    policies and regulations that impact NASA including NASA
    Strategic Plan, Mission Directorate Roadmaps, President’s
    Management Agenda, Space Act, and GPRA. Ability to assess
    impact of work performance on NASA’s relationships with
    external customers and stakeholders.
  </skos:scopeNote>
  <nt2:status>Approved</nt2:status>
  <nt2:type>Descriptor</nt2:type>
  <nt2:inputdate>2006-12-13</nt2:inputdate>
  <dcterms:modified>2006-12-13</dcterms:modified>
  <nt2:code>170</nt2:code>
 </skos:Concept>
 <skos:Concept rdf:about='urn:comp:7'>
  <skos:prefLabel>Systems Engineering</skos:prefLabel>
  <skos:altLabel>SYSTEMSENG</skos:altLabel>
  <skos:broader rdf:resource='urn:comp:1209'/>
  <skos:scopeNote>Knowledge, capabilities and practices associated with
    defining, developing, integrating and verifying an
    end-to-end new or existing system, with the objective of
    optimizing performance, safety and mission objectives.
    Includes knowledge required for safe and reliable system
    development/integration. Ability to perform feasibility
    assessments, provide functional analyses; develop and
    manage system performance and interface requirements to
    ensure the resulting system meets all technical objectives;
    perform systems analysis and trade studies, and oversee
    systems integration and verification. Includes knowledge of
    system engineering tools and procedures such as
    configuration management, integrated logistics management,
    risk management, and documents such as integrated
    schematics, interface control documents, and interface
    requirements documents for defining interconnection of
    system parts, documenting and managing system
    configurations and identifying all required interfaces, and
    mass properties for determining weight distributions.
    Assumes a breadth of knowledge of many specialty areas, and
    a detailed understanding of how the pieces fit together.
    Thorough knowledge of the NASA process of reviews, audits,
    and control gates to ensure all technical and programmatic
    requirements are being met in an organized fashion.
  </skos:scopeNote>
  <nt2:status>Approved</nt2:status>
  <nt2:type>Descriptor</nt2:type>
  <nt2:inputdate>2006-12-13</nt2:inputdate>
  <dcterms:modified>2006-12-13</dcterms:modified>
  <nt2:code>7</nt2:code>
 </skos:Concept>
 <skos:Concept rdf:about='urn:comp:51'>
  <skos:prefLabel>Space Physics</skos:prefLabel>
  <skos:altLabel>SPACEPHY</skos:altLabel>
  <skos:broader rdf:resource='urn:comp:1407'/>
  <skos:scopeNote>Uses knowledge to conduct experimental, theoretical, and/or
    applied physics and modeling relating to matter, radiation,
    and their interactions, and ranging from elementary
    particles and fields to atomic, and nuclear physics,
    condensed matter physics, optical, gravitational and
    quantum mechanical, hydrodynamical and
    magnetohydrodynamical physics and General Relativity, and
    as applied to the nature and structure of the universe and
    to chemical, biological, and geophysical systems. Includes
    specialty areas such as solar physics, involving use of
    observational and experimental studies to model the Sun and
    its magnetic activity, characteristics, composition and
    influence on the Earth and other planetary bodies, as well
    as space plasma physics, focused on near-Earth environments
    such as the magnetosphere and its properties.
  </skos:scopeNote>
  <nt2:status>Approved</nt2:status>
  <nt2:type>Descriptor</nt2:type>
  <nt2:inputdate>2006-12-13</nt2:inputdate>
  <dcterms:modified>2006-12-13</dcterms:modified>
  <nt2:code>51</nt2:code>
 </skos:Concept>
 <skos:Concept rdf:about='urn:comp:1045'>
  <skos:prefLabel>Electrical Circuits Engineering</skos:prefLabel>
  <skos:altLabel>ELCIRCUITS</skos:altLabel>
  <skos:broader rdf:resource='urn:comp:13'/>
  <skos:scopeNote>Knowledge of, and capability to perform, engineering design
    and analysis, development and research of electrical
    circuits components, subsystems, and systems for air, space
    and ground systems and instruments. Includes knowledge of
    electrical cable design, development, and testing;
    electrical power distribution requirements and design;
    electrical packaging integration; subsystem and circuit
    analysis; test procedure development and safety analysis;
    reliability and environmental effects; and knowledge of
    thermal analysis of printed circuit boards and subsequent
    use of thermal data to optimize flight electronics design.
  </skos:scopeNote>
  <nt2:status>Approved</nt2:status>
  <nt2:type>Descriptor</nt2:type>
  <nt2:inputdate>2006-12-13</nt2:inputdate>
  <dcterms:modified>2006-12-13</dcterms:modified>
  <nt2:code>1045</nt2:code>
 </skos:Concept>
 <skos:Concept rdf:about='urn:comp:123'>
  <skos:prefLabel>Risk Management</skos:prefLabel>
  <skos:altLabel>RISKMMT</skos:altLabel>
  <skos:broader rdf:resource='urn:comp:1381'/>
  <skos:scopeNote>Knowledge, capabilities and practices associated with the
    decision process associated with mitigating or accepting
    risks. This includes knowledge of fundamental risk
    management concepts, Continuous Risk Management (CRM)
    implementation in programs/projects, Risk-Based Acquisition
    Management (R-BAM) implementation for major procurements
    that require formal acquisition planning, and ongoing
    assessment of program/project risk management activities.
  </skos:scopeNote>
  <nt2:status>Approved</nt2:status>
  <nt2:type>Descriptor</nt2:type>
  <nt2:inputdate>2006-12-13</nt2:inputdate>
  <dcterms:modified>2006-12-13</dcterms:modified>
  <nt2:code>123</nt2:code>
 </skos:Concept>
 <skos:Concept rdf:about='urn:comp:18'>
  <skos:prefLabel>Pyrotechnics</skos:prefLabel>
  <skos:altLabel>PYROTECH</skos:altLabel>
  <skos:broader rdf:resource='urn:comp:1280'/>
  <skos:scopeNote>Knowledge of the composition, nature, applications and
    handling of devices or assemblies containing or operated by
    propellants or explosives. Involves design and development
    of such systems for aerospace applications, as well as
    study of the safe operation and maintenance of the
    materials and systems. Includes knowledge of fluid and
    mechanics, thermodynamics, materials, chemistry and
    physics, structures, mechanical drawings, manufacturing
    processes and explosive material properties.
  </skos:scopeNote>
  <nt2:status>Approved</nt2:status>
  <nt2:type>Descriptor</nt2:type>
  <nt2:inputdate>2006-12-13</nt2:inputdate>
  <dcterms:modified>2006-12-13</dcterms:modified>
  <nt2:code>18</nt2:code>
 </skos:Concept>
 <skos:Concept rdf:about='urn:comp:1237'>
  <skos:prefLabel>Aeronautics Competency Suite</skos:prefLabel>
  <skos:broader rdf:resource='urn:comp:1208'/>
  <skos:narrower rdf:resource='urn:comp:103'/>
  <skos:narrower rdf:resource='urn:comp:101'/>
  <skos:narrower rdf:resource='urn:comp:100'/>
  <skos:narrower rdf:resource='urn:comp:102'/>
  <skos:narrower rdf:resource='urn:comp:108'/>
  <skos:narrower rdf:resource='urn:comp:98'/>
  <skos:narrower rdf:resource='urn:comp:110'/>
  <nt2:status>Approved</nt2:status>
  <nt2:type>Descriptor</nt2:type>
  <nt2:inputdate>2006-12-13</nt2:inputdate>
  <dcterms:modified>2006-12-13</dcterms:modified>
  <nt2:code>1237</nt2:code>
 </skos:Concept>
 <skos:Concept rdf:about='urn:comp:1318'>
  <skos:prefLabel>Propellantless Propulsion(APNOPROP) [1051]</skos:prefLabel>
  <skos:broader rdf:resource='urn:comp:72'/>
  <skos:scopeNote>Research, development, design, testing and evaluation of
    in-space propulsion systems which use technologies other
    than discharge of a propellant to gain motive force (i.e.,
    non-rocket propulsion). Specialty knowledge in one or more
    categories of propellantless propulsion devices including
    solar sails, momentum exchange – electrodynamic reboost
    tethers, aerocapture, etc.
  </skos:scopeNote>
  <nt2:status>Approved</nt2:status>
  <nt2:type>Descriptor</nt2:type>
  <nt2:inputdate>2006-12-13</nt2:inputdate>
  <dcterms:modified>2006-12-13</dcterms:modified>
  <nt2:code>1318</nt2:code>
 </skos:Concept>
 <skos:Concept rdf:about='urn:comp:164'>
  <skos:prefLabel>Climate Change and Variability</skos:prefLabel>
  <skos:altLabel>CLIMATE</skos:altLabel>
  <skos:broader rdf:resource='urn:comp:1415'/>
  <skos:scopeNote>Applies an integrated and cross discipline approach to
    understanding, assessing, and predicting the Earth's
    complex climate system. This capability draws from the
    other Earth Sciences related competencies to provide
    observations at the high accuracy required to monitor
    climate change, to evaluate its component processes at
    climate relevant time and space scales, and to enable
    prediction of future climate change. This research
    capability includes the ability to estimate the uncertainty
    of future climate predictions, to support impact
    assessments, and to develop new climate observational and
    modeling requirements, methods, and capabilities.
  </skos:scopeNote>
  <nt2:status>Approved</nt2:status>
  <nt2:type>Descriptor</nt2:type>
  <nt2:inputdate>2006-12-13</nt2:inputdate>
  <dcterms:modified>2006-12-13</dcterms:modified>
  <nt2:code>164</nt2:code>
 </skos:Concept>
 <skos:Concept rdf:about='urn:comp:1109'>
  <skos:prefLabel>Liquid Engine Systems</skos:prefLabel>
  <skos:altLabel>LIQUIDENG</skos:altLabel>
  <skos:broader rdf:resource='urn:comp:73'/>
  <skos:scopeNote>Knowledge, capabilities, and practices associated with the
    design and analysis of complex liquid engine systems for
    rocket propulsion. Includes the ability to perform engine
    system requirements development and decomposition, trade
    studies and feasibility assessments, first order
    performance modeling, detailed and functional design,
    steady-state and transient performance analysis of liquid
    engine components, subsystems, and systems, and validation
    and verification of requirements through test and analysis
    to ensure the engine system meets mission requirements.
    Includes the capability to integrate engine components
    including turbomachinery, combustion devices, valves, and
    ducts and the ability to perform detailed calculations and
    analyses to ensure the design met its intended objectives.
    Includes the knowledge and skills associated with
    propulsion system test formulation, analytical prediction,
    and data analysis and reduction including identifying
    appropriate test methods and techiques, test plan
    formulation, test article design, test matrix development,
    identification of special instrumentation, end-to-end
    systems and transient modelling, and test facility
    requirements necessary to conduct propulsion system
    testing. Includes test data assessment and data evaluation
    to assess potential conceptual designs, to anchor
    mathematical models, or to ensure functional performance
    and identify design deficienies of as-designed propulsion
    systems over all flight / ground test regimes. Includes
    knowledge of the systems engineering tools, processes, and
    procedures that are required to ensure safe and reliable
    engine system development and integration.
  </skos:scopeNote>
  <nt2:status>Approved</nt2:status>
  <nt2:type>Descriptor</nt2:type>
  <nt2:inputdate>2006-12-13</nt2:inputdate>
  <dcterms:modified>2006-12-13</dcterms:modified>
  <nt2:code>1109</nt2:code>
 </skos:Concept>
 <skos:Concept rdf:about='urn:comp:71'>
  <skos:prefLabel>Hypergolic Systems</skos:prefLabel>
  <skos:altLabel>HYPERSYS</skos:altLabel>
  <skos:broader rdf:resource='urn:comp:1314'/>
  <skos:scopeNote>Knowledge, capabilities and practices associated with
    hypergolic propellants and propulsion systems. This
    includes handling characteristics, material properties,
    system safety, and system unique requirements for the safe
    and effective test, implementation, and operation of
    hypergolic systems for research, development, design,
    analysis, testing and/or evaluation.
  </skos:scopeNote>
  <nt2:status>Approved</nt2:status>
  <nt2:type>Descriptor</nt2:type>
  <nt2:inputdate>2006-12-13</nt2:inputdate>
  <dcterms:modified>2006-12-13</dcterms:modified>
  <nt2:code>71</nt2:code>
 </skos:Concept>
 <skos:Concept rdf:about='urn:comp:1104'>
  <skos:prefLabel>System Safety</skos:prefLabel>
  <skos:altLabel>SYSSAFETY</skos:altLabel>
  <skos:broader rdf:resource='urn:comp:27'/>
  <skos:scopeNote>Knowledge, capabilities and practices associated with the
    use of formal approaches to analyze hazards that impact
    human, environment and mission assets in order to provide
    decision makers with recommendations on ways to eliminate
    the hazards or reduce their risk to acceptable levels.
    Involves the ability to develop safety risk models using
    qualitative techniques such as System Hazard Analysis (SHA)
    and quantitative techniques such as Probabilistic Risk
    Assessment (PRA); to proactively and reactively identify
    the need for risk trade studies concerning resolution of
    hazards; to formulate risk reduction strategies; and to
    timely and effectively communicate safety risk insights to
    decision-makers.
  </skos:scopeNote>
  <nt2:status>Approved</nt2:status>
  <nt2:type>Descriptor</nt2:type>
  <nt2:inputdate>2005-12-07</nt2:inputdate>
  <dcterms:dateAccepted>2005-12-07</dcterms:dateAccepted>
  <dcterms:modified>2006-12-18</dcterms:modified>
  <nt2:code>1104</nt2:code>
 </skos:Concept>
 <skos:Concept rdf:about='urn:comp:65'>
  <skos:prefLabel>Advanced Materials and Processing Science</skos:prefLabel>
  <skos:altLabel>ADVMATSCI</skos:altLabel>
  <skos:broader rdf:resource='urn:comp:1424'/>
  <skos:scopeNote>Research knowledge, capabilities and practices associated
    with the synthesis, structure, processing and properties of
    materials, from atomic to macroscopic, including the
    behavior and mechanisms by which types of materials react
    to stresses, processes and environments, particularly the
    harsh environment of space. Includes experimental research
    into materials such as electronic materials, glasses and
    ceramics, metals and alloys, lubrication materials,
    sealants, foams, composites and polymers for improving
    current and enabling future aerospace applications.
    Includes computational research to develop validated
    structure-property relationship models for all classes of
    materials. Includes processing, testing, and characterizing
    these materials to further understanding of how they can be
    combined or treated to improve the quality and reliability
    of systems, control defects and prevent contamination of
    operating systems or components.
  </skos:scopeNote>
  <nt2:status>Approved</nt2:status>
  <nt2:type>Descriptor</nt2:type>
  <nt2:inputdate>2006-12-13</nt2:inputdate>
  <dcterms:modified>2006-12-13</dcterms:modified>
  <nt2:code>65</nt2:code>
 </skos:Concept>
 <skos:Concept rdf:about='urn:comp:1090'>
  <skos:prefLabel>Facility Civil Engineering</skos:prefLabel>
  <skos:altLabel>FACIVENG</skos:altLabel>
  <skos:broader rdf:resource='urn:comp:112'/>
  <skos:scopeNote>Knowledge of building and foundation design and
    construction, concrete and steel design and construction as
    well as design and construction of roads, utilities, and
    other civil projects for aerospace facility programs.
    Requires understanding of energy management and
    sustainability standards for sustainable design. Also
    requires knowledge of construction contracting and
    contractor oversight and contracts management.
  </skos:scopeNote>
  <nt2:status>Approved</nt2:status>
  <nt2:type>Descriptor</nt2:type>
  <nt2:inputdate>2006-12-13</nt2:inputdate>
  <dcterms:modified>2006-12-13</dcterms:modified>
  <nt2:code>1090</nt2:code>
 </skos:Concept>
 <skos:Concept rdf:about='urn:comp:165'>
  <skos:prefLabel>Para-Professional Business Operations</skos:prefLabel>
  <skos:altLabel>PARABUSOPS</skos:altLabel>
  <skos:broader rdf:resource='urn:comp:1189'/>
  <skos:scopeNote>The knowledge and capabilities associated with
    administrative, clerical and management support to a
    manager and/or organization to facilitate the mission,
    goals and customer satisfaction. This competency requires
    knowledge of policies, procedures and tools to implement
    operations within a business environment such as scheduling
    of meetings, office communication and document generation
    with the organization.
  </skos:scopeNote>
  <nt2:status>Approved</nt2:status>
  <nt2:type>Descriptor</nt2:type>
  <nt2:inputdate>2006-12-13</nt2:inputdate>
  <dcterms:modified>2006-12-13</dcterms:modified>
  <nt2:code>165</nt2:code>
 </skos:Concept>
 <skos:Concept rdf:about='urn:comp:1058'>
  <skos:prefLabel>Analytical and computational Fluid Mechanics</skos:prefLabel>
  <skos:altLabel>RPFLUIDMCH</skos:altLabel>
  <skos:broader rdf:resource='urn:comp:73'/>
  <skos:scopeNote>Knowledge, capabilities and practices associated with the
    development, validation, and application of Computational
    Fluid Dynamics (CFD) techniques and codes for tanks, ducts,
    valves, turbomachinery, and combustion components as
    commonly found in chemical propulsion systems (solid,
    liquid, and gas propellants). This involves expertise in
    high fidelity numerical simulation of internal flows that
    involve finite-rate chemistry, multiple phases, cavitation,
    unsteadiness, turbulence, a large range in fluid Mach
    number, and relative motion between elements in the
    simulation. Includes the pursuit of experimental research
    and technology projects related to obtaining data for model
    validation and for demonstrating advanced fluid design
    concepts. Requires working knoweledge of thermal and
    structural dynamisc modeling in order to properly provide
    output of tasks to these other disciplines.
  </skos:scopeNote>
  <nt2:status>Approved</nt2:status>
  <nt2:type>Descriptor</nt2:type>
  <nt2:inputdate>2006-12-13</nt2:inputdate>
  <dcterms:modified>2006-12-13</dcterms:modified>
  <nt2:code>1058</nt2:code>
 </skos:Concept>
 <skos:Concept rdf:about='urn:comp:68'>
  <skos:prefLabel>Propulsion Systems &amp; Testing</skos:prefLabel>
  <skos:altLabel>PROSYS</skos:altLabel>
  <skos:broader rdf:resource='urn:comp:1314'/>
  <skos:scopeNote>Knowledge of conceptual aeropropulsion and aviation systems
    analysis and testing to assess the benefits of
    aeropropulsion systems, subsystems and components over all
    flight regimes from general aviation through space access.
    Knowledge of the integration of component technologies into
    conceptual systems. Includes research, design, testing, and
    evaluation of components systems such as combustors,
    inlets, nozzles, and turbomachinery, emissions, engine
    materials and structures, propulsion controls, and
    propulsion airframe integration. Knowledge of advanced,
    distributed instrumentation for acquiring improved
    information in a hostile engine environment. Experience in
    advanced methods for safe and affordable rocket propellant
    aeropropulsion systems testing.
  </skos:scopeNote>
  <nt2:status>Approved</nt2:status>
  <nt2:type>Descriptor</nt2:type>
  <nt2:inputdate>2006-12-13</nt2:inputdate>
  <dcterms:modified>2006-12-13</dcterms:modified>
  <nt2:code>68</nt2:code>
 </skos:Concept>
 <skos:Concept rdf:about='urn:comp:36'>
  <skos:prefLabel>Aerospace Medicine</skos:prefLabel>
  <skos:altLabel>AEROMED</skos:altLabel>
  <skos:broader rdf:resource='urn:comp:1244'/>
  <skos:narrower rdf:resource='urn:comp:1071'/>
  <skos:narrower rdf:resource='urn:comp:1070'/>
  <skos:scopeNote>Knowledge, capabilities, and credentials to engage,
    determine, and maintain and provide for the physical and
    behavioral health, and medical care of crew members, their
    families, and associated personnel during all mission
    phases (pre-flight, in-flight and post-flight) in the
    diverse environments of atmospheric and space flight
    missions.
  </skos:scopeNote>
  <nt2:status>Approved</nt2:status>
  <nt2:type>Descriptor</nt2:type>
  <nt2:inputdate>2006-12-13</nt2:inputdate>
  <dcterms:modified>2006-12-13</dcterms:modified>
  <nt2:code>36</nt2:code>
 </skos:Concept>
 <skos:Concept rdf:about='urn:comp:45'>
  <skos:prefLabel>Geophysical/Geologic Science</skos:prefLabel>
  <skos:altLabel>GEOSCI</skos:altLabel>
  <skos:broader rdf:resource='urn:comp:1415'/>
  <skos:scopeNote>Knowledge of a wide range of disciplines related to the
    earth's composition, its fluid envelopes, and its position
    in space. Apply concepts and methods in mathematics,
    physics, chemistry, and biology to the problems of the
    atmosphere, the oceans, the solid earth, and the evolution
    of the planet. Involves ability to conduct far-reaching
    studies of the origin of the earth and solar system.
  </skos:scopeNote>
  <nt2:status>Approved</nt2:status>
  <nt2:type>Descriptor</nt2:type>
  <nt2:inputdate>2006-12-13</nt2:inputdate>
  <dcterms:modified>2006-12-13</dcterms:modified>
  <nt2:code>45</nt2:code>
 </skos:Concept>
 <skos:Concept rdf:about='urn:comp:64'>
  <skos:prefLabel>Analytical and Computational Structural Methods</skos:prefLabel>
  <skos:altLabel>ACMSTR</skos:altLabel>
  <skos:broader rdf:resource='urn:comp:1347'/>
  <skos:scopeNote>Research knowledge, capability, and practices for
    developing computationally efficient methodologies for
    structural modeling, analysis, and design, for predicting
    response, damage tolerance, and residual strength of
    aerospace structures using nonlinear structural analysis
    methods and models, for developing validated finite element
    methods for special purpose computational methods including
    rapid optimal structural sizing, for developing analytical
    models for radiation protection and shielding, and for
    developing multi-sensory, visually immersive simulation and
    design methodologies for enhanced understanding and
    collaboration. Involves in-depth understanding of
    mathematics and computer science.
  </skos:scopeNote>
  <nt2:status>Approved</nt2:status>
  <nt2:type>Descriptor</nt2:type>
  <nt2:inputdate>2006-12-13</nt2:inputdate>
  <dcterms:modified>2006-12-13</dcterms:modified>
  <nt2:code>64</nt2:code>
 </skos:Concept>
 <skos:Concept rdf:about='urn:comp:17'>
  <skos:prefLabel>Mechanical Systems</skos:prefLabel>
  <skos:altLabel>MECHSYS</skos:altLabel>
  <skos:broader rdf:resource='urn:comp:1347'/>
  <skos:scopeNote>Knowledge, capability and practices involving the design,
    development and testing of vehicle and instrument
    structures, mechanisms deployment systems, associated
    mechanical ground support equipment and facilities
    structures. Includes knowledge of mechanical requirements
    development; mechanical system interfaces among
    instruments, subsystems, vehicle and ground systems;
    vehicle and instrument manufacturing and assembly; and
    vehicle and instrument alignment techniques and
    qualification testing. Includes knowledge of manufacturing
    techniques, materials, mechanical and materials standards,
    parametric computer aided design, mechanisms design, basic
    structural analysis, and knowledge of the state of best
    practice for complex mechanical systems.
  </skos:scopeNote>
  <nt2:status>Approved</nt2:status>
  <nt2:type>Descriptor</nt2:type>
  <nt2:inputdate>2006-12-13</nt2:inputdate>
  <dcterms:modified>2006-12-13</dcterms:modified>
  <nt2:code>17</nt2:code>
 </skos:Concept>
 <skos:Concept rdf:about='urn:comp:1118'>
  <skos:prefLabel>Employee Development</skos:prefLabel>
  <skos:altLabel>HCMEMPDEV</skos:altLabel>
  <skos:broader rdf:resource='urn:comp:128'/>
  <skos:scopeNote>Knowledge of employee development concepts, principles, and
    practices related to planning, evaluating,and
    administering training, organizational development, and
    career development initiatives.
  </skos:scopeNote>
  <nt2:status>Approved</nt2:status>
  <nt2:type>Descriptor</nt2:type>
  <nt2:inputdate>2006-04-05</nt2:inputdate>
  <dcterms:dateAccepted>2006-04-05</dcterms:dateAccepted>
  <dcterms:modified>2006-12-18</dcterms:modified>
  <nt2:code>1118</nt2:code>
 </skos:Concept>
 <skos:Concept rdf:about='urn:comp:1111'>
  <skos:prefLabel>Control Electronics</skos:prefLabel>
  <skos:altLabel>GNCCTLELE</skos:altLabel>
  <skos:broader rdf:resource='urn:comp:22'/>
  <skos:scopeNote>Knowledge of and ability to employ navigation hardware
    including Inertial Measurement Unit’s (IMU: gyro and
    accelerometers), Global Position Satellite receivers, star
    trackers, sun sensors, etc. Knowledge of and skill in using
    Kalman filtering and other software techniques to merge
    data from different sources to obtain an accurate and
    optimum navigation solution. Skill in using the output
    navigation solution for orbit determination.
  </skos:scopeNote>
  <nt2:status>Approved</nt2:status>
  <nt2:type>Descriptor</nt2:type>
  <nt2:inputdate>2005-04-05</nt2:inputdate>
  <dcterms:dateAccepted>2006-04-05</dcterms:dateAccepted>
  <dcterms:modified>2006-12-18</dcterms:modified>
  <nt2:code>1111</nt2:code>
 </skos:Concept>
 <skos:Concept rdf:about='urn:comp:1084'>
  <skos:prefLabel>General Law</skos:prefLabel>
  <skos:altLabel>GENERALLAW</skos:altLabel>
  <skos:broader rdf:resource='urn:comp:125'/>
  <skos:changeNote>Modified ???
  </skos:changeNote>
  <skos:scopeNote>. Speciaized knowledge of matters related to civil and
    administrative law, including but not limited to fiscal and
    appropriations law, ethics, FOIA, torts, privacy issues,
    export control, immigration and foreign visitors, and
    litigation and appeals.
  </skos:scopeNote>
  <nt2:status>Approved</nt2:status>
  <nt2:type>Descriptor</nt2:type>
  <nt2:inputdate>2006-12-13</nt2:inputdate>
  <dcterms:dateAccepted>2006-04-05</dcterms:dateAccepted>
  <dcterms:modified>2006-12-18</dcterms:modified>
  <nt2:code>1084</nt2:code>
 </skos:Concept>
 <skos:Concept rdf:about='urn:comp:1359'>
  <skos:prefLabel>Thermal/Fluid Competency Suite</skos:prefLabel>
  <skos:broader rdf:resource='urn:comp:1208'/>
  <skos:narrower rdf:resource='urn:comp:26'/>
  <skos:narrower rdf:resource='urn:comp:106'/>
  <skos:narrower rdf:resource='urn:comp:104'/>
  <nt2:status>Approved</nt2:status>
  <nt2:type>Descriptor</nt2:type>
  <nt2:inputdate>2006-12-13</nt2:inputdate>
  <dcterms:modified>2006-12-13</dcterms:modified>
  <nt2:code>1359</nt2:code>
 </skos:Concept>
 <skos:Concept rdf:about='urn:comp:1072'>
  <skos:prefLabel>Physical Security</skos:prefLabel>
  <skos:altLabel>SECPHYSCL</skos:altLabel>
  <skos:broader rdf:resource='urn:comp:126'/>
  <skos:scopeNote>Knowledge, capabilities and practices associated with the
    protection of property and individuals from threats or
    adversarial influences. Abilities deal primarily with
    assessing risk, conducting surveys and implementing
    physical counter-measures designed to protect personnel
    from potential threats; prevent unauthorized access to
    equipment, facilities, material, and documents; and
    safeguard against espionage, sabotage, damage, and theft.
  </skos:scopeNote>
  <nt2:status>Approved</nt2:status>
  <nt2:type>Descriptor</nt2:type>
  <nt2:inputdate>2006-12-13</nt2:inputdate>
  <dcterms:modified>2006-12-13</dcterms:modified>
  <nt2:code>1072</nt2:code>
 </skos:Concept>
 <skos:Concept rdf:about='urn:comp:1438'>
  <skos:prefLabel>NASA Workforce Competencies</skos:prefLabel>
  <skos:narrower rdf:resource='urn:comp:1124'/>
  <skos:narrower rdf:resource='urn:comp:1208'/>
  <skos:narrower rdf:resource='urn:comp:1393'/>
  <skos:narrower rdf:resource='urn:comp:1371'/>
  <skos:narrower rdf:resource='urn:comp:1406'/>
  <skos:scopeNote>This facet is derived from the NASA Workforce Competency
    Dictionary, revision 6a, published April 17, 2006.
  </skos:scopeNote>
  <nt2:status>Approved</nt2:status>
  <nt2:type>Descriptor</nt2:type>
  <nt2:inputdate>2007-01-11</nt2:inputdate>
  <dcterms:dateAccepted>2006-04-17</dcterms:dateAccepted>
  <dcterms:modified>2007-01-11</dcterms:modified>
  <nt2:code>1438</nt2:code>
 </skos:Concept>
 <skos:Concept rdf:about='urn:comp:52'>
  <skos:prefLabel>Astronomy &amp; Astrophysics</skos:prefLabel>
  <skos:altLabel>ASTRONOMY</skos:altLabel>
  <skos:broader rdf:resource='urn:comp:1407'/>
  <skos:scopeNote>Knowledge of the fundamental processes of radiation and
    dynamics for the study of the structure and composition of
    the Solar System, other planetary systems, stars and
    stellar systems, galaxies, and the structure and evolution
    of matter and cosmology. Use a variety of observational
    methods, data analysis techniques and theoretical models to
    characterize the physical and dynamical states of celestial
    objects, determine formation history and predict future
    evolution. Use physics and chemistry knowledge to conduct
    observational, experimental and theoretical studies and
    modeling of stars, nebulae, galaxies, and systems of stars
    and galaxies, and of circumstellar, interstellar and
    intergalactic media, particles, molecules and radiation
    fields, in all electromagnetic wavelength ranges. Includes
    study of specialty areas such as Gamma Ray &amp; X-Ray
    Astronomy and Cosmic Ray Astrophysics, in which
    electromagnetic waves, x-ray emissions and cosmic ray
    particles provide data for examining the content,
    structure, origin and evolution of space elements.
  </skos:scopeNote>
  <nt2:status>Approved</nt2:status>
  <nt2:type>Descriptor</nt2:type>
  <nt2:inputdate>2006-12-13</nt2:inputdate>
  <dcterms:modified>2006-12-13</dcterms:modified>
  <nt2:code>52</nt2:code>
 </skos:Concept>
 <skos:Concept rdf:about='urn:comp:14'>
  <skos:prefLabel>Electron Device Technology</skos:prefLabel>
  <skos:altLabel>ELDEVTEC</skos:altLabel>
  <skos:broader rdf:resource='urn:comp:1339'/>
  <skos:scopeNote>Knowledge and practices associated in conducting research
    and development of electron device technology for
    communications component and systems such as microwave
    devices, MEMS and MMICs.
  </skos:scopeNote>
  <nt2:status>Approved</nt2:status>
  <nt2:type>Descriptor</nt2:type>
  <nt2:inputdate>2006-12-13</nt2:inputdate>
  <dcterms:modified>2006-12-13</dcterms:modified>
  <nt2:code>14</nt2:code>
 </skos:Concept>
 <skos:Concept rdf:about='urn:comp:173'>
  <skos:prefLabel>Project Work &amp; Team Management</skos:prefLabel>
  <skos:altLabel>PROWORKMMT</skos:altLabel>
  <skos:broader rdf:resource='urn:comp:1394'/>
  <skos:scopeNote>Knowledge, capabilities and practices associated with
    individuals that must understand and manage both the
    aspects of managing a project, as well as management of
    employees and/or teams. This pseudo competency requires the
    supervisor or lead to have the following competencies:
    Project Management
    Employee &amp; Team Leadership
    Work Performance Leadership
  </skos:scopeNote>
  <nt2:status>Approved</nt2:status>
  <nt2:type>Descriptor</nt2:type>
  <nt2:inputdate>2006-12-13</nt2:inputdate>
  <dcterms:modified>2006-12-13</dcterms:modified>
  <nt2:code>173</nt2:code>
 </skos:Concept>
 <skos:Concept rdf:about='urn:comp:91'>
  <skos:prefLabel>Advanced Analysis and Design Method Development</skos:prefLabel>
  <skos:altLabel>AADMD</skos:altLabel>
  <skos:broader rdf:resource='urn:comp:1363'/>
  <skos:changeNote>???
  </skos:changeNote>
  <skos:scopeNote>Enable the mission and system analysis and technology
    trades for advanced aerospace system concepts. Knowledge of
    systems analysis methods for use in advanced mission
    analysis and aerospace systems concept development &amp;
    technology assessment. Knowledge of multidisciplinary
    design optimization methods for use in conceptual,
    preliminary and detailed engineering analysis and design of
    aerospace vehicles and spacecraft (including design,
    manufacturing, and operations).
  </skos:scopeNote>
  <nt2:status>Approved</nt2:status>
  <nt2:type>Descriptor</nt2:type>
  <nt2:inputdate>2006-12-13</nt2:inputdate>
  <dcterms:dateAccepted>2005-12-07</dcterms:dateAccepted>
  <dcterms:modified>2006-12-18</dcterms:modified>
  <nt2:code>91</nt2:code>
 </skos:Concept>
 <skos:Concept rdf:about='urn:comp:60'>
  <skos:prefLabel>Communication Networks &amp; Engineering</skos:prefLabel>
  <skos:altLabel>COMNETENG</skos:altLabel>
  <skos:broader rdf:resource='urn:comp:1294'/>
  <skos:scopeNote>Knowledge and practices associated with researching and
    developing air and space communications architectures and
    networks to meet mission and system requirements, and to
    research new technology for improving air traffic
    management and communication between satellites,
    flightcraft, spacecraft and ground. Includes knowledge of
    communication systems electronics engineering for sending
    and receiving signals with different networks, including
    wireless, digital and radio frequency bandwidths. May
    involve ability to make effective, efficient, and prudent
    use of the radio spectrum in the best interest of the
    Nation, with care to conserve it for uses where other means
    of communication are not available or feasible.
  </skos:scopeNote>
  <nt2:status>Approved</nt2:status>
  <nt2:type>Descriptor</nt2:type>
  <nt2:inputdate>2006-12-13</nt2:inputdate>
  <dcterms:modified>2006-12-13</dcterms:modified>
  <nt2:code>60</nt2:code>
 </skos:Concept>
 <skos:Concept rdf:about='urn:comp:1038'>
  <skos:prefLabel>Materials Test Engineering</skos:prefLabel>
  <skos:altLabel>TSTMATER</skos:altLabel>
  <skos:broader rdf:resource='urn:comp:10'/>
  <skos:scopeNote>Knowledge, capabilities and practices associated with
    materials testing and the behavior and performance
    characteristics of materials in their use environment.
    Included is the understanding of various test set ups,
    instrumentation, data acquistion, equipment and tools
    utilized for material qualification and certification for
    ground and aerospace flight systems.
  </skos:scopeNote>
  <nt2:status>Approved</nt2:status>
  <nt2:type>Descriptor</nt2:type>
  <nt2:inputdate>2006-12-13</nt2:inputdate>
  <dcterms:modified>2006-12-13</dcterms:modified>
  <nt2:code>1038</nt2:code>
 </skos:Concept>
 <skos:Concept rdf:about='urn:comp:1011'>
  <skos:prefLabel>Communication and Knowledge Management Fundamental Research</skos:prefLabel>
  <skos:altLabel>HFRCOMM</skos:altLabel>
  <skos:broader rdf:resource='urn:comp:40'/>
  <skos:scopeNote>TBD (includes interpersonal communication,
    technology-mediated communication, procedures,
    documentation)
  </skos:scopeNote>
  <nt2:status>Approved</nt2:status>
  <nt2:type>Descriptor</nt2:type>
  <nt2:inputdate>2006-12-13</nt2:inputdate>
  <dcterms:modified>2006-12-13</dcterms:modified>
  <nt2:code>1011</nt2:code>
 </skos:Concept>
 <skos:Concept rdf:about='urn:comp:150'>
  <skos:prefLabel>Workplace Safety</skos:prefLabel>
  <skos:altLabel>WORKSAFETY</skos:altLabel>
  <skos:broader rdf:resource='urn:comp:1159'/>
  <skos:changeNote>???
  </skos:changeNote>
  <skos:scopeNote>Knowledge, capabilities, and practice associated with NASA,
    Federal (29 CFR 1960), and State OSHA health and safety
    regulations, policies and procedures used to develop and
    implement mishap prevention practices and measures in all
    NASA work places. These knowledge areas include safety of
    personnel and equipment during launch vehicle and payload
    processing, range operations, normal and industrial and
    laboratory operations, special high hazard tests and
    operations, develops explosives safety programs for
    pyrotechnics, and propellant operations, explosives and
    propellant citing, aviation and space operations, use and
    handling of exotic materials and chemicals, and design,
    construction, and use of facilities. Capabilities include
    ability to develop,assess and analyze workplace mishap
    prevention policy, manage, and assess the effectiveness of
    safety programs and practices, which are designed to
    prevent injury to personnel and loss of NASA property in
    all work environments on land, sea, air or space, and
    promote the safety of all employees. This function will
    also assure the proper investigation, recording, and
    corrective action documentation of all mishaps within the
    agency. At the National Level assures interagency
    coordination with all concerned departments and agencies
    concerned with safety and health policy development,
    program execution and evaluation.
  </skos:scopeNote>
  <nt2:status>Approved</nt2:status>
  <nt2:type>Descriptor</nt2:type>
  <nt2:inputdate>2006-12-13</nt2:inputdate>
  <dcterms:dateAccepted>2005-12-07</dcterms:dateAccepted>
  <dcterms:modified>2006-12-18</dcterms:modified>
  <nt2:code>150</nt2:code>
 </skos:Concept>
 <skos:Concept rdf:about='urn:comp:61'>
  <skos:prefLabel>Structural Dynamics</skos:prefLabel>
  <skos:altLabel>STRUCTDYN</skos:altLabel>
  <skos:broader rdf:resource='urn:comp:1347'/>
  <skos:scopeNote>Research knowledge, capabilities and practices for
    developing and analyzing methods to predict, verify and
    control structural dynamic response for aerospace
    structures and components including payloads, launch
    vehicles and propulsion systems. Involves ability to
    develop high fidelity integrated mechanical
    three-dimensional models to simulate system behavior and to
    provide a more thorough understanding of interactions
    between structures and the motion of mechanisms.
  </skos:scopeNote>
  <nt2:status>Approved</nt2:status>
  <nt2:type>Descriptor</nt2:type>
  <nt2:inputdate>2006-12-13</nt2:inputdate>
  <dcterms:modified>2006-12-13</dcterms:modified>
  <nt2:code>61</nt2:code>
 </skos:Concept>
 <skos:Concept rdf:about='urn:comp:62'>
  <skos:prefLabel>Mechanics and Durability</skos:prefLabel>
  <skos:altLabel>MECHDUR</skos:altLabel>
  <skos:broader rdf:resource='urn:comp:1347'/>
  <skos:changeNote>???
  </skos:changeNote>
  <skos:scopeNote>Knowledge, capability and practices associated with using
    and modifying advanced analytical and computational methods
    to assess the capability of structures to withstand applied
    loads and environmental conditions without failure.
    Includes the development of structural math models for the
    analysis of complex indeterminate structures, mechanical
    systems, and propulsion systems to determine structural
    response to multiple external and internal environmental
    conditions. Includes the performance of fatigue and
    fracture mechanics analyses to assess structural life.
    Includes broad knowledge of associated disciplines
    including structural dynamics, materials science,
    structural and mechanical design and damage tolerance. Also
    involves the planning and development of structural tests
    including measurement, instrument and test systems to
    assess structural characteristics and validate mathematical
    models.
  </skos:scopeNote>
  <nt2:status>Approved</nt2:status>
  <nt2:type>Descriptor</nt2:type>
  <nt2:inputdate>2006-12-13</nt2:inputdate>
  <dcterms:dateAccepted>2005-12-07</dcterms:dateAccepted>
  <dcterms:modified>2006-12-18</dcterms:modified>
  <nt2:code>62</nt2:code>
 </skos:Concept>
 <skos:Concept rdf:about='urn:comp:1089'>
  <skos:prefLabel>Institutional Environmental Remediation</skos:prefLabel>
  <skos:altLabel>ENVREMED</skos:altLabel>
  <skos:broader rdf:resource='urn:comp:133'/>
  <skos:scopeNote>Uses knowledge of environmental engineering, chemistry,
    biology, geology and hydrogeology to identify, investigate,
    and cleanup contaminated hazardous waste sites in
    compliance with Resource Conservation and Recovery Act
    (RCRA) and Comprehensive Environmental Response,
    Compensation, and Liability Act (CERCLA) requirements.
    Performs remediation contract management duties including
    evaluation of contractor performance and financial and
    schedule planning and tracking. Negotiates agreements with
    Federal, State, and local regulators. Manages the schedule
    of scientific/engineering, contractual, management, and
    informational documents, including preparation of Records
    of Decisions (RODs), administrative orders, and consent
    decrees. Performs necessary community relations activities.
  </skos:scopeNote>
  <nt2:status>Approved</nt2:status>
  <nt2:type>Descriptor</nt2:type>
  <nt2:inputdate>2006-12-13</nt2:inputdate>
  <dcterms:modified>2006-12-13</dcterms:modified>
  <nt2:code>1089</nt2:code>
 </skos:Concept>
 <skos:Concept rdf:about='urn:comp:155'>
  <skos:prefLabel>Space Environments Science and Engineering</skos:prefLabel>
  <skos:altLabel>SPACE_ENV</skos:altLabel>
  <skos:broader rdf:resource='urn:comp:1363'/>
  <skos:scopeNote>Knowledge of composition, elements, behaviors and impact of
    the space environments on the design, development, testing
    and operation of systems and components for aerospace
    vehicles and satellites. Involves understanding of space
    environments such as ionizing radiation, plasma,
    meteoroids, orbital debris, solar and thermal environments.
    Involves the ability to perform analyses to define the
    environments, quantify their effect on spacecraft design,
    development and operations and perform trade-off studies to
    optimize performance and assess risk.
  </skos:scopeNote>
  <nt2:status>Approved</nt2:status>
  <nt2:type>Descriptor</nt2:type>
  <nt2:inputdate>2006-12-13</nt2:inputdate>
  <dcterms:modified>2006-12-13</dcterms:modified>
  <nt2:code>155</nt2:code>
 </skos:Concept>
 <skos:Concept rdf:about='urn:comp:1056'>
  <skos:prefLabel>Propellant Management Systems Design and Analysis</skos:prefLabel>
  <skos:altLabel>RPPRPMMT</skos:altLabel>
  <skos:broader rdf:resource='urn:comp:73'/>
  <skos:scopeNote>Knowledge of cryogenic fluid physics and heat transfer
    associated with the design and development of cyrogenic
    tankage, insulation systems, zero boil-off, cyrocooler
    systems, thermodynamic vent systems, zero-G propellant
    management devices, zero-G liquid mass gauging, and
    incorporation of these into complete cryogenic propellant
    storage and management systems for long-duration space
    flight.
  </skos:scopeNote>
  <nt2:status>Approved</nt2:status>
  <nt2:type>Descriptor</nt2:type>
  <nt2:inputdate>2006-12-13</nt2:inputdate>
  <dcterms:modified>2006-12-13</dcterms:modified>
  <nt2:code>1056</nt2:code>
 </skos:Concept>
 <skos:Concept rdf:about='urn:comp:3'>
  <skos:prefLabel>Advanced Technical Training Design</skos:prefLabel>
  <skos:altLabel>ADVTEC</skos:altLabel>
  <skos:broader rdf:resource='urn:comp:1372'/>
  <skos:scopeNote>Knowledge of state-of-the art practices required to train
    technical personnel such as flight crew or ground support
    to accomplish objectives for near-term or futuristic
    missions. Identify training objectives, design training
    plans, tools, curricula and simulations using advanced
    techniques. Involves knowledge of instruction providers and
    tools, and how to employ and assess these resources.
  </skos:scopeNote>
  <nt2:status>Approved</nt2:status>
  <nt2:type>Descriptor</nt2:type>
  <nt2:inputdate>2006-12-13</nt2:inputdate>
  <dcterms:modified>2006-12-13</dcterms:modified>
  <nt2:code>3</nt2:code>
 </skos:Concept>
 <skos:Concept rdf:about='urn:comp:1067'>
  <skos:prefLabel>Industrial Hygiene</skos:prefLabel>
  <skos:altLabel>OCCHYGIENE</skos:altLabel>
  <skos:broader rdf:resource='urn:comp:130'/>
  <skos:scopeNote>Professional knowledge and skills to develop and implement
    preventive measures regarding all work-related exposures,
    injuries, and illnesses. Knowledge to coordinate,
    implement, manage, and assess the impact and effectiveness
    of related programs, practices and policies across the
    Agency, designed to protect the health of employees.
    Knowledge to provide advice to Agency top management
    concerning the impact that new regulations and technologies
    will have on the health of employees. Knowledge to provide
    professional symposia, workshops, and coordinate the
    development of related training programs for Agency-wide
    application.
  </skos:scopeNote>
  <nt2:status>Approved</nt2:status>
  <nt2:type>Descriptor</nt2:type>
  <nt2:inputdate>2006-12-13</nt2:inputdate>
  <dcterms:modified>2006-12-13</dcterms:modified>
  <nt2:code>1067</nt2:code>
 </skos:Concept>
 <skos:Concept rdf:about='urn:comp:1108'>
  <skos:prefLabel>Solid &amp; Hybrid Motor Systems</skos:prefLabel>
  <skos:altLabel>SOLIDENG</skos:altLabel>
  <skos:broader rdf:resource='urn:comp:73'/>
  <skos:scopeNote>Knowledge, capabilities, and practices associated with the
    design and analysis of complex solid and hybrid rocket
    motor systems for rocket propulsion. Includes the ability
    to perform solid and hybrid motor requirements development
    and decomposition, trade studies and feasibility
    assessments, analytical modeling of solid systems, detailed
    and functional design and analysis of solid and hybrid
    motor components, subsystems, and systems, motor subsystem
    and system development, and validation and verification of
    requirements through test and analysis to ensure the motor
    system meets mission requirements. Includes the capability
    to develop and integrate motor subsystems including the
    propellant, liner, insulation, case, and seal and the
    ability to perform detailed analyses to ensure the design
    met its intended objectives. Includes the knowledge and
    skills associated with solid and hybrid motor system test
    formulation, analytical prediction, and data analysis and
    reduction including identifying appropriate test methods
    and techiques, test plan formulation, test article design,
    test matrix development, identification of special
    instrumentation, ballistics modelling, and test facility
    requirements necessary to conduct solid and hybrid motor
    system testing. Ballistics modeling includes numerical
    simulation of the motor burn, including propellant
    geometry, chemistry, burn rates, gas flows, and combustion
    physics. Includes data analysis, reconstruction and
    trending to assess potential conceptual designs, to anchor
    mathematical models, or to ensure functional performance
    and identify design deficienies of as-designed propulsion
    systems over all flight / ground test regimes. Includes
    knowledge of the systems engineering tools, processes, and
    procedures that are required to ensure safe and reliable
    system development and integration.
  </skos:scopeNote>
  <nt2:status>Approved</nt2:status>
  <nt2:type>Descriptor</nt2:type>
  <nt2:inputdate>2006-12-13</nt2:inputdate>
  <dcterms:modified>2006-12-13</dcterms:modified>
  <nt2:code>1108</nt2:code>
 </skos:Concept>
 <skos:Concept rdf:about='urn:comp:1026'>
  <skos:prefLabel>Training Technologies</skos:prefLabel>
  <skos:altLabel>HFETRNG</skos:altLabel>
  <skos:broader rdf:resource='urn:comp:41'/>
  <skos:scopeNote>TBD (includes computer-based training systems, intelligent
    tutoring systems, handbooks, documentation)
  </skos:scopeNote>
  <nt2:status>Approved</nt2:status>
  <nt2:type>Descriptor</nt2:type>
  <nt2:inputdate>2006-12-13</nt2:inputdate>
  <dcterms:modified>2006-12-13</dcterms:modified>
  <nt2:code>1026</nt2:code>
 </skos:Concept>
 <skos:Concept rdf:about='urn:comp:156'>
  <skos:prefLabel>Bioethics</skos:prefLabel>
  <skos:broader rdf:resource='urn:comp:1430'/>
  <skos:narrower rdf:resource='urn:comp:1064'/>
  <skos:narrower rdf:resource='urn:comp:1065'/>
  <skos:scopeNote>Knowledge and experience in interpreting and implementing
    Federal and Agency regulations and guidelines for the
    protection of human and animal research subjects. Knowledge
    and expertise in the ethical principles that guide
    biomedical research. The ability to apply regulatory
    knowledge to implement appropriate and comprehension review
    mechanisms for the use of human and animal subjects in
    research. The ability to apply the knowledge of ethical
    theory and thought to guide Agency biomedical research and
    clinical medical policy development and decision-making.
  </skos:scopeNote>
  <nt2:status>Approved</nt2:status>
  <nt2:type>Descriptor</nt2:type>
  <nt2:inputdate>2006-12-13</nt2:inputdate>
  <dcterms:modified>2006-12-13</dcterms:modified>
  <nt2:code>156</nt2:code>
 </skos:Concept>
 <skos:Concept rdf:about='urn:comp:1027'>
  <skos:prefLabel>Human Reliability and Human Error Analysis</skos:prefLabel>
  <skos:altLabel>HFEHUMERR</skos:altLabel>
  <skos:broader rdf:resource='urn:comp:41'/>
  <skos:scopeNote>TBD
  </skos:scopeNote>
  <nt2:status>Approved</nt2:status>
  <nt2:type>Descriptor</nt2:type>
  <nt2:inputdate>2006-12-13</nt2:inputdate>
  <dcterms:modified>2006-12-13</dcterms:modified>
  <nt2:code>1027</nt2:code>
 </skos:Concept>
 <skos:Concept rdf:about='urn:comp:127'>
  <skos:prefLabel>Inspection, Investigation and Compliance</skos:prefLabel>
  <skos:altLabel>INSCOMP</skos:altLabel>
  <skos:broader rdf:resource='urn:comp:1125'/>
  <skos:scopeNote>Knowledge of how to provide objective evaluation of Agency
    standards and operation through use of inspection and
    investigation techniques and compliance audits.
    Understanding of how to assess risk, evaluate evidence,
    design and conduct inquiries such as inspections and
    investigations, and make recommendations to prevent, detect
    or solve crime, fraud, waste and abuse and ensure efficient
    Agency operations. Involves understanding of how to
    communicate information to constituents, including Agency
    leadership and management, employees, and Congress.
  </skos:scopeNote>
  <nt2:status>Approved</nt2:status>
  <nt2:type>Descriptor</nt2:type>
  <nt2:inputdate>2006-12-13</nt2:inputdate>
  <dcterms:modified>2006-12-13</dcterms:modified>
  <nt2:code>127</nt2:code>
 </skos:Concept>
 <skos:Concept rdf:about='urn:comp:57'>
  <skos:prefLabel>Nanotechnology</skos:prefLabel>
  <skos:altLabel>TINYTEC</skos:altLabel>
  <skos:broader rdf:resource='urn:comp:1363'/>
  <skos:scopeNote>Knowledge of the study of characteristics and properties of
    extremely small materials for development of new
    capabilities and applications in support of agency
    missions, programs and projects such as advanced
    structures, storage capabilities and computer systems.
    Includes an understanding of how to apply nanoscience
    findings, and a broad knowledge of other research and
    engineering disciplines.
  </skos:scopeNote>
  <nt2:status>Approved</nt2:status>
  <nt2:type>Descriptor</nt2:type>
  <nt2:inputdate>2006-12-13</nt2:inputdate>
  <dcterms:modified>2006-12-13</dcterms:modified>
  <nt2:code>57</nt2:code>
 </skos:Concept>
 <skos:Concept rdf:about='urn:comp:96'>
  <skos:prefLabel>Detector Systems</skos:prefLabel>
  <skos:altLabel>DETECTSYS</skos:altLabel>
  <skos:broader rdf:resource='urn:comp:1339'/>
  <skos:changeNote>Was deleted for REv. 6 (2005-12-07), then restored in 6a
    (2006-04-05). Will be scheduled for deletion in a future
    revision.
  </skos:changeNote>
  <skos:scopeNote>Knowledge, capabilities, and practices related to the
    research, design, development, characterization, and
    application of detectors and detector systems with an
    emphasis on remote sensing applications. Includes research
    and development of advanced detectors and detector systems
    covering a wide spectral range to include UV, visible, IR,
    and microwave. Also includes the design, development, test,
    characterization, and integration of detectors and detector
    systems into a variety of applications with an emphasis on
    remote sensing systems.
  </skos:scopeNote>
  <nt2:status>Approved</nt2:status>
  <nt2:type>Descriptor</nt2:type>
  <nt2:inputdate>2006-12-13</nt2:inputdate>
  <dcterms:dateAccepted>2006-04-05</dcterms:dateAccepted>
  <dcterms:modified>2006-12-18</dcterms:modified>
  <nt2:code>96</nt2:code>
 </skos:Concept>
 <skos:Concept rdf:about='urn:comp:15'>
  <skos:prefLabel>Electro-Mechanical Systems</skos:prefLabel>
  <skos:altLabel>ELMECHSY</skos:altLabel>
  <skos:broader rdf:resource='urn:comp:1294'/>
  <skos:scopeNote>Knowledge of and ability to design, develop, test,
    integrate and evaluate electro-mechanical systems such as;
    gimbals, cryogenic mechanisms, smart structures, and
    magnetic bearings, solar array drive systems, choppers,
    shutters, scanning, and focusing mechanisms. Has capability
    to perform the complete engineering lifecycle on systems
    for the drive, sensing, and control of precision flight
    instruments, and spacecraft subsystems.
  </skos:scopeNote>
  <nt2:status>Approved</nt2:status>
  <nt2:type>Descriptor</nt2:type>
  <nt2:inputdate>2006-12-13</nt2:inputdate>
  <dcterms:modified>2006-12-13</dcterms:modified>
  <nt2:code>15</nt2:code>
 </skos:Concept>
 <skos:Concept rdf:about='urn:comp:102'>
  <skos:prefLabel>Aerothermodynamics</skos:prefLabel>
  <skos:altLabel>AEROTHM</skos:altLabel>
  <skos:broader rdf:resource='urn:comp:1237'/>
  <skos:scopeNote>Knowledge, capabilities, and practices related to
    aero/aerothermodynamic design for aerospace vehicles and
    components under various flight conditions including
    liftoff, ascent, stage separation and reentry. Ability to
    plan, conduct and interpret results of experimental
    investigations and analytical/computational fluid dynamics
    to derive aerothermal environments. Inherent within this
    competency is also the ability to determine the effects of
    propulsion system plumes on the vehicle/components
    performance and environment. Knowledge of high temperature
    gas physics including molecular and atomic internal energy
    structure, rate processes, and radiative emission
    characteristics.
  </skos:scopeNote>
  <nt2:status>Approved</nt2:status>
  <nt2:type>Descriptor</nt2:type>
  <nt2:inputdate>2006-12-13</nt2:inputdate>
  <dcterms:modified>2006-12-13</dcterms:modified>
  <nt2:code>102</nt2:code>
 </skos:Concept>
 <skos:Concept rdf:about='urn:comp:1092'>
  <skos:prefLabel>Facility Electrical Engineering</skos:prefLabel>
  <skos:altLabel>FACELECENG</skos:altLabel>
  <skos:broader rdf:resource='urn:comp:112'/>
  <skos:scopeNote>Knowledge of planning, designing, developing, testing, or
    evaluating electrical components, electrical installation
    and inspection for aerospace facility programs. Knowledge
    of electrical codes and standards, and testing of complex
    electrical or electronic systems including sources, loads,
    power management and distribution, communications and
    controls. Also requires knowledge of construction
    contracting and contractor oversight and contracts
    management.
  </skos:scopeNote>
  <nt2:status>Approved</nt2:status>
  <nt2:type>Descriptor</nt2:type>
  <nt2:inputdate>2006-12-13</nt2:inputdate>
  <dcterms:modified>2006-12-13</dcterms:modified>
  <nt2:code>1092</nt2:code>
 </skos:Concept>
 <skos:Concept rdf:about='urn:comp:157'>
  <skos:prefLabel>International Program Development</skos:prefLabel>
  <skos:altLabel>INTLPGMDEV</skos:altLabel>
  <skos:broader rdf:resource='urn:comp:1125'/>
  <skos:scopeNote>This competency refers to the knowledge and capabilities
    associated with establishing international
    programs/agreements through international negotiations,
    drafting international agreements that comply with U.S.
    laws and regulations, arranging negotiation meetings,
    understanding the protocol issues involved in meetings,
    signing ceremonies, meetings between heads of agencies and
    NASA, exchange of gifts, liaison with Department of State
    and other U.S. Agencies and Departments. This may involve
    both reimbursable and non-reimbursable agreements.
  </skos:scopeNote>
  <nt2:status>Approved</nt2:status>
  <nt2:type>Descriptor</nt2:type>
  <nt2:inputdate>2006-12-13</nt2:inputdate>
  <dcterms:modified>2006-12-13</dcterms:modified>
  <nt2:code>157</nt2:code>
 </skos:Concept>
 <skos:Concept rdf:about='urn:comp:92'>
  <skos:prefLabel>Laser Technology</skos:prefLabel>
  <skos:altLabel>LASER</skos:altLabel>
  <skos:broader rdf:resource='urn:comp:1339'/>
  <skos:scopeNote>Knowledge of high performance, high reliability lasers and
    laser systems for measurement of essential planet
    atmospheric variables including aerosols, water vapor,
    ozone, wind velocity, green house gasses, ozone, and
    metrology applications such as ice cap thickness, as well
    as medicine and manufacturing technologies. Able to apply
    subspecialty knowledge to research crystal materials and
    their frequencies, and design highly precise laser systems
    (such as those tunable and stable to a part per million
    with high spectral purity, in double pulse format with
    multibillion shot lifetime) that can withstand both launch
    and the rigors of deployment in space.
  </skos:scopeNote>
  <nt2:status>Approved</nt2:status>
  <nt2:type>Descriptor</nt2:type>
  <nt2:inputdate>2006-12-13</nt2:inputdate>
  <dcterms:modified>2006-12-13</dcterms:modified>
  <nt2:code>92</nt2:code>
 </skos:Concept>
 <skos:Concept rdf:about='urn:comp:1044'>
  <skos:prefLabel>Parts &amp; Packaging</skos:prefLabel>
  <skos:altLabel>ELPARTSPKG</skos:altLabel>
  <skos:broader rdf:resource='urn:comp:13'/>
  <skos:scopeNote>Knowledge, capabilities, and practices associated with
    electro-mechanical design including printed circuit (pc)
    layout, design of mechanical housings (black boxes),
    thermal analysis of pc boards and black boxes, and
    processes involved in the manufacturing/assembly of this
    hardware.
  </skos:scopeNote>
  <nt2:status>Approved</nt2:status>
  <nt2:type>Descriptor</nt2:type>
  <nt2:inputdate>2006-12-13</nt2:inputdate>
  <dcterms:modified>2006-12-13</dcterms:modified>
  <nt2:code>1044</nt2:code>
 </skos:Concept>
 <skos:Concept rdf:about='urn:comp:1231'>
  <skos:prefLabel>Systems Analysis &amp; Mission Planning Competency Suite</skos:prefLabel>
  <skos:broader rdf:resource='urn:comp:1208'/>
  <skos:narrower rdf:resource='urn:comp:89'/>
  <skos:narrower rdf:resource='urn:comp:WQQ-590'/>
  <skos:narrower rdf:resource='urn:comp:WQQ-591'/>
  <skos:narrower rdf:resource='urn:comp:1'/>
  <skos:narrower rdf:resource='urn:comp:2'/>
  <skos:narrower rdf:resource='urn:comp:175'/>
  <nt2:status>Approved</nt2:status>
  <nt2:type>Descriptor</nt2:type>
  <nt2:inputdate>2006-12-13</nt2:inputdate>
  <dcterms:modified>2006-12-13</dcterms:modified>
  <nt2:code>1231</nt2:code>
 </skos:Concept>
 <skos:Concept rdf:about='urn:comp:43'>
  <skos:prefLabel>Fluid Physics</skos:prefLabel>
  <skos:altLabel>FLUIDPHY</skos:altLabel>
  <skos:broader rdf:resource='urn:comp:1424'/>
  <skos:scopeNote>Employ knowledge of the motion of fluids and the effects of
    such motion, to the understanding, control and improvement
    of industrial and natural processes. Areas of research
    include microgravitational study of complex fluids,
    multiphase and phase change, fluid dynamics and
    instabilities, and interfacial phenomena.
  </skos:scopeNote>
  <nt2:status>Approved</nt2:status>
  <nt2:type>Descriptor</nt2:type>
  <nt2:inputdate>2006-12-13</nt2:inputdate>
  <dcterms:modified>2006-12-13</dcterms:modified>
  <nt2:code>43</nt2:code>
 </skos:Concept>
 <skos:Concept rdf:about='urn:comp:116'>
  <skos:prefLabel>Partnership &amp; Business Development</skos:prefLabel>
  <skos:altLabel>BUSDEV</skos:altLabel>
  <skos:broader rdf:resource='urn:comp:1125'/>
  <skos:scopeNote>Knowledge, capabilities and practices associated with the
    effective targeting and acquisition of external
    partnerships and business opportunities, including funding
    opportunities for projects and programs Includes an
    understanding of the Agency's strategic plan, the ability
    to identify, assess and forecast new business opportunities
    such as technology transfer, leasing, enhanced use leasing,
    and develop and use appropriate marketing strategies.
    Requires knowledge of relevant markets, customer needs in
    those markets, and an ability to recognize and analyze
    market trends. Involves development,or assessment, of
    proposals to win business, and management of existing
    agreements with external entities such as industry,
    government, university, and international partnerships.
    Also includes knowledge of Space Act Agreements, and an
    ability to facilitate and manage partnerships that support
    Agency strategies, partner requirements and Space Act
    provisions. Ability to integrate and work with the
    appropriate elements of the agency's technical and support
    communities.
  </skos:scopeNote>
  <nt2:status>Approved</nt2:status>
  <nt2:type>Descriptor</nt2:type>
  <nt2:inputdate>2006-12-13</nt2:inputdate>
  <dcterms:modified>2006-12-13</dcterms:modified>
  <nt2:code>116</nt2:code>
 </skos:Concept>
 <skos:Concept rdf:about='urn:comp:44'>
  <skos:prefLabel>Earth Atmosphere</skos:prefLabel>
  <skos:altLabel>EARTHATM</skos:altLabel>
  <skos:broader rdf:resource='urn:comp:1407'/>
  <skos:scopeNote>Knowledge of the fundamental processes of radiation,
    chemistry and dynamics in the study of the structure and
    composition of the Earth's atmosphere. Conceive and
    implement a variety of observational methods, data analysis
    techniques, and theoretical models to characterize the
    state of the atmosphere, detect variability and explain the
    responsible forcing mechanisms, and predict the future
    state of the atmosphere. Able to develop and implement
    missions to conduct atmospheric research, and contribute to
    the development of atmospheric instrument and sensor
    development. Includes subspecialty knowledge in areas such
    as Radiation and Climate, Stratospheric &amp; Tropospheric
    Chemistry.
  </skos:scopeNote>
  <nt2:status>Approved</nt2:status>
  <nt2:type>Descriptor</nt2:type>
  <nt2:inputdate>2006-12-13</nt2:inputdate>
  <dcterms:modified>2006-12-13</dcterms:modified>
  <nt2:code>44</nt2:code>
 </skos:Concept>
 <skos:Concept rdf:about='urn:comp:1101'>
  <skos:prefLabel>Technical Student Trainee</skos:prefLabel>
  <skos:altLabel>STUTECH</skos:altLabel>
  <skos:broader rdf:resource='urn:comp:174'/>
  <skos:scopeNote>This is a training and development competency for employees
    who are classified as Technical Student Trainees.
  </skos:scopeNote>
  <nt2:status>Approved</nt2:status>
  <nt2:type>Descriptor</nt2:type>
  <nt2:inputdate>2005-12-07</nt2:inputdate>
  <dcterms:dateAccepted>2005-12-07</dcterms:dateAccepted>
  <dcterms:modified>2006-12-18</dcterms:modified>
  <nt2:code>1101</nt2:code>
 </skos:Concept>
 <skos:Concept rdf:about='urn:comp:58'>
  <skos:prefLabel>Bioengineering</skos:prefLabel>
  <skos:altLabel>BIOENG</skos:altLabel>
  <skos:broader rdf:resource='urn:comp:1244'/>
  <skos:scopeNote>Application of technologies to living systems including
    such areas as biomechanics, imaging, biomedical
    transducers, biofluids and sensors.
  </skos:scopeNote>
  <nt2:status>Approved</nt2:status>
  <nt2:type>Descriptor</nt2:type>
  <nt2:inputdate>2006-12-13</nt2:inputdate>
  <dcterms:modified>2006-12-13</dcterms:modified>
  <nt2:code>58</nt2:code>
 </skos:Concept>
 <skos:Concept rdf:about='urn:comp:1028'>
  <skos:prefLabel>Structural Design and Development Engineering</skos:prefLabel>
  <skos:altLabel>DDESTRUCT</skos:altLabel>
  <skos:broader rdf:resource='urn:comp:8'/>
  <skos:scopeNote>Knowledge, capability and practices associated with all
    aspects of the technical structural design and development
    by using and modifying advanced analytical and
    computational methods to design, develop, test and research
    the characteristics and performance of structures. Includes
    the development of structural math models for and
    comprehensive assessment of air, space and ground
    structures, the analysis of the models to determine
    structural response to multiple external and internal
    environmental conditions, and analysis of flight and test
    data for structural systems. Includes broad knowledge of
    structures disciplines including structural dynamics,
    structural mechanics, structural acoustics, mechanisms,
    electro-mechanical devices, aeroelasticity, impact, damage
    tolerance and structural life prediction. Also involves
    research into measurement, instrument and test systems to
    assess structural characteristics and risks, and ensure
    system integration.
  </skos:scopeNote>
  <nt2:status>Approved</nt2:status>
  <nt2:type>Descriptor</nt2:type>
  <nt2:inputdate>2006-12-13</nt2:inputdate>
  <dcterms:modified>2006-12-13</dcterms:modified>
  <nt2:code>1028</nt2:code>
 </skos:Concept>
 <skos:Concept rdf:about='urn:comp:1002'>
  <skos:prefLabel>Knowledge &amp; Communication Management</skos:prefLabel>
  <skos:altLabel>LEADCOMM</skos:altLabel>
  <skos:broader rdf:resource='urn:comp:140'/>
  <skos:scopeNote>Understands and applies knowledge management practices,
    theories and success factors. Possesses knowledge and
    capability to lead efforts to capture, organize, store and
    share knowledge from major team, functional community or
    programmatic efforts. Creates systems that facilitate
    communication of knowledge within NASA in order to leverage
    best practices, and technical know how or advancements
    within the Agency. Possesses knowledge of information
    technologies available at NASA and selects and uses those
    appropriately for managing work and develops strategies to
    integrate new technology into the workplace. Understands
    and applies principles of information security in relation
    to data publishing, technology transfer and release of
    information.
  </skos:scopeNote>
  <nt2:status>Approved</nt2:status>
  <nt2:type>Descriptor</nt2:type>
  <nt2:inputdate>2006-12-13</nt2:inputdate>
  <dcterms:modified>2006-12-13</dcterms:modified>
  <nt2:code>1002</nt2:code>
 </skos:Concept>
 <skos:Concept rdf:about='urn:comp:22'>
  <skos:prefLabel>Control Systems, Guidance &amp; Navigation</skos:prefLabel>
  <skos:altLabel>GNC</skos:altLabel>
  <skos:broader rdf:resource='urn:comp:1294'/>
  <skos:narrower rdf:resource='urn:comp:1110'/>
  <skos:narrower rdf:resource='urn:comp:1111'/>
  <skos:narrower rdf:resource='urn:comp:1048'/>
  <skos:narrower rdf:resource='urn:comp:1049'/>
  <skos:narrower rdf:resource='urn:comp:1046'/>
  <skos:narrower rdf:resource='urn:comp:1047'/>
  <skos:scopeNote>Knowledge of and ability to develop analytical,
    computational, and experimental methods for
    control/guidance algorithms, and apply research to develop
    requirements for control and instrumentation systems;
    establish component and systems; and use analytical
    modeling and simulation tools that determine control
    dynamic solutions. Knowledge of research and engineering of
    integrated aerospace vehicle systems for the guidance,
    navigation, and control and health management of flight
    vehicles in the atmosphere and space. Includes knowledge of
    sensors and avionics, flight dynamics, mathematical
    modeling, experimental methods and a broad array of
    engineering disciplines.
  </skos:scopeNote>
  <nt2:status>Approved</nt2:status>
  <nt2:type>Descriptor</nt2:type>
  <nt2:inputdate>2006-12-13</nt2:inputdate>
  <dcterms:modified>2006-12-13</dcterms:modified>
  <nt2:code>22</nt2:code>
 </skos:Concept>
 <skos:Concept rdf:about='urn:comp:69'>
  <skos:prefLabel>Airbreathing Propulsion</skos:prefLabel>
  <skos:altLabel>AIRPRO</skos:altLabel>
  <skos:broader rdf:resource='urn:comp:1314'/>
  <skos:scopeNote>Knowledge of technologies and concepts for airbreathing
    propelled vehicles in order to enhance the safety of
    operations, reduce lifecycle costs, contribute to reduced
    costs of air travel and access to space, and reduce carbon
    dioxide emissions. Includes knowledge of various engine
    cycles, flight conditions, efficient mixing and combustion,
    various materials, and reliable design tools for
    aerodynamic and propulsion system design and performance
    prediction, as well as application of combined cycle
    systems to advanced propulsion techniques.
  </skos:scopeNote>
  <nt2:status>Approved</nt2:status>
  <nt2:type>Descriptor</nt2:type>
  <nt2:inputdate>2006-12-13</nt2:inputdate>
  <dcterms:modified>2006-12-13</dcterms:modified>
  <nt2:code>69</nt2:code>
 </skos:Concept>
 <skos:Concept rdf:about='urn:comp:1070'>
  <skos:prefLabel>Medical Practice</skos:prefLabel>
  <skos:altLabel>MDPRACTICE</skos:altLabel>
  <skos:broader rdf:resource='urn:comp:36'/>
  <skos:scopeNote>Knowledge and expertise of the multi-disciplinary practice
    of Aerospace Medicine taking into account the hostile,
    diverse environments of NASA aeronautic and space missions.
    Health maintenance and diagnosis and treatment of illness
    and injuries are the goals of medical practice. Knowledge
    and skills of physiology of mission environment,
    operational medicine, clinical practice, human systems
    interfaces, and astronaut selection and training.
  </skos:scopeNote>
  <nt2:status>Approved</nt2:status>
  <nt2:type>Descriptor</nt2:type>
  <nt2:inputdate>2006-12-13</nt2:inputdate>
  <dcterms:modified>2006-12-13</dcterms:modified>
  <nt2:code>1070</nt2:code>
 </skos:Concept>
 <skos:Concept rdf:about='urn:comp:1039'>
  <skos:prefLabel>Thermal Test Engineering</skos:prefLabel>
  <skos:altLabel>TSTTHERMO</skos:altLabel>
  <skos:broader rdf:resource='urn:comp:10'/>
  <skos:scopeNote>Knowledge of physics, engineering, thermal, and thermal
    vacuum to test systems or subsystems under development,
    qualification, or acceptance requirements for their
    functioning, efficacy and conformance to design
    requirements and performance, or to test prototypes for
    feasibility. May involve ability to plan, create test
    procedures, conduct, and evaluate developmental,
    qualification, acceptance, and flight test and checkout
    requirements in accordance with NASA, Military or
    Commercial Specifications of test facilities, space and
    ground systems, components, piece parts, as well as
    integrated systems. Includes knowledge of environmental
    test techniques used to simulate thermal and thermal vacuum
    conditions such as launch, reentry, orbit, and landing,
    including radiation, pressure, thermal, outgassing,
    microgravity and solar vacuum, aerodynamics and temperature
    and humidity. Includes knowledge required for safe and
    reliable system testing and development/integration.
  </skos:scopeNote>
  <nt2:status>Approved</nt2:status>
  <nt2:type>Descriptor</nt2:type>
  <nt2:inputdate>2006-12-13</nt2:inputdate>
  <dcterms:modified>2006-12-13</dcterms:modified>
  <nt2:code>1039</nt2:code>
 </skos:Concept>
 <skos:Concept rdf:about='urn:comp:103'>
  <skos:prefLabel>Acoustics</skos:prefLabel>
  <skos:broader rdf:resource='urn:comp:1237'/>
  <skos:scopeNote>Knowledge, capabilities, and practices related to interior
    and exterior noise reduction and acoustic design for
    advanced aerospace systems, subsystems, and components to
    meet environmental requirements. Includes knowledge and
    application of experimental and computational aero and
    structural acoustics. Inherent in this competency is the
    capability to determine the influence of acoustic
    environment on ground observers and vehicle passengers
    alike, as well as to develop an understanding of its impact
    on vehicle structural responses, including sonic fatigue.
    Includes ability to conceive, plan, and implement
    appropriate experimental and flight test programs that are
    designed to understand and predict the acoustic environment
    and to validate advanced active and passive noise control
    concepts.
    NASA Competency Management SystemPage 32
  </skos:scopeNote>
  <nt2:status>Approved</nt2:status>
  <nt2:type>Descriptor</nt2:type>
  <nt2:inputdate>2006-12-13</nt2:inputdate>
  <dcterms:modified>2006-12-13</dcterms:modified>
  <nt2:code>103</nt2:code>
 </skos:Concept>
 <skos:Concept rdf:about='urn:comp:152'>
  <skos:prefLabel>Institutional Aircraft Operations</skos:prefLabel>
  <skos:altLabel>AIROPS</skos:altLabel>
  <skos:broader rdf:resource='urn:comp:1159'/>
  <skos:scopeNote>Knowledge of aircraft operations, maintenance, acquisition,
    airworthiness and aviation safety principles for
    technologically complex aircraft programs and their
    associated systems and facilities. Knowledge of how to
    develop aircraft requirements and the associated costs and
    scheduling to satisfy functional and regulatory
    requirements. Ability to develop and manage a comprehensive
    aviation program to sustain and optimize institutional and
    research and development (R&amp;D) requirements consistent with
    standards, codes and regulations. Effectively integrate
    these aircraft services to be consistent with the broader
    objectives, strategies, and program goals of the
    organization.
  </skos:scopeNote>
  <nt2:status>Approved</nt2:status>
  <nt2:type>Descriptor</nt2:type>
  <nt2:inputdate>2006-12-13</nt2:inputdate>
  <dcterms:modified>2006-12-13</dcterms:modified>
  <nt2:code>152</nt2:code>
 </skos:Concept>
 <skos:Concept rdf:about='urn:comp:77'>
  <skos:prefLabel>Power Generation -Photovoltaics</skos:prefLabel>
  <skos:altLabel>PWRPHO</skos:altLabel>
  <skos:broader rdf:resource='urn:comp:1314'/>
  <skos:scopeNote>Knowledge, capabilities, and practices associated with the
    design, development, test and evaluation of photovoltaic
    power generation systems, including electric actuation and
    solar cell/array systems.
  </skos:scopeNote>
  <nt2:status>Approved</nt2:status>
  <nt2:type>Descriptor</nt2:type>
  <nt2:inputdate>2006-12-13</nt2:inputdate>
  <dcterms:modified>2006-12-13</dcterms:modified>
  <nt2:code>77</nt2:code>
 </skos:Concept>
 <skos:Concept rdf:about='urn:comp:168'>
  <skos:prefLabel>Research, Development or Flight Facility Planning</skos:prefLabel>
  <skos:altLabel>FACLTYPLAN</skos:altLabel>
  <skos:broader rdf:resource='urn:comp:1159'/>
  <skos:scopeNote>Knowledge of strategic and long-term planning for research,
    development or flight facilities and related equipment
    required to support operations for current and future
    program needs. Knowledge required to develop functional and
    facility requirements and the associated costs and
    scheduling. Includes knowledge required to coordinate and
    incorporate the necessary architectural engineering to
    satisfy all functional, institutional and regulatory
    requirements. Specialized knowledge of engineering and
    technology competencies to address specific high energy/
    high risk facility systems including but not limited to:
    high temperature systems, high pressure systems, cryogenic
    systems, exotic gases, control systems, data acquisition
    systems, energy transfer systems, laboratory workspace
    planning, communication infrastructure. Knowledge of
    project management and control including life-cycle costs,
    engineering economics, and project planning and evaluation
    including scope, cost and schedule and program controls
    including earned value management or other measure for
    project controls. Includes abilities to devise and
    implement policies and procedures regarding risk/hazard
    mitigation and safety assurance.
  </skos:scopeNote>
  <nt2:status>Approved</nt2:status>
  <nt2:type>Descriptor</nt2:type>
  <nt2:inputdate>2006-12-13</nt2:inputdate>
  <dcterms:modified>2006-12-13</dcterms:modified>
  <nt2:code>168</nt2:code>
 </skos:Concept>
 <skos:Concept rdf:about='urn:comp:1050'>
  <skos:prefLabel>Electric Propulsion</skos:prefLabel>
  <skos:altLabel>APELEC</skos:altLabel>
  <skos:broader rdf:resource='urn:comp:72'/>
  <skos:scopeNote>Research, development, design, testing and evaluation of
    in-space electric propulsion system technologies,
    comprising power, power conditioning, propellant storage
    and management, and thrusters. Specialty knowledge in the
    three categories of electric propulsion thruster devices:
    electrothermal, electromagnetic and electrostatic.
  </skos:scopeNote>
  <nt2:status>Approved</nt2:status>
  <nt2:type>Descriptor</nt2:type>
  <nt2:inputdate>2006-12-13</nt2:inputdate>
  <dcterms:modified>2006-12-13</dcterms:modified>
  <nt2:code>1050</nt2:code>
 </skos:Concept>
 <skos:Concept rdf:about='urn:comp:1371'>
  <skos:prefLabel>Mission Operations Knowledge Domain</skos:prefLabel>
  <skos:broader rdf:resource='urn:comp:1438'/>
  <skos:narrower rdf:resource='urn:comp:1372'/>
  <skos:narrower rdf:resource='urn:comp:1381'/>
  <nt2:status>Approved</nt2:status>
  <nt2:type>Descriptor</nt2:type>
  <nt2:inputdate>2006-12-13</nt2:inputdate>
  <dcterms:modified>2007-01-11</dcterms:modified>
  <nt2:code>1371</nt2:code>
 </skos:Concept>
 <skos:Concept rdf:about='urn:comp:1110'>
  <skos:prefLabel>Control Components</skos:prefLabel>
  <skos:altLabel>GNCCTLCOM</skos:altLabel>
  <skos:broader rdf:resource='urn:comp:22'/>
  <skos:scopeNote>Knowledge of and ability to perform research, design,
    development, test and evaluation of inertial, celestial,
    magnetic and electro-optical sensors; momentum control
    actuators, precision gimbal systems, and precision mirror
    actuators; and linear and rotational magnetic and
    piezo-electric actuators for guidance, navigation and
    control systems; pointing and attitude control systems; and
    large space structures control. Ability to select and test
    appropriate sensors and actuators for the various
    applications and integrate them into larger subsystems.
    Includes knowledge of control circuitry, control theory,
    experimental methods, statistical analysis and application
    and mathematical modeling..
  </skos:scopeNote>
  <nt2:status>Approved</nt2:status>
  <nt2:type>Descriptor</nt2:type>
  <nt2:inputdate>2006-04-05</nt2:inputdate>
  <dcterms:dateAccepted>2006-04-05</dcterms:dateAccepted>
  <dcterms:modified>2006-12-18</dcterms:modified>
  <nt2:code>1110</nt2:code>
 </skos:Concept>
 <skos:Concept rdf:about='urn:comp:1096'>
  <skos:prefLabel>Construction Management</skos:prefLabel>
  <skos:altLabel>FACONSTMMT</skos:altLabel>
  <skos:broader rdf:resource='urn:comp:112'/>
  <skos:scopeNote>Knowledge of the materials, methods, systems, and the tools
    used to construct facilities and other real property
    infrastructure.
  </skos:scopeNote>
  <nt2:status>Approved</nt2:status>
  <nt2:type>Descriptor</nt2:type>
  <nt2:inputdate>2006-12-13</nt2:inputdate>
  <dcterms:modified>2006-12-13</dcterms:modified>
  <nt2:code>1096</nt2:code>
 </skos:Concept>
 <skos:Concept rdf:about='urn:comp:11'>
  <skos:prefLabel>Engineering and Science Support</skos:prefLabel>
  <skos:altLabel>ENGSCISUP</skos:altLabel>
  <skos:broader rdf:resource='urn:comp:1209'/>
  <skos:scopeNote>Knowledge, capabilities and practices associated with
    supporting engineering and science functions. This support
    includes laboratory, modeling, manufacturing and analytical
    activities. Focus is on the abilities of an individual to
    visualize, plan and execute limited instructions from
    engineering, in the form of drawings/schematics, written or
    verbal direction, in order to produce a model, prototype or
    finished product. The technician’s application of tools and
    apparatus, both physical and analytical, are a key element
    of this competency.
  </skos:scopeNote>
  <nt2:status>Approved</nt2:status>
  <nt2:type>Descriptor</nt2:type>
  <nt2:inputdate>2006-12-13</nt2:inputdate>
  <dcterms:modified>2006-12-13</dcterms:modified>
  <nt2:code>11</nt2:code>
 </skos:Concept>
 <skos:Concept rdf:about='urn:comp:1033'>
  <skos:prefLabel>Materials Integration Engineering</skos:prefLabel>
  <skos:altLabel>INTMATER</skos:altLabel>
  <skos:broader rdf:resource='urn:comp:9'/>
  <skos:scopeNote>Knowledge and capability to integrate all materials
    engineering elements and practices associated with research
    into the characteristics and performance of materials and
    the design, development and testing of those materials,
    into a functioning system or subsystem such as complex
    flight to flight and flight to ground and facilities
    systems. Includes knowledge and capabilities required for
    the development and application of math models and
    statistical analysis for assessment of material durability
    and response to environmental conditions and contaminants,
    required for safe and
    reliable application and integration of materials
    engineering elements of a system, schedules, configurations
    and resources as well as the development of launch,
    mission, manifest, contigency and long-range plans and
    responses to externally-driven requirements.
  </skos:scopeNote>
  <nt2:status>Approved</nt2:status>
  <nt2:type>Descriptor</nt2:type>
  <nt2:inputdate>2006-12-13</nt2:inputdate>
  <dcterms:modified>2006-12-13</dcterms:modified>
  <nt2:code>1033</nt2:code>
 </skos:Concept>
 <skos:Concept rdf:about='urn:comp:100'>
  <skos:prefLabel>Aeroelasticity</skos:prefLabel>
  <skos:altLabel>AEROELA</skos:altLabel>
  <skos:broader rdf:resource='urn:comp:1237'/>
  <skos:scopeNote>Research knowledge, capabilities, and practices for
    investigating aeroelastic phenomena and complex steady and
    unsteady aerodynamic flow phenomena especially in the
    transonic speed range, for investigating, developing, and
    demonstrating novel concepts that prevent aeroelastic
    instabilities, alleviate adverse aeroelastic responses,
    reduce loads and vibrations, and exploit the aeroelastic
    characteristics of aerospace vehicles, for developing
    analytical methods that predict the aeroelastic and
    aeroservoelastic responses of aerospace vehicles, and for
    conducting unsteady aerodynamic, aeroelastic, and
    aeroservoelastic wind-tunnel tests.
  </skos:scopeNote>
  <nt2:status>Approved</nt2:status>
  <nt2:type>Descriptor</nt2:type>
  <nt2:inputdate>2006-12-13</nt2:inputdate>
  <dcterms:modified>2006-12-13</dcterms:modified>
  <nt2:code>100</nt2:code>
 </skos:Concept>
 <skos:Concept rdf:about='urn:comp:1244'>
  <skos:prefLabel>Human and Biological Competency Suite</skos:prefLabel>
  <skos:broader rdf:resource='urn:comp:1208'/>
  <skos:narrower rdf:resource='urn:comp:36'/>
  <skos:narrower rdf:resource='urn:comp:58'/>
  <skos:narrower rdf:resource='urn:comp:35'/>
  <skos:narrower rdf:resource='urn:comp:59'/>
  <skos:narrower rdf:resource='urn:comp:97'/>
  <skos:narrower rdf:resource='urn:comp:37'/>
  <skos:narrower rdf:resource='urn:comp:39'/>
  <skos:narrower rdf:resource='urn:comp:38'/>
  <skos:narrower rdf:resource='urn:comp:40'/>
  <skos:narrower rdf:resource='urn:comp:41'/>
  <nt2:status>Approved</nt2:status>
  <nt2:type>Descriptor</nt2:type>
  <nt2:inputdate>2006-12-13</nt2:inputdate>
  <dcterms:modified>2006-12-13</dcterms:modified>
  <nt2:code>1244</nt2:code>
 </skos:Concept>
 <skos:Concept rdf:about='urn:comp:1'>
  <skos:prefLabel>Mission Analysis and Planning</skos:prefLabel>
  <skos:altLabel>MAP</skos:altLabel>
  <skos:broader rdf:resource='urn:comp:1231'/>
  <skos:scopeNote>Knowledge and ability to analyze requirements of current
    and near-term missions. Manage integration of technical
    elements such as vehicle design, flight trajectories, and
    operational and ground-based infrastructure requirements in
    order to meet mission and programmatic objectives.
  </skos:scopeNote>
  <nt2:status>Approved</nt2:status>
  <nt2:type>Descriptor</nt2:type>
  <nt2:inputdate>2006-12-13</nt2:inputdate>
  <dcterms:modified>2006-12-13</dcterms:modified>
  <nt2:code>1</nt2:code>
 </skos:Concept>
 <skos:Concept rdf:about='urn:comp:161'>
  <skos:prefLabel>Data Systems and Technology</skos:prefLabel>
  <skos:altLabel>DATSYS</skos:altLabel>
  <skos:broader rdf:resource='urn:comp:1283'/>
  <skos:narrower rdf:resource='urn:comp:1100'/>
  <skos:narrower rdf:resource='urn:comp:1080'/>
  <skos:narrower rdf:resource='urn:comp:1099'/>
  <skos:scopeNote>Knowledge of the principles, procedures, and tools of data
    management, such as modeling techniques, data backup, data
    recovery, data dictionaries, data warehousing, data mining,
    data disposal, and data standardization processes.
  </skos:scopeNote>
  <nt2:status>Approved</nt2:status>
  <nt2:type>Descriptor</nt2:type>
  <nt2:inputdate>2006-12-13</nt2:inputdate>
  <dcterms:modified>2006-12-13</dcterms:modified>
  <nt2:code>161</nt2:code>
 </skos:Concept>
 <skos:Concept rdf:about='urn:comp:1032'>
  <skos:prefLabel>Structural Integration Engineering</skos:prefLabel>
  <skos:altLabel>INTSTRUCT</skos:altLabel>
  <skos:broader rdf:resource='urn:comp:9'/>
  <skos:scopeNote>Knowledge of engineering; system engineering;
    manufacturing; testing; quality, reliability, and safety
    engineering; risk management; and resource, schedule, and
    programmatic requirements for the integration of structural
    systems, subsystems, and components that verify the
    completed products function, efficacy, and conformance to
    design requirements. This activity involves the long range
    planning, coordination, oversight, and integration of all
    structural systems, subsystems, and components in
    accordance with requirements and specifications, both
    external and internal.
  </skos:scopeNote>
  <nt2:status>Approved</nt2:status>
  <nt2:type>Descriptor</nt2:type>
  <nt2:inputdate>2006-12-13</nt2:inputdate>
  <dcterms:modified>2006-12-13</dcterms:modified>
  <nt2:code>1032</nt2:code>
 </skos:Concept>
 <skos:Concept rdf:about='urn:comp:1100'>
  <skos:prefLabel>Data Visualization</skos:prefLabel>
  <skos:altLabel>DATVISUAL</skos:altLabel>
  <skos:broader rdf:resource='urn:comp:161'/>
  <skos:scopeNote>Knowledge capabilities and practices associated with
    extracting information and knowledge from extremely large
    data sets through interactions with visualization systems.
    Capabilities include developing and using advanced data
    visualization systems for data mining, pattern recognition
    and feature extraction for application to earth and space
    science data sets, as well as large engineering data sets
    for aviation and space systems. Also involves knowledge of
    state-of-the art modeling and simulation techniques and
    hardware for interpreting data and translating the data
    into animated images for use in scientific and education
    contexts. Includes understanding of computer science,
    digital
    animation three dimensional modeling, video generation and
    other data representation techniques. Also involves
    aesthetic skills in creating renditions of data with the
    power to communicate meaning.
  </skos:scopeNote>
  <nt2:status>Approved</nt2:status>
  <nt2:type>Descriptor</nt2:type>
  <nt2:inputdate>2006-12-13</nt2:inputdate>
  <dcterms:modified>2006-12-13</dcterms:modified>
  <nt2:code>1100</nt2:code>
 </skos:Concept>
 <skos:Concept rdf:about='urn:comp:162'>
  <skos:prefLabel>Integrated Logistics Support</skos:prefLabel>
  <skos:altLabel>INTLOGSUP</skos:altLabel>
  <skos:broader rdf:resource='urn:comp:1372'/>
  <skos:scopeNote>Knowledge, capabilities, concepts, and methods of strategic
    logistics planning, ad execution, emphasizing proactive
    techniques to ensure maximum logistics influence on systems
    acquisition as well as optimum life-cycle management of
    acquisition and legacy systems. Capabilities include
    planning, developing, implementing, and sustaining the
    Logistics Engineering activities necessary to satisfy
    support requirements while minimizing life-cycle costs;
    maintenance planning; manpower and support planning; supply
    support; support equipment to include test, measurement and
    diagnostic equipment (TMDE); providing technical data;
    training and training support; Logistics Support Analysis
    (LSA) for developed and modified hardware and software
    interfaces and components down to the piece part level on
    both a continual and iterative basis; generation of data
    inputs to the Logistics Management Information (LMI)
    database.
  </skos:scopeNote>
  <nt2:status>Approved</nt2:status>
  <nt2:type>Descriptor</nt2:type>
  <nt2:inputdate>2006-12-13</nt2:inputdate>
  <dcterms:modified>2006-12-13</dcterms:modified>
  <nt2:code>162</nt2:code>
 </skos:Concept>
 <skos:Concept rdf:about='urn:comp:94'>
  <skos:prefLabel>Microwave Systems</skos:prefLabel>
  <skos:altLabel>MICROSYS</skos:altLabel>
  <skos:broader rdf:resource='urn:comp:1339'/>
  <skos:scopeNote>Applies knowledge and practices associated with the design,
    analysis, development and test support for devices
    utilizing advanced technology for instrument (including
    data system) and communications (including telemetry)
    applications. Includes knowledge and capability in one or
    more of the following areas; antenna systems for general
    electromagnetic components, communications systems for
    space, suborbital, aircraft, and ground applications,
    instrument systems (both active and passive) for space,
    suborbital, aircraft, and ground applications, and systems
    and components for instrument, communication, telemetry,
    and radar applications.
  </skos:scopeNote>
  <nt2:status>Approved</nt2:status>
  <nt2:type>Descriptor</nt2:type>
  <nt2:inputdate>2006-12-13</nt2:inputdate>
  <dcterms:modified>2006-12-13</dcterms:modified>
  <nt2:code>94</nt2:code>
 </skos:Concept>
 <skos:Concept rdf:about='urn:comp:6'>
  <skos:prefLabel>Weather Observation and Forecasting</skos:prefLabel>
  <skos:altLabel>WOBSFR</skos:altLabel>
  <skos:broader rdf:resource='urn:comp:1372'/>
  <skos:scopeNote>Knowledge, capabilities and practices associated with
    developing or improving techniques for observing or
    forecasting local weather conditions in a coastal,
    semi-tropical environment. Specific capabilities include
    high resolution in-situ or remote sensing of wind,
    temperature and humidity; mesoscale meteorological
    modeling; high-resolution measurement of atmospheric
    electric fields and charge; radar meteorology; theoretical
    or numerical modeling of free electric charge generation
    and dissipation in clouds; and related areas. It also
    includes developing concepts of operation for the
    application of these technologies to Range operations;
    identifying and evaluating deficiencies in operational
    weather support for new or existing requirements;
    understanding the impact of meteorological variables on
    Range operations and systems; and knowledge of the
    application of weather data and technologies to the design
    of operational systems and procedures.
  </skos:scopeNote>
  <nt2:status>Approved</nt2:status>
  <nt2:type>Descriptor</nt2:type>
  <nt2:inputdate>2006-12-13</nt2:inputdate>
  <dcterms:modified>2006-12-13</dcterms:modified>
  <nt2:code>6</nt2:code>
 </skos:Concept>
 <skos:Concept rdf:about='urn:comp:111'>
  <skos:prefLabel>Advanced Measurement, Diagnostics, and Instrumentation</skos:prefLabel>
  <skos:altLabel>ADVMDI</skos:altLabel>
  <skos:broader rdf:resource='urn:comp:1363'/>
  <skos:scopeNote>Knowledge, capabilities, and practices associated with
    research and development, assessment, implementation, and
    integration of advanced measurement, flow diagnostics,
    instrumentation to understand and discover flow physics, to
    develop and validate physical/chemical models, and to
    support aerodynamic, aerothermodynamic, acoustic, and
    hypersonic airbreathing propulsion design and analysis of
    aerospace vehicles in ground facilities and in flight.
    Inherent within this competency is also the ability to
    resolve issues arising from test articles, data systems,
    and integrated measurement systems and their interactions.
  </skos:scopeNote>
  <nt2:status>Approved</nt2:status>
  <nt2:type>Descriptor</nt2:type>
  <nt2:inputdate>2006-12-13</nt2:inputdate>
  <dcterms:modified>2006-12-13</dcterms:modified>
  <nt2:code>111</nt2:code>
 </skos:Concept>
 <skos:Concept rdf:about='urn:comp:74'>
  <skos:prefLabel>Combustion Science</skos:prefLabel>
  <skos:altLabel>BOOMSCI</skos:altLabel>
  <skos:broader rdf:resource='urn:comp:1314'/>
  <skos:scopeNote>Employs knowledge, capabilities and practices of study of
    the science of burning and burning processes, including
    reaction kinetics and fuels, particularly related to heat
    transfer, combustion and fluid flow processes by which
    chemical energy is converted to propulsive power. Utilizes
    ground based or microgravity experiments to increase basic
    knowledge of combustion processes
  </skos:scopeNote>
  <nt2:status>Approved</nt2:status>
  <nt2:type>Descriptor</nt2:type>
  <nt2:inputdate>2006-12-13</nt2:inputdate>
  <dcterms:modified>2006-12-13</dcterms:modified>
  <nt2:code>74</nt2:code>
 </skos:Concept>
 <skos:Concept rdf:about='urn:comp:1034'>
  <skos:prefLabel>Systems Integration Engineering</skos:prefLabel>
  <skos:altLabel>INTSYSTEMS</skos:altLabel>
  <skos:broader rdf:resource='urn:comp:9'/>
  <skos:scopeNote>The Systems Integration Engineer (SIE) is responsible for
    integration of all engineering products and resources
    necessary for product development and is the single
    technical interface between the engineering organization
    and the program/project office (PPO) for a specific
    product. The SIE is responsible for vertical and horizontal
    integration of all engineering activities required for
    product delivery and is responsible to the PPO for cost and
    schedule performance under technical direction of a chief
    engineer. The SIE tracks design decisions and requirements,
    maintains techncial baselines, manages interfaces, provides
    input to the PPO for risk management, tracks cost and
    schedule, tracks technical performance, verifies
    requirements are met and reviews and audits program
    engineering support activities.
  </skos:scopeNote>
  <nt2:status>Approved</nt2:status>
  <nt2:type>Descriptor</nt2:type>
  <nt2:inputdate>2006-12-13</nt2:inputdate>
  <dcterms:modified>2006-12-13</dcterms:modified>
  <nt2:code>1034</nt2:code>
 </skos:Concept>
 <skos:Concept rdf:about='urn:comp:1086'>
  <skos:prefLabel>Personnel/EEO Law</skos:prefLabel>
  <skos:altLabel>PERSONLAW</skos:altLabel>
  <skos:broader rdf:resource='urn:comp:125'/>
  <skos:changeNote>???
  </skos:changeNote>
  <skos:scopeNote>Speciaized knowledge of matters related to employee and
    personnel issues, including but not limited to employee
    discipline and performance matters, MSPB, labor unions and
    collective bargaining, EEO, ADR, and litigation and appeals
    related to employment and personnel matters.
  </skos:scopeNote>
  <nt2:status>Approved</nt2:status>
  <nt2:type>Descriptor</nt2:type>
  <nt2:inputdate>2006-12-13</nt2:inputdate>
  <dcterms:dateAccepted>2006-04-05</dcterms:dateAccepted>
  <dcterms:modified>2006-12-18</dcterms:modified>
  <nt2:code>1086</nt2:code>
 </skos:Concept>
 <skos:Concept rdf:about='urn:comp:1078'>
  <skos:prefLabel>Information Resources Planning and Evaluation</skos:prefLabel>
  <skos:altLabel>BITPLAN</skos:altLabel>
  <skos:broader rdf:resource='urn:comp:131'/>
  <skos:scopeNote>Knowledge of the principles, methods, and techniques of IT
    assessment, planning, management, monitoring, and
    evaluation, such as IT baseline assessment, interagency
    functional analysis, contingency planning, and disaster
    recovery.
  </skos:scopeNote>
  <nt2:status>Approved</nt2:status>
  <nt2:type>Descriptor</nt2:type>
  <nt2:inputdate>2006-12-13</nt2:inputdate>
  <dcterms:modified>2006-12-13</dcterms:modified>
  <nt2:code>1078</nt2:code>
 </skos:Concept>
 <skos:Concept rdf:about='urn:comp:129'>
  <skos:prefLabel>Equal Opportunity Management</skos:prefLabel>
  <skos:altLabel>EEOMMT</skos:altLabel>
  <skos:broader rdf:resource='urn:comp:1189'/>
  <skos:scopeNote>Knowledge, capabilities, and practices associated with
    formulating, planning, implementing, managing, tracking and
    evaluating equal employment opportunity initiatives and
    programs. Includes the ability to fully integrate EO into
    all aspects of NASA’s mission as core values, to ensure a
    balanced and consistent implementation of statutory and
    administrative mandates such as maintaining an efficient
    and timely complaints processing program, an effective
    alternative dispute resolution program, and a comprehensive
    federally assisted and conducted non-discrimination
    program. Knowledge, capabilities and practices associated
    with creating an environment where all persons associated
    with NASA are treated fairly and without any form of
    unlawful discrimination in any agency program or activity.
    Includes the conceptualization, delivery and management of
    equal employment opportunity systems that meet NASA and
    Federal goals and objectives to eliminate discrimination
    and influence change in programs, practices and attitudes
    that are considered barriers to equal opportunity.
    Advisor/advocate role to agency officials to influence
    change and ensure compliance with relevant federal law,
    rules and regulations.
  </skos:scopeNote>
  <nt2:status>Approved</nt2:status>
  <nt2:type>Descriptor</nt2:type>
  <nt2:inputdate>2006-12-13</nt2:inputdate>
  <dcterms:modified>2006-12-13</dcterms:modified>
  <nt2:code>129</nt2:code>
 </skos:Concept>
 <skos:Concept rdf:about='urn:comp:72'>
  <skos:prefLabel>Advanced In-Space Propulsion</skos:prefLabel>
  <skos:altLabel>ADVPRO</skos:altLabel>
  <skos:broader rdf:resource='urn:comp:1314'/>
  <skos:narrower rdf:resource='urn:comp:1052'/>
  <skos:narrower rdf:resource='urn:comp:1050'/>
  <skos:narrower rdf:resource='urn:comp:1318'/>
  <skos:scopeNote>Research, development, design, testing and evaluation of
    propulsion technologies, such as nuclear propulsion, and
    space power generation systems to dramatically improve
    every aspect of in-space propulsion. Specialty knowledge in
    specific technologies such as nuclear propulsion, high
    powered electrical, solar voltaic, fuel cells, solar
    dynamic, and propellantless propulsion such as
    electrodynamic tethers and beamed energy.
  </skos:scopeNote>
  <nt2:status>Approved</nt2:status>
  <nt2:type>Descriptor</nt2:type>
  <nt2:inputdate>2006-12-13</nt2:inputdate>
  <dcterms:modified>2006-12-13</dcterms:modified>
  <nt2:code>72</nt2:code>
 </skos:Concept>
 <skos:Concept rdf:about='urn:comp:112'>
  <skos:prefLabel>Facilities Engineering and Management</skos:prefLabel>
  <skos:altLabel>FACENG</skos:altLabel>
  <skos:broader rdf:resource='urn:comp:1159'/>
  <skos:narrower rdf:resource='urn:comp:1096'/>
  <skos:narrower rdf:resource='urn:comp:1098'/>
  <skos:narrower rdf:resource='urn:comp:1090'/>
  <skos:narrower rdf:resource='urn:comp:1092'/>
  <skos:narrower rdf:resource='urn:comp:1091'/>
  <skos:narrower rdf:resource='urn:comp:1097'/>
  <skos:scopeNote>Knowledge of facilities engineering , facility evaluation,
    cost, schedules and formulation of performance requirements
    and alternative analysis/scenarios for key facilities.
    General knowledge of architectural, civil, mechanical and
    electrical engineering disciplines. Knowledge of project
    management and control including life-cycle costs,
    engineering economics, and project planning and evaluation
    including scope, cost and schedule and program controls
    including earned value management or other measure for
    facility project controls. Also requires knowledge of
    construction contracting and contractor oversight and
    contracts management.
  </skos:scopeNote>
  <nt2:status>Approved</nt2:status>
  <nt2:type>Descriptor</nt2:type>
  <nt2:inputdate>2006-12-13</nt2:inputdate>
  <dcterms:modified>2006-12-13</dcterms:modified>
  <nt2:code>112</nt2:code>
 </skos:Concept>
 <skos:Concept rdf:about='urn:comp:1372'>
  <skos:prefLabel>Mission Operations Competency Suite</skos:prefLabel>
  <skos:broader rdf:resource='urn:comp:1371'/>
  <skos:narrower rdf:resource='urn:comp:3'/>
  <skos:narrower rdf:resource='urn:comp:162'/>
  <skos:narrower rdf:resource='urn:comp:30'/>
  <skos:narrower rdf:resource='urn:comp:4'/>
  <skos:narrower rdf:resource='urn:comp:5'/>
  <skos:narrower rdf:resource='urn:comp:147'/>
  <skos:narrower rdf:resource='urn:comp:153'/>
  <skos:narrower rdf:resource='urn:comp:6'/>
  <nt2:status>Approved</nt2:status>
  <nt2:type>Descriptor</nt2:type>
  <nt2:inputdate>2006-12-13</nt2:inputdate>
  <dcterms:modified>2006-12-13</dcterms:modified>
  <nt2:code>1372</nt2:code>
 </skos:Concept>
 <skos:Concept rdf:about='urn:comp:1424'>
  <skos:prefLabel>Physical Sciences Competency Suite</skos:prefLabel>
  <skos:broader rdf:resource='urn:comp:1406'/>
  <skos:narrower rdf:resource='urn:comp:65'/>
  <skos:narrower rdf:resource='urn:comp:43'/>
  <skos:narrower rdf:resource='urn:comp:42'/>
  <skos:narrower rdf:resource='urn:comp:107'/>
  <skos:narrower rdf:resource='urn:comp:56'/>
  <nt2:status>Approved</nt2:status>
  <nt2:type>Descriptor</nt2:type>
  <nt2:inputdate>2006-12-13</nt2:inputdate>
  <dcterms:modified>2006-12-13</dcterms:modified>
  <nt2:code>1424</nt2:code>
 </skos:Concept>
 <skos:Concept rdf:about='urn:comp:1088'>
  <skos:prefLabel>Institutional Environmental Planning/NEPA</skos:prefLabel>
  <skos:altLabel>ENVPLAN</skos:altLabel>
  <skos:broader rdf:resource='urn:comp:133'/>
  <skos:scopeNote>Uses knowledge of environmental engineering, environmental
    law, economics and the physical sciences to fully consider
    the possible environmental effects, along with technical,
    economic, and other factors, in the earliest planning of
    proposed NASA Programs, Projects, and related activities.
    Implements the requirements of the National Environmental
    Policy Act (NEPA) including developing and reviewing NEPA
    documentation including Environmental Assessments,
    Environmental Impact Statements, Findings of No Significant
    Impact, and Records of Decision. Coordinates public
    meetings to solicit input on major Agency actions.
  </skos:scopeNote>
  <nt2:status>Approved</nt2:status>
  <nt2:type>Descriptor</nt2:type>
  <nt2:inputdate>2006-12-13</nt2:inputdate>
  <dcterms:modified>2006-12-13</dcterms:modified>
  <nt2:code>1088</nt2:code>
 </skos:Concept>
 <skos:Concept rdf:about='urn:comp:137'>
  <skos:prefLabel>Education Programs and Technologies</skos:prefLabel>
  <skos:altLabel>EDTECH</skos:altLabel>
  <skos:broader rdf:resource='urn:comp:1125'/>
  <skos:scopeNote>Knowledge, capabilities and practices associated with the
    research and application of education programs, standards,
    requirements, activities and services relevant to the
    fields and disciplines of science, technology, engineering,
    and mathematics (STEM) within the contexts of pre-college,
    higher education, and non-traditional learning. Includes
    knowledge of education concepts and principles, curriculum
    development, infrastructure, audiences, instructional
    technologies and distance learning tools, and trends in
    order for NASA to appropriately influence and contribute to
    national and state education initiatives and requirements
    through the use of NASA's unique assets. Includes knowledge
    of NASA Enterprise and Center-based research and technology
    needs, and ability to align education activities and
    programs with these needs. Includes knowledge of
    demographic and geographic dynamics that influence the
    educational effectiveness and success within the various
    student and educator communities.
  </skos:scopeNote>
  <nt2:status>Approved</nt2:status>
  <nt2:type>Descriptor</nt2:type>
  <nt2:inputdate>2006-12-13</nt2:inputdate>
  <dcterms:modified>2006-12-13</dcterms:modified>
  <nt2:code>137</nt2:code>
 </skos:Concept>
 <skos:Concept rdf:about='urn:comp:115'>
  <skos:prefLabel>Professional Administrative Operations</skos:prefLabel>
  <skos:altLabel>PROFADMOPS</skos:altLabel>
  <skos:broader rdf:resource='urn:comp:1189'/>
  <skos:scopeNote>Knowledge, capabilities and practices associated with the
    support of administrative and management activities to
    facilitate organizational and mission goals and objectives.
    This competency requires knowledge of the appropriate
    rules, regulations, processes and associated systems within
    various enabling functions which may include human
    resources management, resource management, employee support
    services, documentation, procurement and financial
    management.
  </skos:scopeNote>
  <nt2:status>Approved</nt2:status>
  <nt2:type>Descriptor</nt2:type>
  <nt2:inputdate>2006-12-13</nt2:inputdate>
  <dcterms:modified>2006-12-13</dcterms:modified>
  <nt2:code>115</nt2:code>
 </skos:Concept>
 <skos:Concept rdf:about='urn:comp:172'>
  <skos:prefLabel>Business Work &amp; Team Management</skos:prefLabel>
  <skos:altLabel>BUSWORKMMT</skos:altLabel>
  <skos:broader rdf:resource='urn:comp:1394'/>
  <skos:scopeNote>Knowledge, capabilities and practices associated with
    individuals that must understand and manage both the
    aspects of functional business opertions, as well as
    management of employees and/or teams. This pseudo
    competency requires the supervisor or lead to have the
    following competencies:
    Any business management related competency
    Employee &amp; Team Leadership
    Work Performance Leadership
  </skos:scopeNote>
  <nt2:status>Approved</nt2:status>
  <nt2:type>Descriptor</nt2:type>
  <nt2:inputdate>2006-12-13</nt2:inputdate>
  <dcterms:modified>2006-12-13</dcterms:modified>
  <nt2:code>172</nt2:code>
 </skos:Concept>
 <skos:Concept rdf:about='urn:comp:59'>
  <skos:prefLabel>Biomimetics</skos:prefLabel>
  <skos:altLabel>BIOMIMETIC</skos:altLabel>
  <skos:broader rdf:resource='urn:comp:1244'/>
  <skos:scopeNote>Knowledge and capability to research and further study
    natural processes which have potential to be deciphered,
    mimicked and adopted in technology applications based on
    biological systems such as environmental heat sensors,
    retinal or iris scans or face recognition technology. Also
    includes capabilities in the area of neural electric
    machine control.
  </skos:scopeNote>
  <nt2:status>Approved</nt2:status>
  <nt2:type>Descriptor</nt2:type>
  <nt2:inputdate>2006-12-13</nt2:inputdate>
  <dcterms:modified>2006-12-13</dcterms:modified>
  <nt2:code>59</nt2:code>
 </skos:Concept>
 <skos:Concept rdf:about='urn:comp:147'>
  <skos:prefLabel>Program/Project Analysis</skos:prefLabel>
  <skos:altLabel>PROJANALYS</skos:altLabel>
  <skos:broader rdf:resource='urn:comp:1372'/>
  <skos:scopeNote>Knowledge, capabilities and practices associated with
    formulating, planning, implementing, tracking and
    evaluating work and its associated requirements and risks,
    ranging from one-time projects to program-level work.
    Critical ability is to develop, analyze, and oversee
    resources, schedule, and management controls needed by the
    Program/Project manager to achieve the appropriate balance
    between resources, schedule, and technical objectives.
    Includes knowledge associated with finance, budgeting,
    schedule, configuration management, and project controls.
  </skos:scopeNote>
  <nt2:status>Approved</nt2:status>
  <nt2:type>Descriptor</nt2:type>
  <nt2:inputdate>2006-12-13</nt2:inputdate>
  <dcterms:modified>2006-12-13</dcterms:modified>
  <nt2:code>147</nt2:code>
 </skos:Concept>
 <skos:Concept rdf:about='urn:comp:88'>
  <skos:prefLabel>Geospatial Science and Technologies</skos:prefLabel>
  <skos:altLabel>GEOSPATIAL</skos:altLabel>
  <skos:broader rdf:resource='urn:comp:1415'/>
  <skos:scopeNote>Applies knowledge and practices of geospatial science and
    has the ability to utilize and/or develop the tools for
    acquiring, storing, analyzing, and outputting data in
    multiple dimensions, as referenced to the earth by some
    type of real-world coordinate system (eg, a map
    projection). The ability to reference a geographic location
    as an important component in the analyses of effects or
    trends in biological and physical socio-economic resources.
    Understanding of and ability to use a variety of technology
    tools, such as geographic information systems (GIS), remote
    sensing, thematic mapping, image processing, satellite
    positioning systems such as the Global Positioning System
    (GPS), and telemetry.
  </skos:scopeNote>
  <nt2:status>Approved</nt2:status>
  <nt2:type>Descriptor</nt2:type>
  <nt2:inputdate>2006-12-13</nt2:inputdate>
  <dcterms:modified>2006-12-13</dcterms:modified>
  <nt2:code>88</nt2:code>
 </skos:Concept>
 <skos:Concept rdf:about='urn:comp:149'>
  <skos:prefLabel>Mishap Investigation</skos:prefLabel>
  <skos:altLabel>MISHAPINV</skos:altLabel>
  <skos:broader rdf:resource='urn:comp:1381'/>
  <skos:scopeNote>A NASA employee who understands NASA mishap investigation
    policy, and requirements, and has the skills to perform all
    aspects of mishap investigation including preserving,
    collecting, and impounding evidence, interviewing,
    conducting analyses, drawing collusions, generating
    recommendations, and writing NASA mishap reports.
  </skos:scopeNote>
  <nt2:status>Approved</nt2:status>
  <nt2:type>Descriptor</nt2:type>
  <nt2:inputdate>2006-12-13</nt2:inputdate>
  <dcterms:modified>2006-12-13</dcterms:modified>
  <nt2:code>149</nt2:code>
 </skos:Concept>
 <skos:Concept rdf:about='urn:comp:1209'>
  <skos:prefLabel>Engineering of Systems Competency Suite</skos:prefLabel>
  <skos:broader rdf:resource='urn:comp:1208'/>
  <skos:narrower rdf:resource='urn:comp:8'/>
  <skos:narrower rdf:resource='urn:comp:11'/>
  <skos:narrower rdf:resource='urn:comp:9'/>
  <skos:narrower rdf:resource='urn:comp:24'/>
  <skos:narrower rdf:resource='urn:comp:114'/>
  <skos:narrower rdf:resource='urn:comp:7'/>
  <skos:narrower rdf:resource='urn:comp:10'/>
  <nt2:status>Approved</nt2:status>
  <nt2:type>Descriptor</nt2:type>
  <nt2:inputdate>2006-12-13</nt2:inputdate>
  <dcterms:modified>2006-12-13</dcterms:modified>
  <nt2:code>1209</nt2:code>
 </skos:Concept>
 <skos:Concept rdf:about='urn:comp:124'>
  <skos:prefLabel>Acquisition and Contract Management</skos:prefLabel>
  <skos:altLabel>CONMMT</skos:altLabel>
  <skos:broader rdf:resource='urn:comp:1150'/>
  <skos:narrower rdf:resource='urn:comp:1093'/>
  <skos:narrower rdf:resource='urn:comp:1094'/>
  <skos:narrower rdf:resource='urn:comp:1095'/>
  <skos:scopeNote>Knowledge, capabilities and practices associated with each
    phase of the acquisition and contract management lifecycle
    including requirement analysis, market research,
    acquisition planning and strategy, solicitation, proposal
    evaluation, negotiation, determination of price
    reasonableness, selection, contract management, and
    performance assessment. Requires understanding of
    applicable public laws, executive orders, Federal
    regulations, Agency requirements, policies, and
    initiatives. Requires knowledge of contracts to review
    products and services to determine if they are in
    compliance with contract terms and conditions. Includes
    ability to assess technical requirements needed to support
    program and project implementation and provide guidance and
    direction to contractors to ensure delivery and quality of
    services and products. Ability to use contract or
    acquisition instruments and surveillance systems as
    necessary to ensure contract or acquisition requirements
    are being met throughout the life of the contract.
  </skos:scopeNote>
  <nt2:status>Approved</nt2:status>
  <nt2:type>Descriptor</nt2:type>
  <nt2:inputdate>2006-12-13</nt2:inputdate>
  <dcterms:modified>2006-12-13</dcterms:modified>
  <nt2:code>124</nt2:code>
 </skos:Concept>
 <skos:Concept rdf:about='urn:comp:125'>
  <skos:prefLabel>Legal Application Practice</skos:prefLabel>
  <skos:altLabel>LEGALAPP</skos:altLabel>
  <skos:broader rdf:resource='urn:comp:1125'/>
  <skos:narrower rdf:resource='urn:comp:1113'/>
  <skos:narrower rdf:resource='urn:comp:1085'/>
  <skos:narrower rdf:resource='urn:comp:1087'/>
  <skos:narrower rdf:resource='urn:comp:1084'/>
  <skos:narrower rdf:resource='urn:comp:1083'/>
  <skos:narrower rdf:resource='urn:comp:1112'/>
  <skos:narrower rdf:resource='urn:comp:1086'/>
  <skos:changeNote>Introduced ???
    Modified for 6a by ???
    New child nodes added for International Law and Commercial
    Law.
  </skos:changeNote>
  <skos:scopeNote>Member in good standing of the bar of either a Federal
    court or the highest court of any state in the United
    States or the District of Columbia. Knowledge, capabilities
    and practices associated with representation, counseling,
    advising, researching, performing, and / or supervising
    professional legal work in the administration of applicable
    statutes, regulations, Executive Orders, rules, and case
    law. This includes knowledge of topics such as, but not
    limited to civil and administrative law, procurement,
    claims, , fiscal matters, personnel matters, environmental
    matters, FOIA, Congressional inquiries, ethics,
    intellectual property and data rights, litigation, and
    appeals.
  </skos:scopeNote>
  <nt2:status>Approved</nt2:status>
  <nt2:type>Descriptor</nt2:type>
  <nt2:inputdate>2006-12-13</nt2:inputdate>
  <dcterms:dateAccepted>2006-04-05</dcterms:dateAccepted>
  <dcterms:modified>2006-12-18</dcterms:modified>
  <nt2:code>125</nt2:code>
 </skos:Concept>
 <skos:Concept rdf:about='urn:comp:41'>
  <skos:prefLabel>Human Factors Engineering</skos:prefLabel>
  <skos:altLabel>HUMFACTENG</skos:altLabel>
  <skos:broader rdf:resource='urn:comp:1244'/>
  <skos:narrower rdf:resource='urn:comp:1019'/>
  <skos:narrower rdf:resource='urn:comp:1024'/>
  <skos:narrower rdf:resource='urn:comp:1020'/>
  <skos:narrower rdf:resource='urn:comp:1022'/>
  <skos:narrower rdf:resource='urn:comp:1027'/>
  <skos:narrower rdf:resource='urn:comp:1025'/>
  <skos:narrower rdf:resource='urn:comp:1023'/>
  <skos:narrower rdf:resource='urn:comp:1021'/>
  <skos:narrower rdf:resource='urn:comp:1026'/>
  <skos:scopeNote>Knowledge and capabilities to apply human factors
    engineering principles, standards, design guides,
    regulations, and advisory material to the .design, test,
    evaluation, operation, and maintenance of systems and
    processes. Knowledge of the physical and psychological
    processes, capabilities, skill levels, and limitations of
    humans, such as the science and practical application of
    experimental psychology, cognitive psychology, human
    reliability, anthropometrics, biomechanics, and
    psychophysiology. Knowledge of hardware and software
    human-interface design principles, modalities (e.g.
    physical, visual, auditory, verbal), methods (e.g. field
    studies, analysis, modeling, prototyping, laboratory
    experiments, simulations, mockups, database reviews) and
    tools. The ability to define and analyze human engineering
    requirements, formulate human performance criteria, develop
    guidelines, develop system concepts, designs, and
    prototypes; evaluate human-centered technologies, and
    develop training curricula for application to processes and
    systems.
  </skos:scopeNote>
  <nt2:status>Approved</nt2:status>
  <nt2:type>Descriptor</nt2:type>
  <nt2:inputdate>2006-12-13</nt2:inputdate>
  <dcterms:modified>2006-12-13</dcterms:modified>
  <nt2:code>41</nt2:code>
 </skos:Concept>
 <skos:Concept rdf:about='urn:comp:1015'>
  <skos:prefLabel>Manual Control Fundamental Research</skos:prefLabel>
  <skos:altLabel>HFRMANCNTL</skos:altLabel>
  <skos:broader rdf:resource='urn:comp:40'/>
  <skos:scopeNote>TBD
  </skos:scopeNote>
  <nt2:status>Approved</nt2:status>
  <nt2:type>Descriptor</nt2:type>
  <nt2:inputdate>2006-12-13</nt2:inputdate>
  <dcterms:modified>2006-12-13</dcterms:modified>
  <nt2:code>1015</nt2:code>
 </skos:Concept>
 <skos:Concept rdf:about='urn:comp:1060'>
  <skos:prefLabel>Metallurgy</skos:prefLabel>
  <skos:altLabel>MSEMETAL</skos:altLabel>
  <skos:broader rdf:resource='urn:comp:66'/>
  <skos:scopeNote>Knowledge capability and practices associated with research
    into the production, characteristics, structure,
    properties, and performance of metallic materials and the
    design, development, processing and testing of those metals
    within aerospace structures such as flight systems, ground
    support and facility systems. Includes the development of
    math models and statistical methods for assessment of the
    durability and response of metallic materials to
    environmental conditions, composition, processes and
    applied forces. Includes broad knowledge of the
    metallurgical discipline, including characteristics of
    metallic alloy types and methods of processing metals into
    final products such as molding, shaping, forming, thermal
    treatment, joining, electrochemical processes, corrosion
    control, superalloys, powder metallurgy, metal matrix
    composites, and nanostructures. Also includes broad
    capabilities in metallurgical analysis, evaluation and
    testing , including surface, microscopic, chemical,
    crystallography, internal micro and macrostructural
    analysis, and practices in physical and mechanical testing
    to determine and achieve design criteria such as strength,
    hardness, toughness, corrosion behavior and performance in
    extremes of environment and temperature, with emphasis on
    evaluation of metals under operating environments to
    produce reliable and quality materials that will resist
    expected failue modes such as corrosion, stress
    concentration, metal fatigue, creep and environmental
    stress fracture. Includes analysis of the nature, behavior,
    and physical characteristics of metals and their alloys,
    including the mechanisms and effects by which materials
    react to stresses, environments, and processes in order to
    select, plan, design, develop processing methods and
    produce materials with specific and exacting properties for
    aerospace applications.
  </skos:scopeNote>
  <nt2:status>Approved</nt2:status>
  <nt2:type>Descriptor</nt2:type>
  <nt2:inputdate>2006-12-13</nt2:inputdate>
  <dcterms:modified>2006-12-13</dcterms:modified>
  <nt2:code>1060</nt2:code>
 </skos:Concept>
 <skos:Concept rdf:about='urn:comp:1007'>
  <skos:prefLabel>Perception and Psychophysics Fundamental Research</skos:prefLabel>
  <skos:altLabel>HFRPERCEPT</skos:altLabel>
  <skos:broader rdf:resource='urn:comp:40'/>
  <skos:scopeNote>TBD (includes vision, audition, haptics, vestibular,
    multimodal)
  </skos:scopeNote>
  <nt2:status>Approved</nt2:status>
  <nt2:type>Descriptor</nt2:type>
  <nt2:inputdate>2006-12-13</nt2:inputdate>
  <dcterms:modified>2006-12-13</dcterms:modified>
  <nt2:code>1007</nt2:code>
 </skos:Concept>
 <skos:Concept rdf:about='urn:comp:138'>
  <skos:prefLabel>Nuclear Engineering /Propulsion</skos:prefLabel>
  <skos:altLabel>NUCLEARENG</skos:altLabel>
  <skos:broader rdf:resource='urn:comp:1314'/>
  <skos:scopeNote>Knowledge of scientific and engineering principles
    associated with the safe design and operations of
    terrestrial and non-terrestrial nuclear reactor systems and
    radioisotope decay power systems. Knowledge and practice of
    neutron fission and
    decay of nuclear material, radioactivity
    determination/calculation/shielding due to fission and
    decay of nuclear materials, thermodynamics, nuclear/quantum
    physics, materials science, operations and control
    principles of nuclear reactors, simulation of reactor
    operations, health-physics effects of reactor radioactivity
    on humans, and probabilistic risk assessment. Ability to
    develop design concepts for potential nuclear propulsion
    systems, evaluating proposed designs and doing tradeoffs to
    determine which concepts can be incorporated into future
    space missions.
  </skos:scopeNote>
  <nt2:status>Approved</nt2:status>
  <nt2:type>Descriptor</nt2:type>
  <nt2:inputdate>2006-12-13</nt2:inputdate>
  <dcterms:modified>2006-12-13</dcterms:modified>
  <nt2:code>138</nt2:code>
 </skos:Concept>
 <skos:Concept rdf:about='urn:comp:139'>
  <skos:prefLabel>Software Assurance Engineering</skos:prefLabel>
  <skos:altLabel>SWASSURANCE</skos:altLabel>
  <skos:broader rdf:resource='urn:comp:1381'/>
  <skos:scopeNote>Knowledge, capabilities and practices associated with the
    planning, organizing, performing, monitoring and directing
    software assurance activities for software acquired and
    developed for all phases of the product lifecycle including
    product concept, acquisition, contractor selection and
    oversight, requirements, design, implementation, problem
    reporting, corrective action, verification and validation,
    testing, operations, maintenance, and retirement. SA
    practices include software product assurance, process
    assurance, quality, reliability, safety, security, risk
    management, verification, validation, and independent
    verification and validation. Additionally, demonstrate
    knowledge of current software and systems engineering
    practices, languages, management, planning, standards,
    procedures, and recommended processes. Assures that process
    and product standards are appropriate, implemented
    correctly, followed, and improved.
  </skos:scopeNote>
  <nt2:status>Approved</nt2:status>
  <nt2:type>Descriptor</nt2:type>
  <nt2:inputdate>2006-12-13</nt2:inputdate>
  <dcterms:modified>2006-12-13</dcterms:modified>
  <nt2:code>139</nt2:code>
 </skos:Concept>
 <skos:Concept rdf:about='urn:comp:126'>
  <skos:prefLabel>Security &amp; Program Protection</skos:prefLabel>
  <skos:altLabel>SECURITY</skos:altLabel>
  <skos:broader rdf:resource='urn:comp:1159'/>
  <skos:narrower rdf:resource='urn:comp:WQQ-564'/>
  <skos:narrower rdf:resource='urn:comp:WQQ-565'/>
  <skos:narrower rdf:resource='urn:comp:1077'/>
  <skos:narrower rdf:resource='urn:comp:1074'/>
  <skos:narrower rdf:resource='urn:comp:1075'/>
  <skos:narrower rdf:resource='urn:comp:1076'/>
  <skos:narrower rdf:resource='urn:comp:1072'/>
  <skos:scopeNote>Knowledge, capabilities and practices associated with
    providing security to protect facilities, personnel and
    programs. Ability to develop, implement and manage
    processes and programs involving law enforcement,
    counter-intelligence and counter-terrorism investigations,
    and security support programs including physical,
    information, personnel and industrial security.
  </skos:scopeNote>
  <nt2:status>Approved</nt2:status>
  <nt2:type>Descriptor</nt2:type>
  <nt2:inputdate>2006-12-13</nt2:inputdate>
  <dcterms:modified>2006-12-13</dcterms:modified>
  <nt2:code>126</nt2:code>
 </skos:Concept>
 <skos:Concept rdf:about='urn:comp:27'>
  <skos:prefLabel>Safety Engineering and Assurance</skos:prefLabel>
  <skos:altLabel>SAFENG</skos:altLabel>
  <skos:broader rdf:resource='urn:comp:1381'/>
  <skos:narrower rdf:resource='urn:comp:1107'/>
  <skos:narrower rdf:resource='urn:comp:1105'/>
  <skos:narrower rdf:resource='urn:comp:1104'/>
  <skos:narrower rdf:resource='urn:comp:1106'/>
  <skos:changeNote>???
  </skos:changeNote>
  <skos:scopeNote>Knowledge of scientific, engineering and management
    principles for ensuring safety of missions and systems
    through controlled design, development, operation, and
    disposal. Includes ability to develop safety policies and
    to use analytical tools such as hazard analysis, failure
    modes and effects analysis, fault tree analysis, and
    probabilistic risk assessment, and develop technical
    reports of results, conclusions, and recommendations to
    support risk-informed decision-making. Develop safety
    performance measures and apply criteria and techniques such
    as safety audits, assessments, inspections, trend analysis,
    precursor analysis, and sampling to monitor safety
    performance and to identify and eliminate/mitigate hazards
    and achieve an acceptable level of risk, within the
    constraints of operational effectiveness and suitability,
    time, and cost throughout all phases of the system
    (mission) life cycle.
  </skos:scopeNote>
  <nt2:status>Approved</nt2:status>
  <nt2:type>Descriptor</nt2:type>
  <nt2:inputdate>2006-12-13</nt2:inputdate>
  <dcterms:dateAccepted>2005-12-07</dcterms:dateAccepted>
  <dcterms:modified>2006-12-18</dcterms:modified>
  <nt2:code>27</nt2:code>
 </skos:Concept>
 <skos:Concept rdf:about='urn:comp:13'>
  <skos:prefLabel>Electrical and Electronic Systems</skos:prefLabel>
  <skos:altLabel>ELSYS</skos:altLabel>
  <skos:broader rdf:resource='urn:comp:1294'/>
  <skos:narrower rdf:resource='urn:comp:1043'/>
  <skos:narrower rdf:resource='urn:comp:1045'/>
  <skos:narrower rdf:resource='urn:comp:1042'/>
  <skos:narrower rdf:resource='urn:comp:1044'/>
  <skos:scopeNote>Knowledge of engineering design and analysis, development
    and research of electrical systems and components for air,
    space and ground systems and instruments. Includes
    knowledge of electrical integration (cable
    design/development/testing) such as electrical / electronic
    design requirements definition, subsystem and circuit
    analysis, test procedure development, and safety analysis.
    Includes knowledge of analog and digital electrical systems
    engineering, EEE parts, electronic packaging design and
    tools, reliability and environmental effects, power
    generation, distribution, storage and conditioning systems.
    Knowledge of thermal analysis of printed circuit boards and
    use to analyze data to optimize design of flight
    electronics.
  </skos:scopeNote>
  <nt2:status>Approved</nt2:status>
  <nt2:type>Descriptor</nt2:type>
  <nt2:inputdate>2006-12-13</nt2:inputdate>
  <dcterms:modified>2006-12-13</dcterms:modified>
  <nt2:code>13</nt2:code>
 </skos:Concept>
 <skos:Concept rdf:about='urn:comp:4'>
  <skos:prefLabel>Mission Execution</skos:prefLabel>
  <skos:altLabel>MISEXC</skos:altLabel>
  <skos:broader rdf:resource='urn:comp:1372'/>
  <skos:scopeNote>Knowledge, capabilities and practices associated with the
    execution of missions, including pre-launch, launch,
    in-orbit and recovery operations for space flight, or
    conducting safe, efficient and effective operation of
    research or training aircraft. Manage command and control
    activities, payload integration and operations, robotic
    operations and EVA operations according to mission
    objectives including the technical activities and real-time
    decision -making and problem resolution during mission
    critical operations.
  </skos:scopeNote>
  <nt2:status>Approved</nt2:status>
  <nt2:type>Descriptor</nt2:type>
  <nt2:inputdate>2006-12-13</nt2:inputdate>
  <dcterms:modified>2006-12-13</dcterms:modified>
  <nt2:code>4</nt2:code>
 </skos:Concept>
 <skos:Concept rdf:about='urn:comp:63'>
  <skos:prefLabel>Structural Systems</skos:prefLabel>
  <skos:altLabel>STRSYS</skos:altLabel>
  <skos:broader rdf:resource='urn:comp:1347'/>
  <skos:scopeNote>Knowledge, capability and practices associated with using
    and modifying advanced analytical and computational methods
    to design, develop, test and research the characteristics
    and performance of structures. Includes the development of
    structural math models for and comprehensive assessment of
    air, space and ground structures, the analysis of the
    models to determine structural response to multiple
    external and internal environmental conditions, and
    analysis of flight and test data for structural systems.
    Includes broad knowledge of structures disciplines
    including structural dynamics, structural mechanics,
    structural acoustics, mechanisms, electro-mechanical
    devices, aeroelasticity, impact, damage tolerance and
    structural life prediction. Also involves research into
    measurement, instrument and test systems to assess
    structural characteristics and risks, and ensure system
    integration.
  </skos:scopeNote>
  <nt2:status>Notvalid</nt2:status>
  <nt2:type>Descriptor</nt2:type>
  <nt2:inputdate>2004-10-08</nt2:inputdate>
  <dcterms:dateAccepted>2004-10-08</dcterms:dateAccepted>
  <dcterms:modified>2006-12-18</dcterms:modified>
  <nt2:notValidDate>2005-12-07</nt2:notValidDate>
  <nt2:code>63</nt2:code>
 </skos:Concept>
 <skos:Concept rdf:about='urn:comp:167'>
  <skos:prefLabel>Master Planning</skos:prefLabel>
  <skos:altLabel>MASTERPLAN</skos:altLabel>
  <skos:broader rdf:resource='urn:comp:1159'/>
  <skos:scopeNote>Knowledge of strategic and long-term planning for
    operations, research or development activities at the
    Center level. Knowledge required to develop functional and
    overall Center requirements including fit of specific
    facility needs and requirements as well as workflow and
    long-term scheduling. Includes knowledge required to
    coordinate and incorporate the necessary facilities and
    other building and infrastructure to satisfy all
    functional, institutional needs to meet mission
    requirements. Specialized knowledge of transportation
    modeling as well as broad aspects of community interface
    for emergency services and other requirements of large
    complex industrial installations.
  </skos:scopeNote>
  <nt2:status>Approved</nt2:status>
  <nt2:type>Descriptor</nt2:type>
  <nt2:inputdate>2006-12-13</nt2:inputdate>
  <dcterms:modified>2006-12-13</dcterms:modified>
  <nt2:code>167</nt2:code>
 </skos:Concept>
 <skos:Concept rdf:about='urn:comp:1117'>
  <skos:prefLabel>Employee Benefits</skos:prefLabel>
  <skos:altLabel>HCMEMPBENF</skos:altLabel>
  <skos:broader rdf:resource='urn:comp:128'/>
  <skos:scopeNote>Knowledge of HR concepts, principles, and practices related
    to retirement, insurance, injury compensation, and other
    employee benefits programs..
  </skos:scopeNote>
  <nt2:status>Approved</nt2:status>
  <nt2:type>Descriptor</nt2:type>
  <nt2:inputdate>2006-04-05</nt2:inputdate>
  <dcterms:dateAccepted>2006-04-05</dcterms:dateAccepted>
  <dcterms:modified>2006-12-18</dcterms:modified>
  <nt2:code>1117</nt2:code>
 </skos:Concept>
 <skos:Concept rdf:about='urn:comp:1406'>
  <skos:prefLabel>Science Knowledge Domain</skos:prefLabel>
  <skos:broader rdf:resource='urn:comp:1438'/>
  <skos:narrower rdf:resource='urn:comp:1430'/>
  <skos:narrower rdf:resource='urn:comp:1415'/>
  <skos:narrower rdf:resource='urn:comp:1424'/>
  <skos:narrower rdf:resource='urn:comp:1407'/>
  <nt2:status>Approved</nt2:status>
  <nt2:type>Descriptor</nt2:type>
  <nt2:inputdate>2006-12-13</nt2:inputdate>
  <dcterms:modified>2007-01-11</dcterms:modified>
  <nt2:code>1406</nt2:code>
 </skos:Concept>
 <skos:Concept rdf:about='urn:comp:46'>
  <skos:prefLabel>Biology and Biogeochemistry of Ecosystems</skos:prefLabel>
  <skos:altLabel>BBECO</skos:altLabel>
  <skos:broader rdf:resource='urn:comp:1415'/>
  <skos:scopeNote>Apply knowledge of biology, biogeochemistry of ecosystems
    and the global carbon cycle to research, understand and
    predict how terrestrial and marine ecosystems change.
    Research ecosystems as they are affected by human activity,
    and as they change due to their own intrinsic biological
    dynamics, and as they respond to climatic variations and,
    in turn, affect climate. Emphasis is on an understanding of
    the processes of the Earth system that affect its capacity
    for biological productivity, explain the role of the
    biosphere in Earth system function, and promote proactive
    ecological stewardship. Ability to understand, study and
    properly document changes in land cover and land use.
  </skos:scopeNote>
  <nt2:status>Approved</nt2:status>
  <nt2:type>Descriptor</nt2:type>
  <nt2:inputdate>2006-12-13</nt2:inputdate>
  <dcterms:modified>2006-12-13</dcterms:modified>
  <nt2:code>46</nt2:code>
 </skos:Concept>
 <skos:Concept rdf:about='urn:comp:23'>
  <skos:prefLabel>Terrestrial &amp; Planetary Environmental Science and Engineering</skos:prefLabel>
  <skos:altLabel>PLANETENV</skos:altLabel>
  <skos:broader rdf:resource='urn:comp:1363'/>
  <skos:scopeNote>Knowledge of composition, elements, behaviors and impact of
    the terrestrial and planetary environments on the design,
    development, testing and operation of systems and
    components for aerospace vehicles and satellites. Involves
    understanding of atmospheric variables such as wind
    profiles, turbulence, cloud cover, ice/frost formation.
    Involves the ability to perform analyses to define the
    environments, quantify their effect on vehicle design,
    development and operations and perform trade-off studies to
    optimize performance and assess risk.
  </skos:scopeNote>
  <nt2:status>Approved</nt2:status>
  <nt2:type>Descriptor</nt2:type>
  <nt2:inputdate>2006-12-13</nt2:inputdate>
  <dcterms:modified>2006-12-13</dcterms:modified>
  <nt2:code>23</nt2:code>
 </skos:Concept>
 <skos:Concept rdf:about='urn:comp:1102'>
  <skos:prefLabel>Clerical Student Trainee</skos:prefLabel>
  <skos:altLabel>STUCLERICAL</skos:altLabel>
  <skos:broader rdf:resource='urn:comp:174'/>
  <skos:scopeNote>This is a training and development competency for employees
    who are classified as Clerical Student Trainees.
  </skos:scopeNote>
  <nt2:status>Approved</nt2:status>
  <nt2:type>Descriptor</nt2:type>
  <nt2:inputdate>2005-12-07</nt2:inputdate>
  <dcterms:dateAccepted>2005-12-07</dcterms:dateAccepted>
  <dcterms:modified>2006-12-18</dcterms:modified>
  <nt2:code>1102</nt2:code>
 </skos:Concept>
 <skos:Concept rdf:about='urn:comp:109'>
  <skos:prefLabel>Advanced Experimentation and Testing Technologies</skos:prefLabel>
  <skos:altLabel>AETT</skos:altLabel>
  <skos:broader rdf:resource='urn:comp:1363'/>
  <skos:changeNote>???
  </skos:changeNote>
  <skos:scopeNote>Knowledge of advanced experimentation and testing
    philosophies and approaches that provide results to inform
    research activities in specialized areas such as
    structures, materials, airborne Systems, aerodynamics, and
    propulsion. Ability to develop and use specialized
    facilities and equipment such as wind tunnels, arc-jets,
    and laboratories. Includes knowledge of how to plan,
    conduct and interpret experimental test results to
    understand the interaction of test elements on the design
    of current and future aerospace vehicles. Also involves
    ability to develop, manage and enhance test processes to
    optimize productivity, cycle time, data quality, cost and
    customer satisfaction.
  </skos:scopeNote>
  <nt2:status>Approved</nt2:status>
  <nt2:type>Descriptor</nt2:type>
  <nt2:inputdate>2006-12-13</nt2:inputdate>
  <dcterms:dateAccepted>2005-12-07</dcterms:dateAccepted>
  <dcterms:modified>2006-12-18</dcterms:modified>
  <nt2:code>109</nt2:code>
 </skos:Concept>
 <skos:Concept rdf:about='urn:comp:1031'>
  <skos:prefLabel>Test Fixtures and GSE Design and Development Engineering</skos:prefLabel>
  <skos:altLabel>DDETEST</skos:altLabel>
  <skos:broader rdf:resource='urn:comp:8'/>
  <skos:scopeNote>Knowledge of all aspects of the technical design and
    development process as applied to ground support equipment
    and special test fixtures relating to systems or subsystems
    including structural, electrical and propulsion components
    and technologies. Includes the definition or assessment of
    concepts and designs to assure adequate functional
    performance is achieved and system requirements are met and
    an assessment of the fabrication process and techniques,
    production assessment, and process verification of the
    hardware design. Includes knowledge and capability to
    create and evaluate subscale or full-scale models, test
    articles, or prototypes to assess the system or subsystem
    design, development, and integration meets the intended
    objectives.
  </skos:scopeNote>
  <nt2:status>Approved</nt2:status>
  <nt2:type>Descriptor</nt2:type>
  <nt2:inputdate>2006-12-13</nt2:inputdate>
  <dcterms:modified>2006-12-13</dcterms:modified>
  <nt2:code>1031</nt2:code>
 </skos:Concept>
 <skos:Concept rdf:about='urn:comp:66'>
  <skos:prefLabel>Materials Science and Engineering</skos:prefLabel>
  <skos:altLabel>MATSCIENG</skos:altLabel>
  <skos:broader rdf:resource='urn:comp:1347'/>
  <skos:narrower rdf:resource='urn:comp:1063'/>
  <skos:narrower rdf:resource='urn:comp:1062'/>
  <skos:narrower rdf:resource='urn:comp:1060'/>
  <skos:narrower rdf:resource='urn:comp:1061'/>
  <skos:scopeNote>Knowledge capability and practices associated with research
    into the characteristics and performance of materials and
    the design, development and testing of those materials
    within aerospace structures such as flight systems, ground
    support and facility systems. Includes the development of
    math models for assessment of material durability and
    response to environmental conditions and contaminants.
    Includes broad knowledge of materials disciplines,
    including material types such as ceramics, metallics, and
    polymers as well as tribology or surface science.
  </skos:scopeNote>
  <nt2:status>Approved</nt2:status>
  <nt2:type>Descriptor</nt2:type>
  <nt2:inputdate>2006-12-13</nt2:inputdate>
  <dcterms:modified>2006-12-13</dcterms:modified>
  <nt2:code>66</nt2:code>
 </skos:Concept>
 <skos:Concept rdf:about='urn:comp:1103'>
  <skos:prefLabel>Professional Administrative Student Trainee</skos:prefLabel>
  <skos:altLabel>STUPROFADM</skos:altLabel>
  <skos:broader rdf:resource='urn:comp:174'/>
  <skos:scopeNote>This is a training and development competency for employees
    who are classified as Professional Administrative
    Student Trainees.
  </skos:scopeNote>
  <nt2:status>Approved</nt2:status>
  <nt2:type>Descriptor</nt2:type>
  <nt2:inputdate>2005-12-07</nt2:inputdate>
  <dcterms:dateAccepted>2005-12-07</dcterms:dateAccepted>
  <dcterms:modified>2006-12-18</dcterms:modified>
  <nt2:code>1103</nt2:code>
 </skos:Concept>
 <skos:Concept rdf:about='urn:comp:1020'>
  <skos:prefLabel>Ergonomics Engineering, Technology, and Standards</skos:prefLabel>
  <skos:altLabel>HFEERGO</skos:altLabel>
  <skos:broader rdf:resource='urn:comp:41'/>
  <skos:scopeNote>TBD (including lighting, noise, vibration, physical
    ergonomics of hand tools, manual materials handling, etc.)
  </skos:scopeNote>
  <nt2:status>Approved</nt2:status>
  <nt2:type>Descriptor</nt2:type>
  <nt2:inputdate>2006-12-13</nt2:inputdate>
  <dcterms:modified>2006-12-13</dcterms:modified>
  <nt2:code>1020</nt2:code>
 </skos:Concept>
 <skos:Concept rdf:about='urn:comp:1082'>
  <skos:prefLabel>Paralegal</skos:prefLabel>
  <skos:broader rdf:resource='urn:comp:176'/>
  <skos:changeNote>Created ??
    Modified by ???
  </skos:changeNote>
  <skos:scopeNote>Knowledge of legal research and writing, litigation case
    management, and providing professional administrative and
    technical legal support. Possesses paralegal certificate or
    equivalent
  </skos:scopeNote>
  <nt2:status>Approved</nt2:status>
  <nt2:type>Descriptor</nt2:type>
  <nt2:inputdate>2006-12-13</nt2:inputdate>
  <dcterms:dateAccepted>2006-04-05</dcterms:dateAccepted>
  <dcterms:modified>2006-12-18</dcterms:modified>
  <nt2:code>1082</nt2:code>
 </skos:Concept>
 <skos:Concept rdf:about='urn:comp:1055'>
  <skos:prefLabel>Valves, Lines &amp; Ducts</skos:prefLabel>
  <skos:altLabel>RPVALVES</skos:altLabel>
  <skos:broader rdf:resource='urn:comp:73'/>
  <skos:scopeNote>Knowledge, capabilities, and practices associated with
    propulsion system valves, valve actuators, lines, ducts,
    miscellaneous fluid components, and fluid systems,
    including functional design, detailed design, testing and
    evaluation, anomaly resolution, manufacturing techniques,
    assembly, inspection, insight and oversight. Knowledge
    pertaining to integration of valves, valve actuators,
    lines, ducts, and miscellaneous fluid components into
    flight systems, developmental systems, and ground test
    systems.
  </skos:scopeNote>
  <nt2:status>Approved</nt2:status>
  <nt2:type>Descriptor</nt2:type>
  <nt2:inputdate>2006-12-13</nt2:inputdate>
  <dcterms:modified>2006-12-13</dcterms:modified>
  <nt2:code>1055</nt2:code>
 </skos:Concept>
 <skos:Concept rdf:about='urn:comp:1080'>
  <skos:prefLabel>Database Management Systems</skos:prefLabel>
  <skos:altLabel>DATDBMMT</skos:altLabel>
  <skos:broader rdf:resource='urn:comp:161'/>
  <skos:scopeNote>Knowledge of the uses of database management systems and
    software to control the organization, storage, retrieval,
    security, and integrity of data. This could include the
    knowledge of the principles, methods, and tools for
    automating, developing, implementing, or administering
    database systems.
  </skos:scopeNote>
  <nt2:status>Approved</nt2:status>
  <nt2:type>Descriptor</nt2:type>
  <nt2:inputdate>2006-12-13</nt2:inputdate>
  <dcterms:modified>2006-12-13</dcterms:modified>
  <nt2:code>1080</nt2:code>
 </skos:Concept>
 <skos:Concept rdf:about='urn:comp:1024'>
  <skos:prefLabel>Cognitive Technologies</skos:prefLabel>
  <skos:altLabel>HFECOG</skos:altLabel>
  <skos:broader rdf:resource='urn:comp:41'/>
  <skos:scopeNote>TBD (includes augmented cognition devices, decision support
    technologies, intelligent assistant systems)
  </skos:scopeNote>
  <nt2:status>Approved</nt2:status>
  <nt2:type>Descriptor</nt2:type>
  <nt2:inputdate>2006-12-13</nt2:inputdate>
  <dcterms:modified>2006-12-13</dcterms:modified>
  <nt2:code>1024</nt2:code>
 </skos:Concept>
 <skos:Concept rdf:about='urn:comp:1001'>
  <skos:prefLabel>Employee &amp; Team Leadership</skos:prefLabel>
  <skos:altLabel>LEADTEAM</skos:altLabel>
  <skos:broader rdf:resource='urn:comp:140'/>
  <skos:scopeNote>Knowledge, capabilities and practices associated with
    communicating business direction, goals and performance,
    developing and maintaining relationships and alliances, and
    conducting problem solving for effective decision making.
    Includes understanding of effective interpersonal and group
    communication principles and techniques to gather,
    comprehend and express ideas in an effective manner, and
    inform and influence others. Includes knowledge of
    techniques and approaches to resolve conflict and negotiate
    effective outcomes. Demonstrates ability to balance
    short-term needs with long-term priorities and consider
    complex cross-functional, cross-center, division, business
    and geographic implications when approaching problems or
    issues. Knows how to apply appropriate techniques,
    procedures and policies in the management of workforce to
    achieve work objectives and maintain effective and positive
    operational environments.
  </skos:scopeNote>
  <nt2:status>Approved</nt2:status>
  <nt2:type>Descriptor</nt2:type>
  <nt2:inputdate>2006-12-13</nt2:inputdate>
  <dcterms:modified>2006-12-13</dcterms:modified>
  <nt2:code>1001</nt2:code>
 </skos:Concept>
 <skos:Concept rdf:about='urn:comp:1013'>
  <skos:prefLabel>Organizational Science Fundamental Research</skos:prefLabel>
  <skos:altLabel>HFRORG</skos:altLabel>
  <skos:broader rdf:resource='urn:comp:40'/>
  <skos:scopeNote>TBD
  </skos:scopeNote>
  <nt2:status>Approved</nt2:status>
  <nt2:type>Descriptor</nt2:type>
  <nt2:inputdate>2006-12-13</nt2:inputdate>
  <dcterms:modified>2006-12-13</dcterms:modified>
  <nt2:code>1013</nt2:code>
 </skos:Concept>
 <skos:Concept rdf:about='urn:comp:1079'>
  <skos:prefLabel>IT Architecture</skos:prefLabel>
  <skos:altLabel>BITARCH</skos:altLabel>
  <skos:broader rdf:resource='urn:comp:131'/>
  <skos:scopeNote>Knowledge of architectural methodologies used in the design
    and development of information systems, including physical
    structure of a system's internal operations and
    interactions with other systems.This may also include the
    knowledge of enterprise achitecure principles, methods, and
    tools utilized to simplify processes and unify work across
    agencies and within the lines-of-business of the Federal
    Government. This could also includet heknowledge of the
    princilpes, tools, and technquies used to design, develop,
    and/or implement Knolwedge Management practices at a local
    or enterprise level.
  </skos:scopeNote>
  <nt2:status>Approved</nt2:status>
  <nt2:type>Descriptor</nt2:type>
  <nt2:inputdate>2006-12-13</nt2:inputdate>
  <dcterms:modified>2006-12-13</dcterms:modified>
  <nt2:code>1079</nt2:code>
 </skos:Concept>
 <skos:Concept rdf:about='urn:comp:28'>
  <skos:prefLabel>Reliability &amp; Maintainability Engineering &amp; Assurance</skos:prefLabel>
  <skos:altLabel>RMEA</skos:altLabel>
  <skos:broader rdf:resource='urn:comp:1381'/>
  <skos:scopeNote>Knowledge, capabilities and practices used to design
    flight, ground support, and facility systems, equipment and
    instruments for performing their intended function for a
    specified interval under stated conditions (reliability)
    and/or have a defined capability to be restored to
    operational status following a failure (maintainability).
    Capabilities include the capacity to: define mission
    success criteria; define and evaluate compliance with
    systems/equipment reliability/maintainability requirements,
    including redundancy requirements; model systems/equipment
    from a reliability/maintainability perspective, including
    allocations and predictions; perform and evaluate
    quantitative and qualitative analyses and assessments,
    including failure modes and effects analyses/critical items
    list, probabilistic risk assessments, limited life items,
    quantitative computations; perform and evaluate statistical
    analysis, trending, and trade-offs; perform and evaluate
    maintenance analyses, such as reliability centered
    maintenance techniques; plan, perform and evaluate
    laboratory testing and engineering analyses; evaluate
    system/equipment failures to determine root cause and
    develop corrective actions to prevent similar failures in
    the future; integrate reliability/maintainability
    requirements, activities and results with other related
    disciplines (competencies) such as Safety Engineering and
    Assurance, Risk Management, Quality Engineering and
    Assurance, Human Factors, Software Assurance, Acquisition
    and Contract Management, and Logistics. Also includes
    availability which can combine the elements of reliability
    and maintainability in a single parameter."
  </skos:scopeNote>
  <nt2:status>Approved</nt2:status>
  <nt2:type>Descriptor</nt2:type>
  <nt2:inputdate>2006-12-13</nt2:inputdate>
  <dcterms:modified>2006-12-13</dcterms:modified>
  <nt2:code>28</nt2:code>
 </skos:Concept>
 <skos:Concept rdf:about='urn:comp:134'>
  <skos:prefLabel>Institutional Logistics, Supply and Transportation</skos:prefLabel>
  <skos:altLabel>LOGSUPTRAN</skos:altLabel>
  <skos:broader rdf:resource='urn:comp:1159'/>
  <skos:scopeNote>Knowledge of principles, practices, equipment and tools in
    the areas of Logistics, Supply and Transportation.
    Understanding of how to manage and optimize equipment,
    supplies and transportation systems to provide an
    infrastructure that enables the agency to operate
    effectively. Includes management of specifications,
    acquisition, certification, storage, delivery, lifecycle
    support, distribution, and disposal of supplies, hardware,
    materials, equipment, and property (except real estate) and
    the operation and maintenance of transportation and other
    equipment used to move materials or passengers. Also
    includes management of inventories, including government
    property, equipment and materials provided to employees and
    contractors, so that the property is accurately accounted
    for, reported against and disposed of at the end of its
    useful life. Requires understanding of government
    regulations regarding property management and disposal, and
    related contracting terminology and requirements.
  </skos:scopeNote>
  <nt2:status>Approved</nt2:status>
  <nt2:type>Descriptor</nt2:type>
  <nt2:inputdate>2006-12-13</nt2:inputdate>
  <dcterms:modified>2006-12-13</dcterms:modified>
  <nt2:code>134</nt2:code>
 </skos:Concept>
 <skos:Concept rdf:about='urn:comp:1119'>
  <skos:prefLabel>Employee Relations</skos:prefLabel>
  <skos:altLabel>HCMEMPREL</skos:altLabel>
  <skos:broader rdf:resource='urn:comp:128'/>
  <skos:scopeNote>Knowledge of laws, rules, regulations, case law,
    principles, and practices related to employee conduct,
    performance, and dispute resolution.
  </skos:scopeNote>
  <nt2:status>Approved</nt2:status>
  <nt2:type>Descriptor</nt2:type>
  <nt2:inputdate>2006-04-05</nt2:inputdate>
  <dcterms:dateAccepted>2006-04-05</dcterms:dateAccepted>
  <dcterms:modified>2006-12-18</dcterms:modified>
  <nt2:code>1119</nt2:code>
 </skos:Concept>
 <skos:Concept rdf:about='urn:comp:1019'>
  <skos:prefLabel>Biomechanical Engineering, Technology, Standards</skos:prefLabel>
  <skos:altLabel>HFEBIOMECH</skos:altLabel>
  <skos:broader rdf:resource='urn:comp:41'/>
  <skos:scopeNote>TBD
  </skos:scopeNote>
  <nt2:status>Approved</nt2:status>
  <nt2:type>Descriptor</nt2:type>
  <nt2:inputdate>2006-12-13</nt2:inputdate>
  <dcterms:modified>2006-12-13</dcterms:modified>
  <nt2:code>1019</nt2:code>
 </skos:Concept>
 <skos:Concept rdf:about='urn:comp:39'>
  <skos:prefLabel>Environmental Factors</skos:prefLabel>
  <skos:altLabel>ENVFACT</skos:altLabel>
  <skos:broader rdf:resource='urn:comp:1244'/>
  <skos:changeNote>Name changed from "Habitability and Environmenal Factors".
    Scope note modified to remove mentions of "habitability".
  </skos:changeNote>
  <skos:scopeNote>Knowledge of practices associated with research of and
    applying research to spacecraft and space-based
    environments and the environmental effects on humans and
    other organisms with specific emphasis on barophysiology,
    microbiology and toxicology and radiation. Knowledge of
    physical and chemical sciences, including heat and mass
    transfer, acoustics, radiation, thermodynamics, fluid
    mechanics, and chemical, biological, and metabolic
    processes. Ability to integrate and apply this
    understanding to develop systems and technology to enable
    humans to live and work safely and effectively in space.
  </skos:scopeNote>
  <nt2:status>Approved</nt2:status>
  <nt2:type>Descriptor</nt2:type>
  <nt2:inputdate>2006-12-13</nt2:inputdate>
  <dcterms:dateAccepted>2006-04-05</dcterms:dateAccepted>
  <dcterms:modified>2006-12-18</dcterms:modified>
  <nt2:code>39</nt2:code>
 </skos:Concept>
 <skos:Concept rdf:about='urn:comp:73'>
  <skos:prefLabel>Rocket Propulsion</skos:prefLabel>
  <skos:altLabel>ROCKETPRO</skos:altLabel>
  <skos:broader rdf:resource='urn:comp:1314'/>
  <skos:narrower rdf:resource='urn:comp:1058'/>
  <skos:narrower rdf:resource='urn:comp:1054'/>
  <skos:narrower rdf:resource='urn:comp:1059'/>
  <skos:narrower rdf:resource='urn:comp:1109'/>
  <skos:narrower rdf:resource='urn:comp:1056'/>
  <skos:narrower rdf:resource='urn:comp:1108'/>
  <skos:narrower rdf:resource='urn:comp:WQQ-542'/>
  <skos:narrower rdf:resource='urn:comp:WQQ-543'/>
  <skos:narrower rdf:resource='urn:comp:1053'/>
  <skos:narrower rdf:resource='urn:comp:1055'/>
  <skos:scopeNote>Knowledge of research and testing activities associated
    with liquid and solid rocket propulsion. Includes knowledge
    of combustion devices, cryogenic tanks, propellant
    feedlines, tank pressurization systems, engine systems, and
    propulsion system subcomponents such as gas generators,
    thrust chambers, turbopump assemblies, valves, propellant
    ducts, and auxiliary propulsion systems, as well as
    application of combined cycle systems to advanced
    propulsion techniques.
  </skos:scopeNote>
  <nt2:status>Approved</nt2:status>
  <nt2:type>Descriptor</nt2:type>
  <nt2:inputdate>2006-12-13</nt2:inputdate>
  <dcterms:modified>2006-12-13</dcterms:modified>
  <nt2:code>73</nt2:code>
 </skos:Concept>
 <skos:Concept rdf:about='urn:comp:1065'>
  <skos:prefLabel>Research Subject Protection Regulation</skos:prefLabel>
  <skos:altLabel>RSPR</skos:altLabel>
  <skos:broader rdf:resource='urn:comp:156'/>
  <skos:scopeNote>Knowledge and a thorough understanding of the Federal and
    Agency regulatory framework, which governs the use of human
    and animal subjects in research. Knowledge of the
    implementation of all regulatory requirements and all
    applicable laws governing research subject protection.
    Detailed understanding of the procedural requirements for
    the conduct of human subjects Institutional Review Boards
    and Institutional Animal Care and Use Committees, and
    knowledge of the implementation of such Agency Boards and
    Committees.
  </skos:scopeNote>
  <nt2:status>Approved</nt2:status>
  <nt2:type>Descriptor</nt2:type>
  <nt2:inputdate>2006-12-13</nt2:inputdate>
  <dcterms:modified>2006-12-13</dcterms:modified>
  <nt2:code>1065</nt2:code>
 </skos:Concept>
 <skos:Concept rdf:about='urn:comp:49'>
  <skos:prefLabel>Earth Science Applications Research</skos:prefLabel>
  <skos:altLabel>EARSCIRES</skos:altLabel>
  <skos:broader rdf:resource='urn:comp:1415'/>
  <skos:scopeNote>Use knowledge of Earth systems and measurement technologies
    for designing research into Earth Science disciplines that
    have the objective of improving the quality of life on
    Earth and the longevity of the planet. Apply research to
    such subjects as resource and disaster management,
    environmental assessment, human health and safety, food and
    fiber, infrastructure planning, and environmental quality.
  </skos:scopeNote>
  <nt2:status>Approved</nt2:status>
  <nt2:type>Descriptor</nt2:type>
  <nt2:inputdate>2006-12-13</nt2:inputdate>
  <dcterms:modified>2006-12-13</dcterms:modified>
  <nt2:code>49</nt2:code>
 </skos:Concept>
 <skos:Concept rdf:about='urn:comp:117'>
  <skos:prefLabel>Commercial Technology</skos:prefLabel>
  <skos:altLabel>COMTEC</skos:altLabel>
  <skos:broader rdf:resource='urn:comp:1125'/>
  <skos:scopeNote>Knowledge and abilities associated with transferring
    current and future Agency technology to external entities
    in order to meet broad Agency vision and missions, and
    extend the lifecycle and broaden the usefulness of Agency
    technologies. Involves expertise in business practices
    pertaining to intellectual property, patents, licenses and
    partnerships as well as general business knowledge for
    assessing potential partners. Includes broad understanding
    of Agency technologies and programs, as well as familiarity
    with external entities and markets.
  </skos:scopeNote>
  <nt2:status>Approved</nt2:status>
  <nt2:type>Descriptor</nt2:type>
  <nt2:inputdate>2006-12-13</nt2:inputdate>
  <dcterms:modified>2006-12-13</dcterms:modified>
  <nt2:code>117</nt2:code>
 </skos:Concept>
 <skos:Concept rdf:about='urn:comp:1006'>
  <skos:prefLabel>Habitability and Environmental Psychology Fundamental Research</skos:prefLabel>
  <skos:altLabel>HFRHABIT</skos:altLabel>
  <skos:broader rdf:resource='urn:comp:40'/>
  <skos:scopeNote>TBD
  </skos:scopeNote>
  <nt2:status>Approved</nt2:status>
  <nt2:type>Descriptor</nt2:type>
  <nt2:inputdate>2006-12-13</nt2:inputdate>
  <dcterms:modified>2006-12-13</dcterms:modified>
  <nt2:code>1006</nt2:code>
 </skos:Concept>
 <skos:Concept rdf:about='urn:comp:1339'>
  <skos:prefLabel>Sensor Systems Competency Suite</skos:prefLabel>
  <skos:broader rdf:resource='urn:comp:1208'/>
  <skos:narrower rdf:resource='urn:comp:96'/>
  <skos:narrower rdf:resource='urn:comp:14'/>
  <skos:narrower rdf:resource='urn:comp:92'/>
  <skos:narrower rdf:resource='urn:comp:94'/>
  <skos:narrower rdf:resource='urn:comp:93'/>
  <skos:narrower rdf:resource='urn:comp:95'/>
  <skos:narrower rdf:resource='urn:comp:20'/>
  <nt2:status>Approved</nt2:status>
  <nt2:type>Descriptor</nt2:type>
  <nt2:inputdate>2006-12-13</nt2:inputdate>
  <dcterms:modified>2006-12-13</dcterms:modified>
  <nt2:code>1339</nt2:code>
 </skos:Concept>
 <skos:Concept rdf:about='urn:comp:1087'>
  <skos:prefLabel>Environmental/Real Property Law</skos:prefLabel>
  <skos:altLabel>ENVLAW</skos:altLabel>
  <skos:broader rdf:resource='urn:comp:125'/>
  <skos:changeNote>???
  </skos:changeNote>
  <skos:scopeNote>Speciaized knowledge of matters related to environmental
    matters, inclucing but not limited to of local, state and
    Federal environmental laws, regulations, Executive Orders,
    and administrative procedures, NEPA, permits, response or
    corrective actions, pollution prevention, and litigation
    and appeals related to environmental matters.
  </skos:scopeNote>
  <nt2:status>Approved</nt2:status>
  <nt2:type>Descriptor</nt2:type>
  <nt2:inputdate>2006-12-13</nt2:inputdate>
  <dcterms:dateAccepted>2006-04-05</dcterms:dateAccepted>
  <dcterms:modified>2006-12-18</dcterms:modified>
  <nt2:code>1087</nt2:code>
 </skos:Concept>
 <skos:Concept rdf:about='urn:comp:31'>
  <skos:prefLabel>Cell &amp; Molecular Biology</skos:prefLabel>
  <skos:altLabel>CELLBIO</skos:altLabel>
  <skos:broader rdf:resource='urn:comp:1430'/>
  <skos:changeNote>Changed "and" in term label to "&amp;". Added "and development
    of biosentinals" to end of scope note.
  </skos:changeNote>
  <skos:scopeNote>Knowledge of and ability to conduct research on basic
    cellular function and properties such as gene regulation
    and expression or mechanoreception, that may be directly or
    indirectly impacted by altered gravitational force and
    other space-related effects. Includes biotechnology, tissue
    engineering, study of the dynamics of cell behavior and
    interactions and differentiation in cellular systems within
    and across organisms under a variety of environmental
    conditions, such as the physiological changes seen in whole
    animals in response to the space environment, and
    development of biosentinels.
  </skos:scopeNote>
  <nt2:status>Approved</nt2:status>
  <nt2:type>Descriptor</nt2:type>
  <nt2:inputdate>2006-12-13</nt2:inputdate>
  <dcterms:dateAccepted>2006-04-05</dcterms:dateAccepted>
  <dcterms:modified>2006-12-18</dcterms:modified>
  <nt2:code>31</nt2:code>
 </skos:Concept>
 <skos:Concept rdf:about='urn:comp:79'>
  <skos:prefLabel>Robotics</skos:prefLabel>
  <skos:broader rdf:resource='urn:comp:1283'/>
  <skos:scopeNote>Knowledge of engineering, design, development, analysis and
    testing of robotic and robotic/human systems, including
    telerobotics. Includes knowledge of operational impacts and
    sustaining engineering on the system.
  </skos:scopeNote>
  <nt2:status>Approved</nt2:status>
  <nt2:type>Descriptor</nt2:type>
  <nt2:inputdate>2006-12-13</nt2:inputdate>
  <dcterms:modified>2006-12-13</dcterms:modified>
  <nt2:code>79</nt2:code>
 </skos:Concept>
 <skos:Concept rdf:about='urn:comp:110'>
  <skos:prefLabel>Simulation/Flight Research Systems</skos:prefLabel>
  <skos:altLabel>SIMFLTSYS</skos:altLabel>
  <skos:broader rdf:resource='urn:comp:1237'/>
  <skos:scopeNote>Knowledge capabilities and practices used to provide and
    integrate appropriate real-time hardware/software systems
    in support of piloted simulators and research aircraft that
    enable experiments in Flight Dynamics,
    Guidance/Navigation/Control, Crew Systems and Aviation
    Operations, Reliable Digital Systems and Electromagnetics.
  </skos:scopeNote>
  <nt2:status>Approved</nt2:status>
  <nt2:type>Descriptor</nt2:type>
  <nt2:inputdate>2006-12-13</nt2:inputdate>
  <dcterms:modified>2006-12-13</dcterms:modified>
  <nt2:code>110</nt2:code>
 </skos:Concept>
 <skos:Concept rdf:about='urn:comp:21'>
  <skos:prefLabel>Avionics</skos:prefLabel>
  <skos:broader rdf:resource='urn:comp:1294'/>
  <skos:scopeNote>Knowledge of research and engineering of real-time analog
    and/or digital electronic avionics systems that use data
    acquired from sensors and instruments and processes it to
    determine status of systems for aircraft and spacecraft for
    such purposes as flight control, flight path management and
    vehicle health monitoring. Includes knowledge of design and
    development of computational hardware and software networks
    and interfaces, electrical integration, power distribution
    and electrical systems engineering.
  </skos:scopeNote>
  <nt2:status>Approved</nt2:status>
  <nt2:type>Descriptor</nt2:type>
  <nt2:inputdate>2006-12-13</nt2:inputdate>
  <dcterms:modified>2006-12-13</dcterms:modified>
  <nt2:code>21</nt2:code>
 </skos:Concept>
 <skos:Concept rdf:about='urn:comp:1022'>
  <skos:prefLabel>Habitability Engineering, Technology, and Standards</skos:prefLabel>
  <skos:altLabel>HFEHABIT</skos:altLabel>
  <skos:broader rdf:resource='urn:comp:41'/>
  <skos:scopeNote>TBD
  </skos:scopeNote>
  <nt2:status>Approved</nt2:status>
  <nt2:type>Descriptor</nt2:type>
  <nt2:inputdate>2006-12-13</nt2:inputdate>
  <dcterms:modified>2006-12-13</dcterms:modified>
  <nt2:code>1022</nt2:code>
 </skos:Concept>
 <skos:Concept rdf:about='urn:comp:1068'>
  <skos:prefLabel>Health Physics</skos:prefLabel>
  <skos:altLabel>OCCPHYSICS</skos:altLabel>
  <skos:broader rdf:resource='urn:comp:130'/>
  <skos:scopeNote>Knowledge of Federal and State Health Physics (ionizing and
    non-ionizing radiation) regulations, policies, and
    procedures, to develop and implement preventive measures
    regarding all work-related exposures, injuries and
    illnesses. Knowledge to develop, coordinate, implement,
    manage, and assess the effectiveness of related programs,
    practices and policies across the Agency, designed to
    protect the health of employees. Knowledge and skills to
    evaluate the application of new technologies to Agency
    related issues, and the impact of new laws and regulations
    and provides advice to Agency top management. Knowledge to
    provide professional symposia, workshops, and develop
    related training programs for Agency-wide application.
  </skos:scopeNote>
  <nt2:status>Approved</nt2:status>
  <nt2:type>Descriptor</nt2:type>
  <nt2:inputdate>2006-12-13</nt2:inputdate>
  <dcterms:modified>2006-12-13</dcterms:modified>
  <nt2:code>1068</nt2:code>
 </skos:Concept>
 <skos:Concept rdf:about='urn:comp:1018'>
  <skos:prefLabel>Human Performance Fundamental Research</skos:prefLabel>
  <skos:altLabel>HFRHUMPERF</skos:altLabel>
  <skos:broader rdf:resource='urn:comp:40'/>
  <skos:scopeNote>TBD (includes basic research on human error and error
    countermeasures)
    NASA Competency Management SystemPage 36
  </skos:scopeNote>
  <nt2:status>Approved</nt2:status>
  <nt2:type>Descriptor</nt2:type>
  <nt2:inputdate>2006-12-13</nt2:inputdate>
  <dcterms:modified>2006-12-13</dcterms:modified>
  <nt2:code>1018</nt2:code>
 </skos:Concept>
 <skos:Concept rdf:about='urn:comp:48'>
  <skos:prefLabel>Oceanographic Science</skos:prefLabel>
  <skos:altLabel>OCEANSCI</skos:altLabel>
  <skos:broader rdf:resource='urn:comp:1415'/>
  <skos:scopeNote>Research into the composition, activities, processes and
    patterns in the oceans and ocean ice to increase
    understanding of how the marine environment interacts with
    the rest of the planet. Includes research on glaciers and
    ice sheets. Use a variety of data collection methods to
    collect information about the ocean and mathematically
    describe and predict ocean processes. Includes ability to
    translate data into information useful in the understanding
    and interpretation of the oceans themselves and their
    connection to other earth systems.
  </skos:scopeNote>
  <nt2:status>Approved</nt2:status>
  <nt2:type>Descriptor</nt2:type>
  <nt2:inputdate>2006-12-13</nt2:inputdate>
  <dcterms:modified>2006-12-13</dcterms:modified>
  <nt2:code>48</nt2:code>
 </skos:Concept>
 <skos:Concept rdf:about='urn:comp:1114'>
  <skos:prefLabel>Patent Agent</skos:prefLabel>
  <skos:altLabel>PATENTAGT</skos:altLabel>
  <skos:broader rdf:resource='urn:comp:176'/>
  <skos:scopeNote>Knowledge of intellectual property matters, patents,
    copyrights, data rights, trademarks, and commercilization
    of technology. Must be admitted to the practice before U.S.
    Patent Office, but not necessarily liscensed to practice
    law.
  </skos:scopeNote>
  <nt2:status>Approved</nt2:status>
  <nt2:type>Descriptor</nt2:type>
  <nt2:inputdate>2006-04-05</nt2:inputdate>
  <dcterms:dateAccepted>2006-04-05</dcterms:dateAccepted>
  <dcterms:modified>2006-12-18</dcterms:modified>
  <nt2:code>1114</nt2:code>
 </skos:Concept>
 <skos:Concept rdf:about='urn:comp:1115'>
  <skos:prefLabel>Classification</skos:prefLabel>
  <skos:altLabel>HCMCLASS</skos:altLabel>
  <skos:broader rdf:resource='urn:comp:128'/>
  <skos:scopeNote>Knowledge of classification concepts, principles, and
    practices related to structuring organizations and
    positions and determining the appropriate pay system,
    occupational grouping, title, and pay level of positions..
  </skos:scopeNote>
  <nt2:status>Approved</nt2:status>
  <nt2:type>Descriptor</nt2:type>
  <nt2:inputdate>2006-04-05</nt2:inputdate>
  <dcterms:dateAccepted>2006-04-05</dcterms:dateAccepted>
  <dcterms:modified>2006-12-18</dcterms:modified>
  <nt2:code>1115</nt2:code>
 </skos:Concept>
 <skos:Concept rdf:about='urn:comp:133'>
  <skos:prefLabel>Institutional Environmental Engineering &amp; Management</skos:prefLabel>
  <skos:altLabel>ENVENGMMT</skos:altLabel>
  <skos:broader rdf:resource='urn:comp:1159'/>
  <skos:narrower rdf:resource='urn:comp:1088'/>
  <skos:narrower rdf:resource='urn:comp:1089'/>
  <skos:scopeNote>Uses knowledge of environmental engineering, environmental
    law, chemistry, biology, geology and hydrogeology to
    maintain a proactive stance regarding environmental
    stewardship, including protection and restoration of
    environmental resources such as ground water, surface
    water, soils, sediments, air, and natural, cultural and
    historic resources. Plans and assesses compliance with
    Federal, State, and local statutory and regulatory
    requirements, Executive Orders, and directives. Implements
    proactive programs such as recycling, pollution prevention,
    affirmative procurement and energy management, and
    remediation activities under RCRA and CERCLA requirements.
  </skos:scopeNote>
  <nt2:status>Approved</nt2:status>
  <nt2:type>Descriptor</nt2:type>
  <nt2:inputdate>2006-12-13</nt2:inputdate>
  <dcterms:modified>2006-12-13</dcterms:modified>
  <nt2:code>133</nt2:code>
 </skos:Concept>
 <skos:Concept rdf:about='urn:comp:1113'>
  <skos:prefLabel>Commercial Law</skos:prefLabel>
  <skos:altLabel>COMMLAW</skos:altLabel>
  <skos:broader rdf:resource='urn:comp:125'/>
  <skos:scopeNote>Knowledge of negotiating, drafting, and interpreting Space
    Act Agreements with domestic and foreign entities;
    compliance with export-import control regulations; and
    partnering arrangements with commercial organizations.
    Knowledge related to intellectural property law and
    commercialization of NASA activities, in addition to
    policy, legislative drafting, negotiating and drafting
    agreements, and providing legal advice and reviews.
  </skos:scopeNote>
  <nt2:status>Approved</nt2:status>
  <nt2:type>Descriptor</nt2:type>
  <nt2:inputdate>2006-04-05</nt2:inputdate>
  <dcterms:dateAccepted>2006-04-05</dcterms:dateAccepted>
  <dcterms:modified>2006-12-18</dcterms:modified>
  <nt2:code>1113</nt2:code>
 </skos:Concept>
 <skos:Concept rdf:about='urn:comp:1064'>
  <skos:prefLabel>Biomedical and Research Clinical Ethics</skos:prefLabel>
  <skos:altLabel>BRCE</skos:altLabel>
  <skos:broader rdf:resource='urn:comp:156'/>
  <skos:scopeNote>Professional skills and knowledge of bioethics applied to a
    range of bioethical issues surrounding biomedical research,
    particularly those associated with the use of human and
    animal subjects in research. Broad and detailed
    understanding and knowledge of the evolution and
    development of ethical thought related to biomedical
    research and medical practice, to guide the development of
    Agency policy, and provision of expert opinion on relevant
    ethical issues to inform Agency decision-making.
  </skos:scopeNote>
  <nt2:status>Approved</nt2:status>
  <nt2:type>Descriptor</nt2:type>
  <nt2:inputdate>2006-12-13</nt2:inputdate>
  <dcterms:modified>2006-12-13</dcterms:modified>
  <nt2:code>1064</nt2:code>
 </skos:Concept>
 <skos:Concept rdf:about='urn:comp:1025'>
  <skos:prefLabel>Human-Automation System Design</skos:prefLabel>
  <skos:altLabel>HFEHUMAUTO</skos:altLabel>
  <skos:broader rdf:resource='urn:comp:41'/>
  <skos:scopeNote>TBD (includes Distributed Supervisory Control Design;
    fFunction Allocation; Mixed-Initiative Decision Making,
    Planning and Operations; Distributed Human-Machine Systems)
  </skos:scopeNote>
  <nt2:status>Approved</nt2:status>
  <nt2:type>Descriptor</nt2:type>
  <nt2:inputdate>2006-12-13</nt2:inputdate>
  <dcterms:modified>2006-12-13</dcterms:modified>
  <nt2:code>1025</nt2:code>
 </skos:Concept>
 <skos:Concept rdf:about='urn:comp:1105'>
  <skos:prefLabel>Probabilistic Risk Assessment</skos:prefLabel>
  <skos:altLabel>PROBRISK</skos:altLabel>
  <skos:broader rdf:resource='urn:comp:27'/>
  <skos:scopeNote>Knowledge, capabilities and practices associated with the
    development and application of system risk models to
    support risk-informed decision making. This includes the
    assessment of mission success criteria, accident scenario
    development using logic techniques, phenomenological
    failure modeling, quantification of accident scenarios
    using probabilistic and statistical analysis techniques,
    consequence assessment (evaluation of the physical
    consequences of accident scenarios), uncertainty and
    risk-trade-off analysis, and risk communication.
  </skos:scopeNote>
  <nt2:status>Approved</nt2:status>
  <nt2:type>Descriptor</nt2:type>
  <nt2:inputdate>2005-12-07</nt2:inputdate>
  <dcterms:dateAccepted>2005-12-07</dcterms:dateAccepted>
  <dcterms:modified>2006-12-18</dcterms:modified>
  <nt2:code>1105</nt2:code>
 </skos:Concept>
 <skos:Concept rdf:about='urn:comp:1036'>
  <skos:prefLabel>Propulsion Integration Engineering</skos:prefLabel>
  <skos:altLabel>INTPROPEL</skos:altLabel>
  <skos:broader rdf:resource='urn:comp:9'/>
  <skos:scopeNote>Knowledge and capability to integrate propulsion elements
    into a functioning system or subsystem such as the
    integration of a propulsion system into a test stand,
    vehicle, or spacecraft or the integration of components
    (turbomachinery, main chambers, valves, etc.) into a
    propulsion system. Includes knowledge and capabilities
    required to understand the complex fluid and structural
    interactions of the various propulsion system or subsystem
    elements such as the interaction between the engine and
    main propulsion system or the interaction between a
    turbopump and an engine system. Inculdes the planning,
    design, development, and evaluation of the various
    components and subsystems that is necessary to insure
    proper function and compatibility within the propulsion
    systems.
  </skos:scopeNote>
  <nt2:status>Approved</nt2:status>
  <nt2:type>Descriptor</nt2:type>
  <nt2:inputdate>2006-12-13</nt2:inputdate>
  <dcterms:modified>2006-12-13</dcterms:modified>
  <nt2:code>1036</nt2:code>
 </skos:Concept>
 <skos:Concept rdf:about='urn:comp:29'>
  <skos:prefLabel>Quality Engineering &amp; Assurance</skos:prefLabel>
  <skos:altLabel>QEA</skos:altLabel>
  <skos:broader rdf:resource='urn:comp:1381'/>
  <skos:changeNote>???
  </skos:changeNote>
  <skos:scopeNote>Knowledge, capabilities, and practices associated with the
    assurance of quality (aeronautic and astronautic) for all
    phases of the mission life-cycle including design,
    manufacturing, assembly, testing and operations. Capability
    for planning, defining, documenting, and executing quality
    requirements for products, processes, and systems that are
    suitable to the activity, proportional to the risk, and
    consistent with established NASA guidance, practices, and
    standards including NASA workmanship standards, NASA parts
    standards, Federal Acquisition Requirements (FAR), and NASA
    recommended practices for contract quality and supplier
    assessment. Knowledge of destructive and non-destructive
    material testing and inspection techniques used to validate
    product compliance, including related contract data
    deliverable requirements. Knowledge of ISO 9000 and AS 9100
    series of quality standards, as well as the ability to
    apply these standards for complex or critical items.
    Ability to assess quality system compliance and
    effectiveness in accordance with requirements of ISO 9000
    and AS 9100 quality standards. Knowledge of inspection,
    auditing and surveillance methods which can range from a
    one-time test or inspection of a product, process, or
    service to periodic in process monitoring of contract
    performance. Ability to manage, and/or evaluate the results
    of quality functions (audits, surveys, reports, acceptance
    data package/test report, etc.) performed by NASA, NASA
    designated/delegated representatives, and/or third party
    certification bodies. Ability to continually improve
    quality through advocacy and dissemination of advanced
    quality tools, techniques, technology, practices, policy,
    procedures, and training. Ability to perform quality data
    analysis and trending, to determine deficiency root
    cause(s), and to implement effective preventive measures.
  </skos:scopeNote>
  <nt2:status>Approved</nt2:status>
  <nt2:type>Descriptor</nt2:type>
  <nt2:inputdate>2006-12-13</nt2:inputdate>
  <dcterms:dateAccepted>2005-12-07</dcterms:dateAccepted>
  <dcterms:modified>2006-12-18</dcterms:modified>
  <nt2:code>29</nt2:code>
 </skos:Concept>
 <skos:Concept rdf:about='urn:comp:143'>
  <skos:prefLabel>Fire Protection Engineering</skos:prefLabel>
  <skos:altLabel>FIREPROT</skos:altLabel>
  <skos:broader rdf:resource='urn:comp:1159'/>
  <skos:changeNote>???
  </skos:changeNote>
  <skos:scopeNote>Knowledge, capabilities and practices associated fire
    prevention-related tools and their application to systems
    for minimizing the occurrence or effects of fire. Maintains
    comprehensive knowledge of applicable NFPA, OSHA, NASA,
    aerospace and/or prevention industry trends, standards and
    develops policies for fire prevention. Demonstrates a
    comprehensive knowledge of and contributes to resources
    available in the fire prevention community including NASA,
    DOD, academia, and industry. Capability to review and
    assess complex technical documents for their impact on fire
    prevention work. Maintain a comprehensive knowledge of Life
    Safety Systems. Capability to provide mitigation strategies
    for fire protection when requirements cannot be met..
  </skos:scopeNote>
  <nt2:status>Approved</nt2:status>
  <nt2:type>Descriptor</nt2:type>
  <nt2:inputdate>2006-12-13</nt2:inputdate>
  <dcterms:dateAccepted>2005-12-07</dcterms:dateAccepted>
  <dcterms:modified>2006-12-18</dcterms:modified>
  <nt2:code>143</nt2:code>
 </skos:Concept>
 <skos:Concept rdf:about='urn:comp:1043'>
  <skos:prefLabel>EEE Parts</skos:prefLabel>
  <skos:altLabel>ELEEEPART</skos:altLabel>
  <skos:broader rdf:resource='urn:comp:13'/>
  <skos:scopeNote>Knowledge, capabilities, and practices associated with EEE
    Parts requirements, selection, analysis, and verification
    for space flight and ground support hardware.
  </skos:scopeNote>
  <nt2:status>Approved</nt2:status>
  <nt2:type>Descriptor</nt2:type>
  <nt2:inputdate>2006-12-13</nt2:inputdate>
  <dcterms:modified>2006-12-13</dcterms:modified>
  <nt2:code>1043</nt2:code>
 </skos:Concept>
 <skos:Concept rdf:about='urn:comp:1407'>
  <skos:prefLabel>Space Sciences Competency Suite</skos:prefLabel>
  <skos:broader rdf:resource='urn:comp:1406'/>
  <skos:narrower rdf:resource='urn:comp:54'/>
  <skos:narrower rdf:resource='urn:comp:55'/>
  <skos:narrower rdf:resource='urn:comp:52'/>
  <skos:narrower rdf:resource='urn:comp:44'/>
  <skos:narrower rdf:resource='urn:comp:163'/>
  <skos:narrower rdf:resource='urn:comp:53'/>
  <skos:narrower rdf:resource='urn:comp:51'/>
  <nt2:status>Approved</nt2:status>
  <nt2:type>Descriptor</nt2:type>
  <nt2:inputdate>2006-12-13</nt2:inputdate>
  <dcterms:modified>2006-12-13</dcterms:modified>
  <nt2:code>1407</nt2:code>
 </skos:Concept>
 <skos:Concept rdf:about='urn:comp:80'>
  <skos:prefLabel>Computer Systems and Engineering</skos:prefLabel>
  <skos:altLabel>COMPSYSENG</skos:altLabel>
  <skos:broader rdf:resource='urn:comp:1283'/>
  <skos:changeNote>???
  </skos:changeNote>
  <skos:scopeNote>Knowledge of the design and development of computers and/or
    robots. Involves design of hardware, software, networks and
    processes to solve technical problems such as analyzing
    flight systems and aerospace data. Utilizes advanced
    technologies such as virtual reality, artificial
    intelligence, and automation. Includes knowledge of
    computer programming, electronics, mathematical models, and
    neural and/or other networking systems.
  </skos:scopeNote>
  <nt2:status>Approved</nt2:status>
  <nt2:type>Descriptor</nt2:type>
  <nt2:inputdate>2006-12-13</nt2:inputdate>
  <dcterms:dateAccepted>2005-12-07</dcterms:dateAccepted>
  <dcterms:modified>2006-12-18</dcterms:modified>
  <nt2:code>80</nt2:code>
 </skos:Concept>
 <skos:Concept rdf:about='urn:comp:158'>
  <skos:prefLabel>Diversity Management</skos:prefLabel>
  <skos:altLabel>DIVERSEMMT</skos:altLabel>
  <skos:broader rdf:resource='urn:comp:1189'/>
  <skos:scopeNote>Knowledge, capabilities and practices associated with the
    application of diversity management including developing,
    implementing, evaluating, and monitoring the Agency’s
    Diversity Strategic Implementation Plan and related
    programs as well as internal diversity communications and
    external diversity relations, diverse employee network
    groups, diversity training initiatives, diversity councils,
    and mentoring initiatives. Works in partnership with the
    Center(s) leadership and Diversity Council(s) to optimize
    and support efforts to acquire and sustain a vital
    effective workforce, to capitalize on the strengths of a
    diverse workforce to better perform the Center’s mission
    through teamwork and innovation, and to build an
    organizational climate in which employees respect,
    appreciate, and value individual differences as catalysts
    for creativity and productivity..
  </skos:scopeNote>
  <nt2:status>Approved</nt2:status>
  <nt2:type>Descriptor</nt2:type>
  <nt2:inputdate>2006-12-13</nt2:inputdate>
  <dcterms:modified>2006-12-13</dcterms:modified>
  <nt2:code>158</nt2:code>
 </skos:Concept>
 <skos:Concept rdf:about='urn:comp:1040'>
  <skos:prefLabel>Electrical Test Engineering</skos:prefLabel>
  <skos:altLabel>TSTELECT</skos:altLabel>
  <skos:broader rdf:resource='urn:comp:10'/>
  <skos:scopeNote>Knowledge of the principles of electrical engineering, and
    electronic manufacturing to test components, systems, or
    subsystems under development for their functioning,
    efficacy and conformance to design requirements, or to test
    prototypes for feasibility. May involve ability to plan,
    create test procedures, conduct, and evaluate
    developmental, qualification, acceptance, and flight test
    and checkout requirements testing in accordance with NASA,
    Military or Commercial Specifications of air, space and
    ground systems, components, piece parts, as well as
    integrated electronic systems or sub-systems. Includes
    knowledge of environmental test techniques used to verify
    workmanship and validate operations in a relevant
    environment, including vibration, shock, acoustics,
    electromagnetic interference and compatibility (EMI/EMC),
    depressurization and vacuum operation, and thermal cycling.
  </skos:scopeNote>
  <nt2:status>Approved</nt2:status>
  <nt2:type>Descriptor</nt2:type>
  <nt2:inputdate>2006-12-13</nt2:inputdate>
  <dcterms:modified>2006-12-13</dcterms:modified>
  <nt2:code>1040</nt2:code>
 </skos:Concept>
 <skos:Concept rdf:about='urn:comp:160'>
  <skos:prefLabel>Metrology and Calibration Competency</skos:prefLabel>
  <skos:altLabel>METROLOGY</skos:altLabel>
  <skos:broader rdf:resource='urn:comp:1294'/>
  <skos:scopeNote>This competency refers to the knowledge, capabilities and
    responsibilities associated with the NASA Metrology and
    Calibration Program. It requires an understanding of the
    science of measurement and the comparing of a standard of
    known accuracy with a unit of test and measuring equipment
    (TME) for the purpose of detecting, correlating, reporting,
    or eliminating by adjustment any deviation in the accuracy
    of the unit being compared. It requires application of
    traceability principles and uncertainty analyses in
    relating those measurements to National standards,
    intrinsic standards, derived standards, or acceptable
    measurement systems through an unbroken chain of
    comparisons. This competency also includes understanding
    calibration laboratory requirements, their origin and
    purpose, application to contracts, use in auditing and
    surveillance, implementation in management and quality
    systems, and the impact of deficiencies, such as,
    out-of-tolerance TME.
  </skos:scopeNote>
  <nt2:status>Approved</nt2:status>
  <nt2:type>Descriptor</nt2:type>
  <nt2:inputdate>2006-12-13</nt2:inputdate>
  <dcterms:modified>2006-12-13</dcterms:modified>
  <nt2:code>160</nt2:code>
 </skos:Concept>
 <skos:Concept rdf:about='urn:comp:153'>
  <skos:prefLabel>Technical Management</skos:prefLabel>
  <skos:altLabel>TECHMMT</skos:altLabel>
  <skos:broader rdf:resource='urn:comp:1372'/>
  <skos:scopeNote>Knowledge, capabilities, and practices of technical
    formulation, planning, implementing, integration and
    managing of complex engineering work. This includes special
    knowledge in field of expertise, technical resources
    management to meet mission specific technical milestones,
    and processes associated with mitigating or accepting risk.
  </skos:scopeNote>
  <nt2:status>Approved</nt2:status>
  <nt2:type>Descriptor</nt2:type>
  <nt2:inputdate>2006-12-13</nt2:inputdate>
  <dcterms:modified>2006-12-13</dcterms:modified>
  <nt2:code>153</nt2:code>
 </skos:Concept>
 <skos:Concept rdf:about='urn:comp:1009'>
  <skos:prefLabel>Fatigue, Alertness, Circadian Rhythms Fundamental Research</skos:prefLabel>
  <skos:altLabel>HFRATIGUE</skos:altLabel>
  <skos:broader rdf:resource='urn:comp:40'/>
  <skos:scopeNote>TBD
  </skos:scopeNote>
  <nt2:status>Approved</nt2:status>
  <nt2:type>Descriptor</nt2:type>
  <nt2:inputdate>2006-12-13</nt2:inputdate>
  <dcterms:modified>2006-12-13</dcterms:modified>
  <nt2:code>1009</nt2:code>
 </skos:Concept>
 <skos:Concept rdf:about='urn:comp:119'>
  <skos:prefLabel>Budgeting Management</skos:prefLabel>
  <skos:altLabel>BUDGETMMT</skos:altLabel>
  <skos:broader rdf:resource='urn:comp:1150'/>
  <skos:scopeNote>Knowledge of how to apply management knowledge, principles
    and practices to obtain, utilize, manage financial
    resources in the workplace to meet program, project or
    business requirements. Involves maintaining available
    resources, making resource decisions based on need and
    availability, and developing and implementing strategies to
    make rational and well thought-out decisions related to
    organizational resources. Includes the ability to provide
    guidance, formulate a budget plan, defend a budget plan,
    assess budget performance, advocate budget and alternative
    scenarios and execute a budget plan. Requires knowledge of
    policies and practices related to Federal, Agency and
    Installation accounting, and internal business information
    systems.
  </skos:scopeNote>
  <nt2:status>Approved</nt2:status>
  <nt2:type>Descriptor</nt2:type>
  <nt2:inputdate>2006-12-13</nt2:inputdate>
  <dcterms:modified>2006-12-13</dcterms:modified>
  <nt2:code>119</nt2:code>
 </skos:Concept>
 <skos:Concept rdf:about='urn:comp:55'>
  <skos:prefLabel>Astromaterials, Collections, Curation &amp; Analysis</skos:prefLabel>
  <skos:altLabel>ASTROMATER</skos:altLabel>
  <skos:broader rdf:resource='urn:comp:1407'/>
  <skos:scopeNote>Apply knowledge of foreign materials, and planetary
    sciences to the collection of materials from foreign
    planets, and developing and using appropriate processes for
    handling and curating them. Includes knowledge and skill in
    processing the materials to protect Earth system from
    contamination.
  </skos:scopeNote>
  <nt2:status>Approved</nt2:status>
  <nt2:type>Descriptor</nt2:type>
  <nt2:inputdate>2006-12-13</nt2:inputdate>
  <dcterms:modified>2006-12-13</dcterms:modified>
  <nt2:code>55</nt2:code>
 </skos:Concept>
 <skos:Concept rdf:about='urn:comp:2'>
  <skos:prefLabel>Mission Flight Design</skos:prefLabel>
  <skos:altLabel>FLTDSG</skos:altLabel>
  <skos:broader rdf:resource='urn:comp:1231'/>
  <skos:changeNote>???
  </skos:changeNote>
  <skos:scopeNote>Knowledge and ability to conduct computational analysis of
    air and space vehicle flight design for mission
    implementation, including sequencing, trajectory
    optimization, orbital mechanics, flight mechanics and
    celestial mechanics. Use flight design modeling and
    simulation tools that determine optimum trajectory
    solutions. Includes in-depth analysis of air borne and
    ground-based trajectory predictions, automated trajectory
    planning and modeling and trajectory negotiation and data
    exchange as well as optimization tools which take into
    account environmental and design constraints. Involves
    analysis of flight dispersion variables and navigation
    predict generation.
  </skos:scopeNote>
  <nt2:status>Approved</nt2:status>
  <nt2:type>Descriptor</nt2:type>
  <nt2:inputdate>2006-12-13</nt2:inputdate>
  <dcterms:dateAccepted>2005-12-07</dcterms:dateAccepted>
  <dcterms:modified>2006-12-18</dcterms:modified>
  <nt2:code>2</nt2:code>
 </skos:Concept>
 <skos:Concept rdf:about='urn:comp:1430'>
  <skos:prefLabel>Biological Sciences Competency Suite</skos:prefLabel>
  <skos:broader rdf:resource='urn:comp:1406'/>
  <skos:narrower rdf:resource='urn:comp:156'/>
  <skos:narrower rdf:resource='urn:comp:34'/>
  <skos:narrower rdf:resource='urn:comp:31'/>
  <skos:narrower rdf:resource='urn:comp:32'/>
  <nt2:status>Approved</nt2:status>
  <nt2:type>Descriptor</nt2:type>
  <nt2:inputdate>2006-12-13</nt2:inputdate>
  <dcterms:modified>2006-12-13</dcterms:modified>
  <nt2:code>1430</nt2:code>
 </skos:Concept>
 <skos:Concept rdf:about='urn:comp:97'>
  <skos:prefLabel>Crew Systems and Aviation Operations</skos:prefLabel>
  <skos:altLabel>CSAOPS</skos:altLabel>
  <skos:broader rdf:resource='urn:comp:1244'/>
  <skos:scopeNote>Knowledge, capabilities, and practices associated with
    research and technology in analytical and experimental
    methods for pilot/automation integration, crew station
    design, and aerospace vehicle operations concepts.
  </skos:scopeNote>
  <nt2:status>Approved</nt2:status>
  <nt2:type>Descriptor</nt2:type>
  <nt2:inputdate>2006-12-13</nt2:inputdate>
  <dcterms:modified>2006-12-13</dcterms:modified>
  <nt2:code>97</nt2:code>
 </skos:Concept>
 <skos:Concept rdf:about='urn:comp:47'>
  <skos:prefLabel>Hydrological Science</skos:prefLabel>
  <skos:altLabel>HYDROSCI</skos:altLabel>
  <skos:broader rdf:resource='urn:comp:1415'/>
  <skos:scopeNote>Knowledge of the scientific study of waters of the earth,
    especially with relation to the effects of precipitation
    and evaporation upon the occurrence and character of water
    in streams, lakes and on or below the land surface.
    Includes understanding of the hydrologic cycle from
    precipitation to evaporation or return of the water to the
    seas, and application of findings to predict rates and
    amounts of runoff in rivers, assess required spillway and
    reservoir capacities, determine soil-water-plant
    relationships in agriculture and manage water supplies.
  </skos:scopeNote>
  <nt2:status>Approved</nt2:status>
  <nt2:type>Descriptor</nt2:type>
  <nt2:inputdate>2006-12-13</nt2:inputdate>
  <dcterms:modified>2006-12-13</dcterms:modified>
  <nt2:code>47</nt2:code>
 </skos:Concept>
 <skos:Concept rdf:about='urn:comp:1168'>
  <skos:prefLabel>Counterintelligence/Counterterrorism Analysis, Investigation and Liaison(SECOUNTER) [1073]</skos:prefLabel>
  <skos:broader rdf:resource='urn:comp:126'/>
  <skos:scopeNote>Knowledge, capabilities and practices associated with
    receipt, analysis, dissemination and investigation of
    information for the purpose of detecting, deterring and
    neutralizing acts involving espionage, intelligence
    activities, sabotage and/or terrorist activities conducted
    for or on behalf of foreign powers, organizations or
    persons.
  </skos:scopeNote>
  <nt2:status>Approved</nt2:status>
  <nt2:type>Descriptor</nt2:type>
  <nt2:inputdate>2006-12-13</nt2:inputdate>
  <dcterms:modified>2006-12-13</dcterms:modified>
  <nt2:code>1168</nt2:code>
 </skos:Concept>
 <skos:Concept rdf:about='urn:comp:12'>
  <skos:prefLabel>Electromagnetics</skos:prefLabel>
  <skos:altLabel>ELMAG</skos:altLabel>
  <skos:broader rdf:resource='urn:comp:1294'/>
  <skos:scopeNote>Knowledge, capabilities, and practices associated with
    research and technology in analytical, computational, and
    experimental methods to quantify and control complex
    electromagnetics phenomena to address issues such as
    electromagnetic interference, electromagnetic
    compatibility, electrostatic discharge, and advanced
    integral/conformal antennas. Also includes engineering
    design of systems and how they will react given
    electromagnetic fields, compatibility, interference and
    discharge.
  </skos:scopeNote>
  <nt2:status>Approved</nt2:status>
  <nt2:type>Descriptor</nt2:type>
  <nt2:inputdate>2006-12-13</nt2:inputdate>
  <dcterms:modified>2006-12-13</dcterms:modified>
  <nt2:code>12</nt2:code>
 </skos:Concept>
 <skos:Concept rdf:about='urn:comp:1023'>
  <skos:prefLabel>Perceptual Technologies and Standards</skos:prefLabel>
  <skos:altLabel>HFEPERCEPT</skos:altLabel>
  <skos:broader rdf:resource='urn:comp:41'/>
  <skos:scopeNote>TBD (includes visual display design, image and video
    compression, display composition and layout, icon design
    and font selection, auditory displays, multimodal
    environments)
  </skos:scopeNote>
  <nt2:status>Approved</nt2:status>
  <nt2:type>Descriptor</nt2:type>
  <nt2:inputdate>2006-12-13</nt2:inputdate>
  <dcterms:modified>2006-12-13</dcterms:modified>
  <nt2:code>1023</nt2:code>
 </skos:Concept>
 <skos:Concept rdf:about='urn:comp:106'>
  <skos:prefLabel>Fluid Systems</skos:prefLabel>
  <skos:altLabel>FLUIDSYS</skos:altLabel>
  <skos:broader rdf:resource='urn:comp:1359'/>
  <skos:scopeNote>Knowledge, capabilities, and practices associated with
    basic fluid physics research (including microgravitational
    study of complex fluids, multiphase and phase change, fluid
    dynamics and instabilities, and interfacial phenomena), as
    well as
    modeling and development, design, integration, analysis,
    test, operation and evaluation of aerospace ground and
    flight closed fluid systems. Knowledge of assessment of
    requirements, establishment of specifications and
    evaluation to insure proper function and compatibility of
    fluid systems hardware/components. Also includes
    integration of control logic and control systems design to
    ensurea fully functional process system, and design and
    development of instruments for imaging fluid leaks,
    evaluating sensitivity, vibration susceptibility and field
    usability to ensure safe implementation, particularly for
    hydraulic and pneumatic fluid power systems. This requires
    the basic knowledge and skill of mechanical design, fluid
    physics, fluid mechanics, component design, and integrated
    system layouts / designs and evaluation of their capability
    to satisfy functional and performance requirements. Agree
    with recommended change, however, move under new knowledge
    category mechanical engineering.
  </skos:scopeNote>
  <nt2:status>Approved</nt2:status>
  <nt2:type>Descriptor</nt2:type>
  <nt2:inputdate>2006-12-13</nt2:inputdate>
  <dcterms:modified>2006-12-13</dcterms:modified>
  <nt2:code>106</nt2:code>
 </skos:Concept>
 <skos:Concept rdf:about='urn:comp:140'>
  <skos:prefLabel>NASA Leadership Competency</skos:prefLabel>
  <skos:altLabel>NASALEADER</skos:altLabel>
  <skos:broader rdf:resource='urn:comp:1399'/>
  <skos:narrower rdf:resource='urn:comp:1001'/>
  <skos:narrower rdf:resource='urn:comp:1004'/>
  <skos:narrower rdf:resource='urn:comp:1002'/>
  <skos:narrower rdf:resource='urn:comp:1003'/>
  <skos:scopeNote>Knowledge, capabilities and practices associated with
    leading and managing change, people, and work of an
    organization. Includes awareness and understanding of
    relevant strategies and techniques to effectively create a
    vision for change and engage others to implement the change
    process. Knowledge of how to apply human capital and
    leadership strategies to empower individuals and teams to
    achieve shared outcomes and develop leadership capabilities
    in lower level managers. Understanding of range of
    practices that create an environment that values diversity,
    promotes
    inclusion of all employees, and leverages talents of all
    team members. Develop systems that allow effective
    assignment, prioritization and monitoring of work. Align
    work unit performance objectives with organizational
    objectives and removes obstacles and barriers to
    organizational and programmatic performance.
  </skos:scopeNote>
  <nt2:status>Approved</nt2:status>
  <nt2:type>Descriptor</nt2:type>
  <nt2:inputdate>2006-12-13</nt2:inputdate>
  <dcterms:modified>2006-12-13</dcterms:modified>
  <nt2:code>140</nt2:code>
 </skos:Concept>
 <skos:Concept rdf:about='urn:comp:1069'>
  <skos:prefLabel>Employee Assistance</skos:prefLabel>
  <skos:altLabel>OCCASSIST</skos:altLabel>
  <skos:broader rdf:resource='urn:comp:130'/>
  <skos:scopeNote>Professional knowledge and skills to improve the mental
    health and well being of employees. Knowledge of
    regulations and programs to coordinate, implement, manage
    and assess the effectiveness of related employee assistance
    programs, practices and policies, including substance abuse
    prevention and treatment in support of drug-free Federal
    workplace program. Knowledge to implement programs and
    training for all mental health concerns for employees and
    their immediate families. This includes critical incident
    stress or other traumatic events in the workplace,
    promotion of an emotionally healthy workforce, and
    assessment of regulations that potentially impact the
    workplace.
  </skos:scopeNote>
  <nt2:status>Approved</nt2:status>
  <nt2:type>Descriptor</nt2:type>
  <nt2:inputdate>2006-12-13</nt2:inputdate>
  <dcterms:modified>2006-12-13</dcterms:modified>
  <nt2:code>1069</nt2:code>
 </skos:Concept>
 <skos:Concept rdf:about='urn:comp:169'>
  <skos:prefLabel>Policy Management</skos:prefLabel>
  <skos:altLabel>POLICYMGMT</skos:altLabel>
  <skos:broader rdf:resource='urn:comp:1125'/>
  <skos:scopeNote>Knowledge of NASA relationships to headquarters, Centers,
    component facilities, partnerships and other government
    agencies, including international governments, in order to
    effectively integrate services consistent with broad
    strategies and objectives. Requires the capability to
    research and apply government-wide laws and Agency
    operating principles, regulations, and policies associated
    with organizational and business functions such as
    financial, human resources, legal, security,
    communications, inspection, compliance, and health and
    safety. Utilizes a wide variety of resources and tools to
    develop, maintain, monitor, enforce and provide oversight
    of NASA management requirements.
  </skos:scopeNote>
  <nt2:status>Approved</nt2:status>
  <nt2:type>Descriptor</nt2:type>
  <nt2:inputdate>2006-12-13</nt2:inputdate>
  <dcterms:modified>2006-12-13</dcterms:modified>
  <nt2:code>169</nt2:code>
 </skos:Concept>
 <skos:Concept rdf:about='urn:comp:1054'>
  <skos:prefLabel>Combustion Devices Design and Analysis</skos:prefLabel>
  <skos:altLabel>RPCOMBUST</skos:altLabel>
  <skos:broader rdf:resource='urn:comp:73'/>
  <skos:scopeNote>Knowledge, capabilities and practices associated with
    defining, developing, integrating and verifying liquid
    engine combustion devices for advanced propulsion systems.
    This includes ability to conduct preliminary design and
    analysis with respect to approach, dimensions, structural
    analysis, performance predictions and meeting engine
    balance requirements. Includes the ability to coordinate
    all activities necessary for finalization of design,
    fabrication, test planning, testing, and data analysis of
    combustion devices components which include, injectors,
    thrust chambers, nozzles, preburners, heat exchangers, and
    ignition systems.
  </skos:scopeNote>
  <nt2:status>Approved</nt2:status>
  <nt2:type>Descriptor</nt2:type>
  <nt2:inputdate>2006-12-13</nt2:inputdate>
  <dcterms:modified>2006-12-13</dcterms:modified>
  <nt2:code>1054</nt2:code>
 </skos:Concept>
 <skos:Concept rdf:about='urn:comp:82'>
  <skos:prefLabel>Software Engineering</skos:prefLabel>
  <skos:altLabel>SWENG</skos:altLabel>
  <skos:broader rdf:resource='urn:comp:1283'/>
  <skos:scopeNote>Knowledge and ability to apply systematic, disciplines and
    quantifiable approaches to the acquisition and development
    of software systems for spaceflight, ground support,
    airborne and facility applications. Development and
    management of simulations, tools and integrated software
    development environments for the design, development,
    verification, testing, manufacture, operation and
    maintenance of such systems. Specialized knowledge to
    predict, evaluate and manage critical performance
    attributes of software-intense systems such as real-time
    response and embedded hardware-driven resource limits.
    Includes knowledge of high-performance computing, graphical
    user interfaces, networking, data integrity and security.
  </skos:scopeNote>
  <nt2:status>Approved</nt2:status>
  <nt2:type>Descriptor</nt2:type>
  <nt2:inputdate>2006-12-13</nt2:inputdate>
  <dcterms:modified>2006-12-13</dcterms:modified>
  <nt2:code>82</nt2:code>
 </skos:Concept>
 <skos:Concept rdf:about='urn:comp:56'>
  <skos:prefLabel>Nanoscience</skos:prefLabel>
  <skos:altLabel>TINYSCI</skos:altLabel>
  <skos:broader rdf:resource='urn:comp:1424'/>
  <skos:scopeNote>Knowledge, capability and practices to study and research
    extremely small materials is such areas as their structure,
    shape how they act, and how their properties change as
    their size changes.
  </skos:scopeNote>
  <nt2:status>Approved</nt2:status>
  <nt2:type>Descriptor</nt2:type>
  <nt2:inputdate>2006-12-13</nt2:inputdate>
  <dcterms:modified>2006-12-13</dcterms:modified>
  <nt2:code>56</nt2:code>
 </skos:Concept>
 <skos:Concept rdf:about='urn:comp:118'>
  <skos:prefLabel>Financial Management</skos:prefLabel>
  <skos:altLabel>FINMMT</skos:altLabel>
  <skos:broader rdf:resource='urn:comp:1150'/>
  <skos:scopeNote>Knowledge of how to apply financial management skills,
    principles and practices, generally accepted accounting
    principles (GAAP), and the standards, policies and
    practices related to Federal, Agency and Installation
    accounting and financial management to obtain, utilize,
    manage and account for resources in the workplace. Ability
    to use accounting related tools and techniques, perform
    financial data analysis, compile and/or perform
    transactions, review related outputs, and identify problems
    and prepare standard documentation. Ability to develop and
    implement strategies to capture, record, maintain and
    allocate organizational resources rationally and
    effectively.
  </skos:scopeNote>
  <nt2:status>Approved</nt2:status>
  <nt2:type>Descriptor</nt2:type>
  <nt2:inputdate>2006-12-13</nt2:inputdate>
  <dcterms:modified>2006-12-13</dcterms:modified>
  <nt2:code>118</nt2:code>
 </skos:Concept>
</rdf:RDF>
